# Copyright 2016 ITEA 12004 SEAS Project.
# 
# Licensed under the Apache License, Version 2.0 (the "License");
# you may not use this file except in compliance with the License.
# You may obtain a copy of the License at
# 
#      http://www.apache.org/licenses/LICENSE-2.0
# 
# Unless required by applicable law or agreed to in writing,
# distributed under the License is distributed on an "AS IS" BASIS,
# WITHOUT WARRANTIES OR CONDITIONS OF ANY KIND, either express or implied.
# See the License for the specific language governing permissions and
# limitations under the License.

@prefix rdf: <http://www.w3.org/1999/02/22-rdf-syntax-ns#> . #Resource data framework
@prefix owl: <http://www.w3.org/2002/07/owl#> .              #Owl ontology language
@prefix rdfs: <http://www.w3.org/2000/01/rdf-schema#> .      #RDF schema 
@prefix xsd: <http://www.w3.org/2001/XMLSchema#> .           #XML standard datatypes
@prefix dc: <http://purl.org/dc/terms/> .     #Dublin Core Metadata Initiative terms
@prefix vann: <http://purl.org/vocab/vann/> .  #A vocabulary for annotating vocabulary descriptions
@prefix voaf: <http://purl.org/vocommons/voaf#> . #A vocabulary of a friend, for describing relations between linked vocabularies
@prefix vs: <http://www.w3.org/2003/06/sw-vocab-status/ns#> . #Semantic web vocabulary status ontology
@prefix cc: <http://creativecommons.org/ns#>.
@prefix foaf: <http://xmlns.com/foaf/0.1/>.
@prefix saref: <http://ontology.tno.nl/saref#>. #SAREF smart building appliances ontology
@prefix qudt: <http://data.qudt.org/qudt/owl/1.0.0/qudt.owl#> . #QUDT quantities
@prefix qudt-unit: <http://data.qudt.org/qudt/owl/1.0.0/unit.owl#> . #QUDT units
@prefix ssn: <http://www.w3.org/ns/ssn/>.
@prefix skos: <http://www.w3.org/2004/02/skos/core#>.
@prefix sdmx: <http://purl.org/linked-data/sdmx#>.

@prefix seas: <https://w3id.org/seas/>.
@base <https://w3id.org/seas/>.

seas:FlexibilityVocabulary rdf:type voaf:Vocabulary , owl:Ontology ;
  dc:title "SEAS-Flexibility ontology"@en ;
  dc:description """The SEAS Flexibility Vocabulary defines code lists to interpret evaluations of operating features of interest. For instance, the value may be the minimal operating value"""@en ;
  dc:issued "2016-07-24"^^xsd:date ;
  dc:modified "2016-07-24"^^xsd:date ;
  dc:author <http://www.maxime-lefrancois.info/me#> ;
  cc:license <https://creativecommons.org/licenses/by/4.0> ;
  vann:preferredNamespacePrefix "seas" ;
  vann:preferredNamespaceUri <https://w3id.org/seas/> ;  
#  owl:imports seas:EvaluationOntology ;
  owl:versionIRI <https://w3id.org/seas/FlexibilityVocabulary-1.0> ;
  owl:versionInfo "v1.0" .


# CL_FLEX
seas:flexibility a skos:ConceptScheme, sdmx:CodeList;
  rdfs:label "Flexibility - codelist scheme"@en;
  skos:prefLabel "Flexibility - codelist scheme"@en;
  skos:notation "CL_FLEX";
  rdfs:comment """This code list enables to interpret the flexibility of the property."""@en;
  skos:note """This code list enables to interpret the flexibility of the property."""@en;
  skos:definition seas:flexibility ;
  rdfs:seeAlso seas:Flexibility ;
  vs:term_status "testing" ;
  rdfs:isDefinedBy seas:FlexibilityVocabulary .

seas:Flexibility a rdfs:Class, owl:Class;
  rdfs:subClassOf skos:Concept ;
  rdfs:label "Flexibility - codelist class"@en;
  rdfs:comment """This code list enables to interpret the flexibility of the property."""@en;
  rdfs:seeAlso seas:flexibility ;
  vs:term_status "testing" ;
  rdfs:isDefinedBy seas:FlexibilityVocabulary . 

seas:flex-Reduction a skos:Concept, seas:EvaluationInterpretationConcept, seas:Flex;
  rdfs:label "Reduction"@en ;
  skos:prefLabel "Reduction"@en ;
  skos:notation "-" ;
  rdfs:comment """Reduction means that the given value is the reduction flexibility of the quantity value."""@en ;
  skos:definition """Reduction means that the given value is the reduction flexibility of the quantity value."""@en ;
  skos:topConceptOf seas:flexibility;
  skos:inScheme   seas:flexibility;
  vs:term_status "testing" ;
  rdfs:isDefinedBy seas:FlexibilityVocabulary . 

seas:flexibility skos:hasTopConcept seas:flex-Reduction .

seas:flex-Cut a skos:Concept, seas:EvaluationInterpretationConcept, seas:Flex;
  rdfs:label "Cut"@en ;
  skos:prefLabel "Cut"@en ;
  skos:notation "Cut" ;
  rdfs:comment """Cut means that the given value is the cut flexibility of the quantity value."""@en ;
  skos:definition """Cut means that the given value is the cut flexibility of the quantity value."""@en ;
  skos:topConceptOf seas:flexibility;
  skos:inScheme   seas:flexibility;
  vs:term_status "testing" ;
  rdfs:isDefinedBy seas:FlexibilityVocabulary . 

seas:flexibility skos:hasTopConcept seas:flex-Cut .

seas:flex-Move a skos:Concept, seas:EvaluationInterpretationConcept, seas:Flex;
  rdfs:label "Move"@en ;
  skos:prefLabel "Move"@en ;
  skos:notation "Move" ;
  rdfs:comment """Move means that the given value is the Move flexibility of the quantity value."""@en ;
  skos:definition """Move means that the given value is the Move flexibility of the quantity value."""@en ;
  skos:topConceptOf seas:flexibility;
  skos:inScheme   seas:flexibility;
  vs:term_status "testing" ;
  rdfs:isDefinedBy seas:FlexibilityVocabulary . 

seas:flexibility skos:hasTopConcept seas:flex-Move .

seas:flex-Augmentation a skos:Concept, seas:EvaluationInterpretationConcept, seas:Flex;
  rdfs:label "Augmentation"@en ;
  skos:prefLabel "Augmentation"@en ;
  skos:notation "Augmentation" ;
  rdfs:comment """Augmentation means that the given value is the Augmentation flexibility of the quantity value."""@en ;
  skos:definition """Augmentation means that the given value is the Augmentation flexibility of the quantity value."""@en ;
  skos:topConceptOf seas:flexibility;
  skos:inScheme   seas:flexibility;
  vs:term_status "testing" ;
  rdfs:isDefinedBy seas:FlexibilityVocabulary . 

seas:flexibility skos:hasTopConcept seas:flex-Augmentation .
