# Copyright 2016 ITEA 12004 SEAS Project.
# 
# Licensed under the Apache License, Version 2.0 (the "License");
# you may not use this file except in compliance with the License.
# You may obtain a copy of the License at
# 
#      http://www.apache.org/licenses/LICENSE-2.0
# 
# Unless required by applicable law or agreed to in writing,
# distributed under the License is distributed on an "AS IS" BASIS,
# WITHOUT WARRANTIES OR CONDITIONS OF ANY KIND, either express or implied.
# See the License for the specific language governing permissions and
# limitations under the License.

@prefix rdf: <http://www.w3.org/1999/02/22-rdf-syntax-ns#> . #Resource data framework
@prefix owl: <http://www.w3.org/2002/07/owl#> .     #Owl ontology language
@prefix rdfs: <http://www.w3.org/2000/01/rdf-schema#> .   #RDF schema 
@prefix xsd: <http://www.w3.org/2001/XMLSchema#> .  #XML standard datatypes
@prefix dc: <http://purl.org/dc/terms/> .  #Dublin Core Metadata Initiative terms
@prefix vann: <http://purl.org/vocab/vann/> .  #A vocabulary for annotating vocabulary descriptions
@prefix voaf: <http://purl.org/vocommons/voaf#> . #A vocabulary of a friend, for describing relations between linked vocabularies
@prefix vs: <http://www.w3.org/2003/06/sw-vocab-status/ns#> . #Semantic web vocabulary status ontology
@prefix foaf: <http://xmlns.com/foaf/0.1/>.
@prefix ssn: <https://www.w3.org/ns/ssn/>.
@prefix cc: <http://creativecommons.org/ns#>.
@prefix dul: <http://www.ontologydesignpatterns.org/ont/dul/DUL.owl#>. # The DOLCE+DnS Ultralite ontology.
@prefix liner: <https://w3id.org/liner/>.
@prefix skos: <http://www.w3.org/2004/02/skos/core#>.
@prefix qb: <http://purl.org/linked-data/cube#>.
@prefix cdt: <http://w3id.org/lindt/custom_datatypes#>.

@prefix seas: <https://w3id.org/seas/>.
@base <https://w3id.org/seas/>.

seas:PowerSystemVocabulary a owl:Ontology , voaf:Vocabulary ;
  dc:title "seas-PowerSystem vocabulary."@en ;
  dc:description """This vocabulary defines power Systems, and their common properties."""@en ;
  dc:issued "2016-07-19"^^xsd:date ;
  dc:modified "2016-07-19"^^xsd:date ;
  dc:author <http://www.maxime-lefrancois.info/me#> ;
  dc:contributor <https://w3id.org/people/gabrieljlsantos#> ;
  dc:contributor <https://w3id.org/people/franciscosilva#> ;
  dc:contributor <https://w3id.org/people/brigidateixeira#> ;
  cc:license <http://creativecommons.org/licenses/by/4.0/> ;
  vann:preferredNamespacePrefix "seas" ;
  vann:preferredNamespaceUri <https://w3id.org/seas/> ;  
  owl:versionIRI <https://w3id.org/seas/PowerSystemVocabulary/0.10> ;
  owl:versionInfo "v0.10" .

seas:PowerSystem a owl:Class ;
  rdfs:label "Power System" ;
  rdfs:label "Sistemas Elétricos de Energia"@pt ;
  rdfs:comment """The class of systems that are capable of producing, storing, or consuming electricity, and exchange electricity with other systems."""@en ;
  rdfs:subClassOf seas:System ;
  vs:term_status "testing" ;
  rdfs:isDefinedBy seas:PowerSystemVocabulary .

seas:powerConnectedTo a owl:ObjectProperty ;
  rdfs:label "Power connected to"@en ;
  rdfs:comment "The subject power system is connected to the object power system, and electricity can flow between the systems."@en ;
  rdfs:subPropertyOf seas:connectedTo ;
  rdfs:domain seas:PowerSystem ;
  rdfs:range seas:PowerSystem ;
  vs:term_status "testing" ;
  rdfs:isDefinedBy seas:PowerSystemVocabulary .

seas:PowerBus a owl:Class ;
  rdfs:label "Power Bus"@en ;
  rdfs:comment """The class of power buses. A bus is a power systems composed of three phase wires: R, S, T, and a neutral wire N. Other power systems can be connected to a power bus with different connection configurations."""@en ;
  vs:term_status "testing" ;
  rdfs:isDefinedBy seas:PowerSystemVocabulary .

# transmission 

seas:PowerTransmissionSystem a owl:Class ;
  rdfs:subClassOf seas:PowerSystem;
  rdfs:label "PowerTransmission System"@en ;
  rdfs:label "Sistema de Transmissão"@pt ;
  rdfs:comment """The class of systems that are capable of transmitting electricity between two buses."""@en ;
  vs:term_status "testing" ;
  rdfs:isDefinedBy seas:PowerSystemVocabulary .

seas:bus1 a rdf:Property, owl:ObjectProperty, owl:FunctionalProperty ;
  rdfs:label "bus 1"@en ;
  rdfs:comment """The Transmission Systems are always connected to 2 buses. This is the bus 1."""@en ;
  rdfs:subPropertyOf seas:powerConnectedTo;
  rdfs:domain seas:PowerTransmissionSystem;
  rdfs:range seas:PowerBus ;
  vs:term_status "testing" ;
  rdfs:isDefinedBy seas:PowerSystemVocabulary .

seas:bus2 a rdf:Property, owl:ObjectProperty, owl:FunctionalProperty ;
  rdfs:label "bus 2"@en ;
  rdfs:comment """The Transmission Systems are always connected to 2 buses. This is the bus 2."""@en ;
  rdfs:subPropertyOf seas:powerConnectedTo;
  rdfs:domain seas:PowerTransmissionSystem;
  rdfs:range seas:PowerBus ;
  vs:term_status "testing" ;
  rdfs:isDefinedBy seas:PowerSystemVocabulary .

seas:bus1 owl:propertyDisjointWith seas:bus2 .
  

seas:PowerLine a owl:Class ;
  rdfs:label "Power Line"@en ;
  rdfs:comment """The class of power lines, that transmit electricity on a certain distance within a power network."""@en ;
  rdfs:subClassOf seas:PowerTransmissionSystem ;
  vs:term_status "testing" ;
  rdfs:isDefinedBy seas:PowerSystemVocabulary .

seas:PowerTransformer a owl:Class ;
  rdfs:label "Power Transformer"@en ;
  rdfs:label "Transformador"@pt ;
  rdfs:comment """The class of systems that are capable of transforming electricity within a power network."""@en ;
  rdfs:subClassOf seas:PowerTransmissionSystem ;
  vs:term_status "testing" ;
  rdfs:isDefinedBy seas:PowerSystemVocabulary .


seas:primarilyConnectedTo a owl:ObjectProperty ;
  rdfs:label "primarily Connected To"@en ;
  rdfs:comment """The Transformer is always connected to 2 buses. This is the primary."""@en ;
  rdfs:subPropertyOf seas:bus1 ;
  rdfs:domain seas:PowerTransformer ;
  rdfs:range seas:PowerBus ;
  vs:term_status "testing" ;
  rdfs:isDefinedBy seas:TransformerVocabulary .

seas:secondarilyConnectedTo a owl:ObjectProperty ;
  rdfs:label "secondarily Connected To"@en ;
  rdfs:comment """The Transformer is always connected to 2 buses. This is the secondary."""@en ;
  rdfs:subPropertyOf seas:bus2 ;
  rdfs:domain seas:PowerTransformer ;
  rdfs:range seas:PowerBus ;
  vs:term_status "testing" ;
  rdfs:isDefinedBy seas:TransformerVocabulary .


seas:SingleBusSystem a owl:Class ;
  rdfs:label "Single Bus System"@en ;
  rdfs:label "Sistema de Barramento único"@pt ;
  rdfs:comment """The class of systems that are connected to a single Bus, such as: Loads, Generators or Storages"""@en ;
  owl:disjointUnionOf ( seas:PowerLoad seas:PowerGenerator seas:PowerStorage ) ;
  rdfs:subClassOf seas:PowerSystem ;
  vs:term_status "testing" ;
  rdfs:isDefinedBy seas:SingleBusSystemVocabulary .

seas:PowerLoad a owl:Class ;
  rdfs:subClassOf seas:PowerSystem ;  
  rdfs:label "Load"@en ;
  rdfs:comment """Power System that consumes electricity."""@en ;
  vs:term_status "testing" ;
  rdfs:isDefinedBy seas:PowerLoadVocabulary .

seas:PowerStorage a owl:Class ;
  rdfs:subClassOf seas:SingleBusSystem ;
  rdfs:label "Power Storage"@en ;
  rdfs:label "Bateria"@pt ;
  rdfs:comment """The class of systems that are capable of storing electricity."""@en ;
  vs:term_status "testing" ;
  rdfs:isDefinedBy seas:StorageVocabulary .

seas:PowerGenerator a owl:Class ;
  rdfs:subClassOf seas:PowerSystem ;
  rdfs:label "Generator"@en ;
  rdfs:comment """The class of power systems that converts mechanical energy to electrical energy."""@en ;
  vs:term_status "testing" ;
  rdfs:isDefinedBy seas:PowerGeneratorVocabulary .

seas:energyForm a owl:ObjectProperty ;
  rdfs:label "Energy Form" ;
  rdfs:comment """The source type of energy."""@en ;
  rdfs:domain seas:PowerGenerator ;
  rdfs:range seas:EnergyForm ;
  vs:term_status "testing" ;
  rdfs:isDefinedBy seas:PowerGeneratorVocabulary .

