# Copyright 2016 ITEA 12004 SEAS Project.
# 
# Licensed under the Apache License, Version 2.0 (the "License");
# you may not use this file except in compliance with the License.
# You may obtain a copy of the License at
# 
#      http://www.apache.org/licenses/LICENSE-2.0
# 
# Unless required by applicable law or agreed to in writing,
# distributed under the License is distributed on an "AS IS" BASIS,
# WITHOUT WARRANTIES OR CONDITIONS OF ANY KIND, either express or implied.
# See the License for the specific language governing permissions and
# limitations under the License.

@prefix rdf: <http://www.w3.org/1999/02/22-rdf-syntax-ns#> . #Resource data framework
@prefix owl: <http://www.w3.org/2002/07/owl#> .     #Owl ontology language
@prefix rdfs: <http://www.w3.org/2000/01/rdf-schema#> .   #RDF schema 
@prefix xsd: <http://www.w3.org/2001/XMLSchema#> .  #XML standard datatypes
@prefix dc: <http://purl.org/dc/terms/> .  #Dublin Core Metadata Initiative terms
@prefix vann: <http://purl.org/vocab/vann/> .  #A vocabulary for annotating vocabulary descriptions
@prefix voaf: <http://purl.org/vocommons/voaf#> . #A vocabulary of a friend, for describing relations between linked vocabularies
@prefix vs: <http://www.w3.org/2003/06/sw-vocab-status/ns#> . #Semantic web vocabulary status ontology
@prefix foaf: <http://xmlns.com/foaf/0.1/>.
@prefix ssn: <https://www.w3.org/ns/ssn/>.
@prefix cc: <http://creativecommons.org/ns#>.
@prefix dul: <http://www.ontologydesignpatterns.org/ont/dul/DUL.owl#>. # The DOLCE+DnS Ultralite ontology.
@prefix liner: <https://w3id.org/liner/>.
@prefix skos: <http://www.w3.org/2004/02/skos/core#>.
@prefix qb: <http://purl.org/linked-data/cube#>.
@prefix cdt: <http://w3id.org/lindt/custom_datatypes#>.

@prefix seas: <https://w3id.org/seas/>.
@base <https://w3id.org/seas/>.

seas:PowerSystemVocabulary a owl:Ontology , voaf:Vocabulary ;
  dc:title "seas-PowerSystem vocabulary."@en ;
  dc:description """This vocabulary defines common properties of power systems, and evaluation interpretation code lists."""@en ;
  dc:issued "2016-07-19"^^xsd:date ;
  dc:modified "2016-07-19"^^xsd:date ;
  dc:author <http://www.maxime-lefrancois.info/me#> ;
  dc:contributor <https://w3id.org/people/gabrieljlsantos#> ;
  dc:contributor <https://w3id.org/people/franciscosilva#> ;
  dc:contributor <https://w3id.org/people/brigidateixeira#> ;
  cc:license <http://creativecommons.org/licenses/by/4.0/> ;
  vann:preferredNamespacePrefix "seas" ;
  vann:preferredNamespaceUri <https://w3id.org/seas/> ;  
  owl:versionIRI <https://w3id.org/seas/PowerSystemVocabulary/0.10> ;
  owl:versionInfo "v0.10" .

seas:voltage a seas:PropertyKey, rdf:Property ;
  rdfs:label "voltage" ;
  rdfs:comment """Voltage is the voltage at some connection with a bus."""@en ;
  rdfs:subPropertyOf seas:hasProperty ;
  rdfs:domain seas:PowerSystem ;
  rdfs:range seas:QuantifiableProperty ;
  vs:term_status "testing" ;
  rdfs:isDefinedBy seas:PowerSystemVocabulary .

seas:current a seas:PropertyKey, rdf:Property ;
  rdfs:label "current" ;
  rdfs:comment """Current is the current at some connection with a bus."""@en ;
  rdfs:subPropertyOf seas:hasProperty ;
  rdfs:domain seas:PowerSystem ;
  rdfs:range seas:QuantifiableProperty ;
  vs:term_status "testing" ;
  rdfs:isDefinedBy seas:PowerSystemVocabulary .

seas:consumptionPower a seas:PropertyKey, rdf:Property ;
  rdfs:label "consumption Power" ;
  rdfs:comment """Consumption Power is the sum of the electric power that is consumed by the system and its sub systems."""@en ;
  rdfs:subPropertyOf seas:hasProperty ;
  rdfs:domain seas:PowerSystem ;
  rdfs:range seas:QuantifiableProperty ;
  vs:term_status "testing" ;
  rdfs:isDefinedBy seas:PowerSystemVocabulary .

seas:productionPower a seas:PropertyKey, rdf:Property ;
  rdfs:label "production Power" ;
  rdfs:comment """Production Power is the sum of the electric power that is produced by the system and its sub systems."""@en ;
  rdfs:subPropertyOf seas:hasProperty ;
  rdfs:domain seas:PowerSystem ;
  rdfs:range seas:QuantifiableProperty ;
  vs:term_status "testing" ;
  rdfs:isDefinedBy seas:PowerSystemVocabulary .

seas:storagePower a seas:PropertyKey, rdf:Property ;
  rdfs:label "storage Power" ;
  rdfs:comment """Storage Power is the electric power that is stored, usually in a battery, an electric vehicle, or a microgrid."""@en ;
  rdfs:subPropertyOf seas:hasProperty ;
  rdfs:domain seas:PowerSystem ;
  rdfs:range seas:QuantifiableProperty ;
  vs:term_status "testing" ;
  rdfs:isDefinedBy seas:PowerSystemVocabulary .

seas:incomingPower a seas:PropertyKey, rdf:Property ;
  rdfs:label "incoming Power" ;
  rdfs:comment """Incoming Power is the sum of the electric power that enter the system from the exterior."""@en ;
  rdfs:subPropertyOf seas:hasProperty ;
  rdfs:domain seas:PowerSystem ;
  rdfs:range seas:QuantifiableProperty ;
  vs:term_status "testing" ;
  rdfs:isDefinedBy seas:PowerSystemVocabulary .

seas:outgoingPower a seas:PropertyKey, rdf:Property ;
  rdfs:label "outgoing Power" ;
  rdfs:comment """Outgoing Power is the sum of the electric power that leaves the system to the exterior."""@en ;
  rdfs:subPropertyOf seas:hasProperty ;
  rdfs:domain seas:PowerSystem ;
  rdfs:range seas:QuantifiableProperty ;
  vs:term_status "testing" ;
  rdfs:isDefinedBy seas:PowerSystemVocabulary .

seas:powerBalance a seas:PropertyKey, rdf:Property ;
  rdfs:label "Power Balance" ;
  rdfs:comment """Power Balance is equal to the sum of:
  The electric consumption minus the electric production plus the storage power.

  It is also equal to the sum of:
  The outgoing electric power minus the incoming electric power."""@en ;
  rdfs:subPropertyOf seas:hasProperty ;
  rdfs:domain seas:PowerSystem ;
  rdfs:range seas:QuantifiableProperty ;
  vs:term_status "testing" ;
  rdfs:isDefinedBy seas:PowerSystemVocabulary .

seas:consumedEnergy a seas:PropertyKey, rdf:Property ;
  rdfs:label "consumed energy" ;
  rdfs:comment """Consumed Energy is the sum of the electric energy that is consumed by the system and its sub systems."""@en ;
  rdfs:subPropertyOf seas:hasProperty ;
  rdfs:domain seas:PowerSystem ;
  rdfs:range seas:QuantifiableProperty ;
  vs:term_status "testing" ;
  rdfs:isDefinedBy seas:PowerSystemVocabulary .

seas:productedEnergy a seas:PropertyKey, rdf:Property ;
  rdfs:label "produced Energy" ;
  rdfs:comment """Produced Energy is the sum of the electric energy that is produced by the system and its sub systems."""@en ;
  rdfs:subPropertyOf seas:hasProperty ;
  rdfs:domain seas:PowerSystem ;
  rdfs:range seas:QuantifiableProperty ;
  vs:term_status "testing" ;
  rdfs:isDefinedBy seas:PowerSystemVocabulary .

seas:storedEnergy a seas:PropertyKey, rdf:Property ;
  rdfs:label "stored Energy" ;
  rdfs:comment """Stored Energy is the electric energy that is stored, usually in a battery, an electric vehicle, or a microgrid."""@en ;
  rdfs:subPropertyOf seas:hasProperty ;
  rdfs:domain seas:PowerSystem ;
  rdfs:range seas:QuantifiableProperty ;
  vs:term_status "testing" ;
  rdfs:isDefinedBy seas:PowerSystemVocabulary .

seas:totalIncomingEnergy a seas:PropertyKey, rdf:Property ;
  rdfs:label "total Incoming Energy" ;
  rdfs:comment """total incoming Energy is the sum of the electric energy that entered the system from the exterior."""@en ;
  rdfs:subPropertyOf seas:hasProperty ;
  rdfs:domain seas:PowerSystem ;
  rdfs:range seas:QuantifiableProperty ;
  vs:term_status "testing" ;
  rdfs:isDefinedBy seas:PowerSystemVocabulary .

seas:totalOutgoingEnergy a seas:PropertyKey, rdf:Property ;
  rdfs:label "total outgoing Energy" ;
  rdfs:comment """total outgoing Energy is the sum of the electric energy that leaves the system to the exterior."""@en ;
  rdfs:subPropertyOf seas:hasProperty ;
  rdfs:domain seas:PowerSystem ;
  rdfs:range seas:QuantifiableProperty ;
  vs:term_status "testing" ;
  rdfs:isDefinedBy seas:PowerSystemVocabulary .

seas:totalEnergyBalance a seas:PropertyKey, rdf:Property ;
  rdfs:label "total energy Balance" ;
  rdfs:comment """total energy Balance is equal to the sum of:
  The electric consumed energy minus the electric consumed production plus the electric stored energy.

  It is also equal to the sum of:
  The outgoing electric energy minus the incoming electric energy."""@en ;
  rdfs:subPropertyOf seas:hasProperty ;
  rdfs:domain seas:PowerSystem ;
  rdfs:range seas:QuantifiableProperty ;
  vs:term_status "testing" ;
  rdfs:isDefinedBy seas:PowerSystemVocabulary .

# code lists


# CL_FOURIER
seas:fourier a skos:ConceptScheme, sdmx:CodeList;
  rdfs:label "Fourier - codelist scheme"@en;
  skos:prefLabel "Fourier - codelist scheme"@en;
  skos:notation "CL_FOURIER";
  rdfs:comment """This code list enables to interpret the given value with respect to the Fourier-decomposition of the actual observed signal."""@en;
  skos:note """This code list enables to interpret the given value with respect to the Fourier-decomposition of the actual observed signal."""@en;
  skos:definition seas:fourier ;
  rdfs:seeAlso seas:Fourier ;
  vs:term_status "testing" ;
  rdfs:isDefinedBy seas:EvaluationInterpretationVocabulary .

seas:Fourier a rdfs:Class, owl:Class;
  rdfs:subClassOf skos:Concept ;
  rdfs:label "Fourier - codelist class"@en;
  rdfs:comment """This code list enables to interpret the given value with respect to the Fourier-decomposition of the actual observed signal."""@en;
  rdfs:seeAlso seas:fourier ;
  vs:term_status "testing" ;
  rdfs:isDefinedBy seas:EvaluationInterpretationVocabulary . 

seas:fourier-Frequency a skos:Concept, seas:EvaluationInterpretationConcept, seas:Fourier;
  rdfs:label "Frequency"@en ;
  skos:prefLabel "Frequency"@en ;
  skos:notation "Freq" ;
  rdfs:comment """Frequency means that the given value measures the frequency of the periodic signal."""@en ;
  skos:definition """Frequency means that the given value measures the frequency of the periodic signal."""@en ;
  skos:topConceptOf seas:fourier;
  skos:inScheme   seas:fourier;
  seas:dimension seas:frequency ;
  vs:term_status "testing" ;
  rdfs:isDefinedBy seas:EvaluationInterpretationVocabulary . 

seas:fourier skos:hasTopConcept seas:fourier-Frequency .

seas:fourier-peak a skos:Concept, seas:EvaluationInterpretationConcept, seas:Fourier;
  rdfs:label "Peak"@en ;
  skos:prefLabel "Peak"@en ;
  skos:notation "Peak" ;
  rdfs:comment """Peak means that the given value measures the Peak of the periodic signal."""@en ;
  skos:definition """Peak means that the given value measures the Peak of the periodic signal."""@en ;
  skos:topConceptOf seas:fourier;
  skos:inScheme   seas:fourier;
  vs:term_status "testing" ;
  rdfs:isDefinedBy seas:EvaluationInterpretationVocabulary . 

seas:fourier skos:hasTopConcept seas:fourier-peak .

seas:fourier-THD a skos:Concept, seas:EvaluationInterpretationConcept, seas:Fourier;
  rdfs:label "Total Harmonic Distortion"@en ;
  skos:prefLabel "Total Harmonic Distortion"@en ;
  skos:notation "THD" ;
  rdfs:comment """THD means that the given value measures the total harmonic distortion of the periodic signal."""@en ;
  skos:definition """THD means that the given value measures the total harmonic distortion of the periodic signal."""@en ;
  skos:topConceptOf seas:fourier;
  skos:inScheme   seas:fourier;
  vs:term_status "testing" ;
  rdfs:isDefinedBy seas:EvaluationInterpretationVocabulary . 

seas:fourier skos:hasTopConcept seas:fourier-THD .

seas:fourier-RMS a skos:Concept, seas:EvaluationInterpretationConcept, seas:Fourier;
  rdfs:label "RMS Amplitude"@en ;
  skos:prefLabel "RMS Amplitude"@en ;
  skos:notation "RMS" ;
  rdfs:comment """RMS means that the given value measures the Root Mean Square amplitude of the periodic signal."""@en ;
  skos:definition """RMS means that the given value measures the Root Mean Square amplitude of the periodic signal."""@en ;
  skos:topConceptOf seas:fourier;
  skos:inScheme   seas:fourier;
  seas:dimension seas:frequency ;
  vs:term_status "testing" ;
  rdfs:isDefinedBy seas:EvaluationInterpretationVocabulary . 

seas:fourier skos:hasTopConcept seas:fourier-RMS .

# CL_POWER
seas:power a skos:ConceptScheme, sdmx:CodeList;
  rdfs:label "Power - codelist scheme"@en;
  skos:prefLabel "Power - codelist scheme"@en;
  skos:notation "CL_POWER";
  rdfs:comment """This code list enables to interpret the given power value with respect to whether it is active or reactive."""@en;
  skos:note """This code list enables to interpret the given power value with respect to whether it is active or reactive."""@en;
  skos:definition seas:power ;
  rdfs:seeAlso seas:Power ;
  vs:term_status "testing" ;
  rdfs:isDefinedBy seas:EvaluationInterpretationVocabulary .

seas:Power a rdfs:Class, owl:Class;
  rdfs:subClassOf skos:Concept ;
  rdfs:label "Power - codelist class"@en;
  rdfs:comment """This code list enables to interpret the given power value."""@en;
  rdfs:seeAlso seas:power ;
  vs:term_status "testing" ;
  rdfs:isDefinedBy seas:EvaluationInterpretationVocabulary . 

seas:power-Active-Power a skos:Concept, seas:EvaluationInterpretationConcept, seas:Fourier;
  rdfs:label "Active Power"@en ;
  skos:prefLabel "Active Power"@en ;
  skos:notation "P" ;
  rdfs:comment """Active Power means that the given value measures the active power of the electric signal, in (W)."""@en ;
  skos:definition """Active Power means that the given value measures the active power of the electric signal, in (W)."""@en ;
  skos:topConceptOf seas:power;
  skos:inScheme   seas:power;
  seas:dimension seas:power ;
  vs:term_status "testing" ;
  rdfs:isDefinedBy seas:EvaluationInterpretationVocabulary . 

seas:power skos:hasTopConcept seas:power-Active-Power .

seas:power-Reactive-Power a skos:Concept, seas:EvaluationInterpretationConcept, seas:Fourier;
  rdfs:label "Reactive Power"@en ;
  skos:prefLabel "Reactive Power"@en ;
  skos:notation "Q" ;
  rdfs:comment """Reactive Power means that the given value measures the reactive power of the electric signal, in (var)."""@en ;
  skos:definition """Reactive Power means that the given value measures the reactive power of the electric signal, in (var)."""@en ;
  skos:topConceptOf seas:power;
  skos:inScheme   seas:power;
  seas:dimension seas:power ;
  vs:term_status "testing" ;
  rdfs:isDefinedBy seas:EvaluationInterpretationVocabulary . 

seas:power skos:hasTopConcept seas:power-Reactive-Power .

seas:power-Apparent-Power a skos:Concept, seas:EvaluationInterpretationConcept, seas:Fourier;
  rdfs:label "Apparent Power"@en ;
  skos:prefLabel "Apparent Power"@en ;
  skos:notation "S" ;
  rdfs:comment """Apparent Power means that the given value measures the apparent power of the electric signal, in (VA)."""@en ;
  skos:definition """Apparent Power means that the given value measures the apparent power of the electric signal, in (VA)."""@en ;
  skos:topConceptOf seas:power;
  skos:inScheme   seas:power;
  seas:dimension seas:power ;
  vs:term_status "testing" ;
  rdfs:isDefinedBy seas:EvaluationInterpretationVocabulary . 

seas:power skos:hasTopConcept seas:power-Apparent-Power .

seas:power-Power-Factor a skos:Concept, seas:EvaluationInterpretationConcept, seas:Fourier;
  rdfs:label "Power Factor"@en ;
  skos:prefLabel "Power Factor"@en ;
  skos:notation "cos phi" ;
  rdfs:comment """Power Factor means that the given value measures the cosinus of the voltage with respect to current, unitless."""@en ;
  skos:definition """Power Factor means that the given value measures the cosinus of the voltage with respect to current, unitless."""@en ;
  skos:topConceptOf seas:power;
  skos:inScheme   seas:power;
  seas:dimension seas:unitless ;
  vs:term_status "testing" ;
  rdfs:isDefinedBy seas:EvaluationInterpretationVocabulary . 

seas:power skos:hasTopConcept seas:power-Power-Factor .

seas:power-Imported-Active-Energy a skos:Concept, seas:EvaluationInterpretationConcept, seas:Fourier;
  rdfs:label "Imported Active Energy"@en ;
  skos:prefLabel "Imported Active Energy"@en ;
  skos:notation "ActEner" ;
  rdfs:comment """Imported Active Energy means that the given value measures the imported active energy, often in Wh/10."""@en ;
  skos:definition """Imported Active Energy means that the given value measures the imported active energy, often in Wh/10."""@en ;
  skos:topConceptOf seas:power;
  skos:inScheme   seas:power;
  seas:dimension seas:energy ;
  vs:term_status "testing" ;
  rdfs:isDefinedBy seas:EvaluationInterpretationVocabulary . 

seas:power skos:hasTopConcept seas:power-Imported-Active-Energy .
