# Copyright 2016 ITEA 12004 SEAS Project.
# 
# Licensed under the Apache License, Version 2.0 (the "License");
# you may not use this file except in compliance with the License.
# You may obtain a copy of the License at
# 
#      http://www.apache.org/licenses/LICENSE-2.0
# 
# Unless required by applicable law or agreed to in writing,
# distributed under the License is distributed on an "AS IS" BASIS,
# WITHOUT WARRANTIES OR CONDITIONS OF ANY KIND, either express or implied.
# See the License for the specific language governing permissions and
# limitations under the License.

@prefix rdf: <http://www.w3.org/1999/02/22-rdf-syntax-ns#> . #Resource data framework
@prefix owl: <http://www.w3.org/2002/07/owl#> .     #Owl ontology language
@prefix rdfs: <http://www.w3.org/2000/01/rdf-schema#> .   #RDF schema 
@prefix xsd: <http://www.w3.org/2001/XMLSchema#> .  #XML standard datatypes
@prefix dc: <http://purl.org/dc/terms/> .  #Dublin Core Metadata Initiative terms
@prefix vann: <http://purl.org/vocab/vann/> .  #A vocabulary for annotating vocabulary descriptions
@prefix voaf: <http://purl.org/vocommons/voaf#> . #A vocabulary of a friend, for describing relations between linked vocabularies
@prefix vs: <http://www.w3.org/2003/06/sw-vocab-status/ns#> . #Semantic web vocabulary status ontology
@prefix foaf: <http://xmlns.com/foaf/0.1/>.
@prefix ssn: <https://www.w3.org/ns/ssn/>.
@prefix cc: <http://creativecommons.org/ns#>.
@prefix dul: <http://www.ontologydesignpatterns.org/ont/dul/DUL.owl#>. # The DOLCE+DnS Ultralite ontology.
@prefix liner: <https://w3id.org/liner/>.
@prefix skos: <http://www.w3.org/2004/02/skos/core#>.
@prefix qb: <http://purl.org/linked-data/cube#>.
@prefix cdt: <http://w3id.org/lindt/custom_datatypes#>.

@prefix seas: <https://w3id.org/seas/>.
@base <https://w3id.org/seas/>.

seas:PowerGeneratorVocabulary a owl:Ontology , voaf:Vocabulary ;
  dc:title "seas-PowerGenerator vocabulary."@en ;
  dc:description """This vocabulary defines common properties of power generator systems."""@en ;
  dc:issued "2016-07-19"^^xsd:date ;
  dc:modified "2016-07-19"^^xsd:date ;
  dc:author <http://www.maxime-lefrancois.info/me#> ;
  dc:contributor <https://w3id.org/people/gabrieljlsantos#> ;
  dc:contributor <https://w3id.org/people/franciscosilva#> ;
  dc:contributor <https://w3id.org/people/brigidateixeira#> ;
  cc:license <http://creativecommons.org/licenses/by/4.0/> ;
  vann:preferredNamespacePrefix "seas" ;
  vann:preferredNamespaceUri <https://w3id.org/seas/> ;  
  owl:versionIRI <https://w3id.org/seas/PowerGeneratorVocabulary/0.10> ;
  owl:versionInfo "v0.10" .


############################
#     Generator Types      #
############################

seas:PhotovoltaicGenerator a owl:Class ;
  rdfs:subClassOf seas:PowerGenerator ;
  rdfs:label "Photovoltaic Generator"@en ;
  rdfs:comment """The class of generators which type of energy transformation is based on photovoltaic panel."""@en ;
  vs:term_status "testing" ;
  rdfs:isDefinedBy seas:PhotovoltaicGenerator .

seas:WindGenerator a owl:Class ;
  rdfs:subClassOf seas:PowerGenerator ;
  rdfs:label "Wind Generator"@en ;
  rdfs:comment """The class of generators which type of energy transformation is based on wind."""@en ;
  vs:term_status "testing" ;
  rdfs:isDefinedBy seas:WindGenerator .

seas:CoGenerator a owl:Class ;
  rdfs:subClassOf seas:PowerGenerator ;
  rdfs:label "Cogenerator"@en ;
  rdfs:comment """The class of generators which has two types of energy transformation, usually electrical energy and heat."""@en ;
  vs:term_status "testing" ;
  rdfs:isDefinedBy seas:CoGenerator .

seas:BiomassGenerator a owl:Class ;
  rdfs:subClassOf seas:PowerGenerator ;
  rdfs:label "Biomass Generator"@en ;
  rdfs:comment """The class of generators which type of energy is based on Biomass."""@en ;
  vs:term_status "testing" ;
  rdfs:isDefinedBy seas:BiomassGenerator .

seas:WasteToEnergyGenerator a owl:Class ;
  rdfs:subClassOf seas:PowerGenerator ;
  rdfs:label "Waste-to-Energy Generator"@en ;
  rdfs:comment """The class of generators which form of energy transformation is based on waste-to-energy method, that is the process of generating energy in the form of electricity and/or heat from the primary treatment of waste"""@en ;
  vs:term_status "testing" ;
  rdfs:isDefinedBy seas:WasteToEnergyGenerator .

seas:SmallHydroGenerator a owl:Class ;
  rdfs:subClassOf seas:PowerGenerator ;
  rdfs:label "Small Hydro Generator"@en ;
  rdfs:comment """The class of generators which form of energy transformation is based on a small hydro."""@en ;
  vs:term_status "testing" ;
  rdfs:isDefinedBy seas:SmallHydroGenerator .

seas:FuelCellGenerator a owl:Class ;
  rdfs:subClassOf seas:PowerGenerator ;
  rdfs:label "Fuel Cell Generator"@en ;
  rdfs:comment """The class of generators which form of energy transformation is based on a fuel cell"""@en ;
  vs:term_status "testing" ;
  rdfs:isDefinedBy seas:FuelCellGenerator .

############################
#     Properties     #
############################

seas:installedActivePower a seas:PropertyKey, rdf:Property ;
  rdfs:label "Installed active power" ;
  rdfs:comment """The power that is used to do work on the load"""@en ;
  rdfs:subPropertyOf seas:hasProperty ;
  rdfs:domain seas:PowerGenerator ;
  rdfs:range seas:PowerProperty ;
  vs:term_status "testing" ;
  rdfs:isDefinedBy seas:PowerGeneratorVocabulary .

seas:installedActivePower a seas:PropertyKey, rdf:Property ;
  rdfs:label "Installed active power" ;
  rdfs:comment """The average value over time of the instantaneous power of alternating current."""@en ;
  rdfs:subPropertyOf seas:hasProperty ;
  rdfs:domain seas:PowerGenerator ;
  rdfs:range seas:PowerProperty ;
  vs:term_status "testing" ;
  rdfs:isDefinedBy seas:PowerGeneratorVocabulary .

seas:installedApparentPower a seas:PropertyKey, rdf:Property ;
  rdfs:label "Installed apparent power" ;
  rdfs:comment """The quantity that is equal to the product of the effective values of the periodic electric current I in a circuit and of the voltage U across the terminals of the circuit: S = UI."""@en ;
  rdfs:subPropertyOf seas:hasProperty ;
  rdfs:domain seas:PowerGenerator ;
  rdfs:range seas:PowerProperty ;
  vs:term_status "testing" ;
  rdfs:isDefinedBy seas:PowerGeneratorVocabulary .

seas:contractPreviousStatus a seas:PropertyKey, rdf:Property ;
  rdfs:label "Contract previous status" ;
  rdfs:comment """The Generator status (turn on or off) in the beginning of the scheduling."""@en ;
  rdfs:subPropertyOf seas:hasProperty ;
  rdfs:domain seas:PowerGenerator ;
  rdfs:range seas:Property ;
  vs:term_status "testing" ;
  rdfs:isDefinedBy seas:PowerGeneratorVocabulary .

seas:contractPreviousPower a seas:PropertyKey, rdf:Property ;
  rdfs:label "Contract previous power" ;
  rdfs:comment """The scheduled power to the generator in the beginning of the scheduling."""@en ;
  rdfs:subPropertyOf seas:hasProperty ;
  rdfs:domain seas:PowerGenerator ;
  rdfs:range seas:PowerProperty ;
  vs:term_status "testing" ;
  rdfs:isDefinedBy seas:PowerGeneratorVocabulary .

seas:contractGradient a seas:PropertyKey, rdf:Property ;
  rdfs:label "Contract gradient" ;
  rdfs:comment """The Maximum power variation (gradient) to be scheduled for the generator."""@en ;
  rdfs:subPropertyOf seas:hasProperty ;
  rdfs:domain seas:PowerGenerator ;
  rdfs:range seas:PowerProperty ;
  vs:term_status "testing" ;
  rdfs:isDefinedBy seas:PowerGeneratorVocabulary .

seas:contractMinSheduledEnergy a seas:PropertyKey, rdf:Property ;
  rdfs:label "Contract minimum energy" ;
  rdfs:comment """The minimum of energy that must be scheduled to the generator."""@en ;
  rdfs:subPropertyOf seas:hasProperty ;
  rdfs:domain seas:PowerGenerator ;
  rdfs:range seas:EnergyProperty ;
  vs:term_status "testing" ;
  rdfs:isDefinedBy seas:PowerGeneratorVocabulary .

seas:contractMinRemuneration a seas:PropertyKey, rdf:Property ;
  rdfs:label "Contract minimum renumeration" ;
  rdfs:comment """The minimum remuneration that generator must receive during the scheduling."""@en ;
  rdfs:subPropertyOf seas:hasProperty ;
  rdfs:domain seas:PowerGenerator ;
  rdfs:range seas:MonetaryProperty ;
  vs:term_status "testing" ;
  rdfs:isDefinedBy seas:PowerGeneratorVocabulary .

seas:contractMinWorkingPeriods a seas:PropertyKey, rdf:Property ;
  rdfs:label "Contract minimum working periods" ;
  rdfs:comment """The minimum of periods that generator must be scheduled."""@en ;
  rdfs:subPropertyOf seas:hasProperty ;
  rdfs:domain seas:PowerGenerator ;
  rdfs:range seas:PeriodProperty ;
  vs:term_status "testing" ;
  rdfs:isDefinedBy seas:PowerGeneratorVocabulary .

seas:contractMaxEntriesInService a seas:PropertyKey, rdf:Property ;
  rdfs:label "Contract maximum service entries" ;
  rdfs:comment """The Number of times that generator can enter on service."""@en ;
  rdfs:subPropertyOf seas:hasProperty ;
  rdfs:domain seas:PowerGenerator ;
  rdfs:range seas:Property ;
  vs:term_status "testing" ;
  rdfs:isDefinedBy seas:PowerGeneratorVocabulary .

seas:contractMinConsecutivePeriodsInOperation a seas:PropertyKey, rdf:Property ;  # replace by two concepts: min/max, and one in CL_CONTRACT
  rdfs:label "Contract minimum consecutive periods in operation" ;
  rdfs:comment """The Minimum number of consecutive periods that generator is producing."""@en ;
  rdfs:subPropertyOf seas:hasProperty ;
  rdfs:domain seas:PowerGenerator ;
  rdfs:range seas:PeriodProperty ;
  vs:term_status "testing" ;
  rdfs:isDefinedBy seas:PowerGeneratorVocabulary .

seas:contractMinConsecutivePeriodsInOperation a seas:PropertyKey, rdf:Property ;
  rdfs:label "Contract minimum consecutive periods in operation" ;
  rdfs:comment """The Minimum number of consecutive periods that generator is producing."""@en ;
  rdfs:subPropertyOf seas:hasProperty ;
  rdfs:domain seas:PowerGenerator ;
  rdfs:range seas:PeriodProperty ;
  vs:term_status "testing" ;
  rdfs:isDefinedBy seas:PowerGeneratorVocabulary .

seas:rampUp a seas:PropertyKey, rdf:Property ; # replace by a concept in CL_OPERATING 
  rdfs:label "Ramp up" ;
  rdfs:comment """The maximum active power to increase during ramp turn up."""@en ;
  rdfs:subPropertyOf seas:hasProperty ;
  rdfs:domain seas:PowerGenerator ;
  rdfs:range seas:PowerProperty ;
  vs:term_status "testing" ;
  rdfs:isDefinedBy seas:PowerGeneratorVocabulary .

seas:rampDown a seas:PropertyKey, rdf:Property ; # replace by a concept in CL_OPERATING
  rdfs:label "Ramp down" ;
  rdfs:comment """The Maximum active power to reduce during ramp turn down."""@en ;
  rdfs:subPropertyOf seas:hasProperty ;
  rdfs:domain seas:PowerGenerator ;
  rdfs:range seas:PowerProperty ;
  vs:term_status "testing" ;
  rdfs:isDefinedBy seas:PowerGeneratorVocabulary .

seas:overloadTime a seas:PropertyKey, rdf:Property ; # replace by a concept in CL_OPERATING
  rdfs:label "Overload time" ;
  rdfs:comment """The generator Overload maximum time."""@en ;
  rdfs:subPropertyOf seas:hasProperty ;
  rdfs:domain seas:PowerGenerator ;
  rdfs:range seas:TimeProperty ;
  vs:term_status "testing" ;
  rdfs:isDefinedBy seas:PowerGeneratorVocabulary .

seas:overloadPower a seas:PropertyKey, rdf:Property ; # replace by a concept in CL_OPERATING
  rdfs:label "Overload power" ;
  rdfs:comment """The generator overload power."""@en ;
  rdfs:subPropertyOf seas:hasProperty ;
  rdfs:domain seas:PowerGenerator ;
  rdfs:range seas:PowerProperty ;
  vs:term_status "testing" ;
  rdfs:isDefinedBy seas:PowerGeneratorVocabulary .

seas:generatorType a seas:PropertyKey, rdf:Property ;
  rdfs:label "Overload power" ;
  rdfs:comment """if operator must buy all the generated energy or if the operator can buy if wanted, between minimum power and maximum power"""@en ;
  rdfs:subPropertyOf seas:hasProperty ;
  rdfs:domain seas:PowerGenerator ;
  rdfs:range seas:IntegerProperty ;
  vs:term_status "testing" ;
  rdfs:isDefinedBy seas:PowerGeneratorVocabulary .

seas:CofA a seas:PropertyKey, rdf:Property ;
  rdfs:label "Fixed Coefficient" ;
  rdfs:comment """Coefficient A (fixed) of the generation cost."""@en ;
  rdfs:subPropertyOf seas:hasProperty ;
  rdfs:domain seas:PowerGenerator ;
  rdfs:range seas:MonetaryProperty ;
  vs:term_status "testing" ;
  rdfs:isDefinedBy seas:PowerGeneratorVocabulary .

seas:CofB a seas:PropertyKey, rdf:Property ;
  rdfs:label "Linear Coefficient" ;
  rdfs:comment """Coefficient B (linear) of the generation cost."""@en ;
  rdfs:subPropertyOf seas:hasProperty ;
  rdfs:domain seas:PowerGenerator ;
  rdfs:range seas:MonetaryProperty ;
  vs:term_status "testing" ;
  rdfs:isDefinedBy seas:PowerGeneratorVocabulary .

seas:CofC a seas:PropertyKey, rdf:Property ;
  rdfs:label "Quadratic Coefficient" ;
  rdfs:comment """Coefficient C (quadratic) of the generation cost."""@en ;
  rdfs:subPropertyOf seas:hasProperty ;
  rdfs:domain seas:PowerGenerator ;
  rdfs:range seas:MonetaryProperty ;
  vs:term_status "testing" ;
  rdfs:isDefinedBy seas:PowerGeneratorVocabulary .

seas:cofExcess a seas:PropertyKey, rdf:Property ;
  rdfs:label "Coefficient excess" ;
  rdfs:comment """The generator overload power."""@en ;
  rdfs:subPropertyOf seas:hasProperty ;
  rdfs:domain seas:PowerGenerator ;
  rdfs:range seas:MonetaryProperty ;
  vs:term_status "testing" ;
  rdfs:isDefinedBy seas:PowerGeneratorVocabulary .

seas:geeeCofA a seas:PropertyKey, rdf:Property ;
  rdfs:label "GEEE Coefficient A" ;
  rdfs:comment """Fixed coefficient to excess generation."""@en ;
  rdfs:subPropertyOf seas:hasProperty ;
  rdfs:domain seas:PowerGenerator ;
  rdfs:range seas:MonetaryProperty ;
  vs:term_status "testing" ;
  rdfs:isDefinedBy seas:PowerGeneratorVocabulary .
  
seas:geeeCofB a seas:PropertyKey, rdf:Property ;
  rdfs:label "GEEE Coefficient B" ;
  rdfs:comment """Linear coefficient of the greenhouse gas emissions cost."""@en ;
  rdfs:subPropertyOf seas:hasProperty ;
  rdfs:domain seas:PowerGenerator ;
  rdfs:range seas:MonetaryProperty ;
  vs:term_status "testing" ;
  rdfs:isDefinedBy seas:PowerGeneratorVocabulary .

seas:geeeCofC a seas:PropertyKey, rdf:Property ;
  rdfs:label "GEEE Coefficient C" ;
  rdfs:comment """Quadratic coefficient of the greenhouse gas emissions cost."""@en ;
  rdfs:subPropertyOf seas:hasProperty ;
  rdfs:domain seas:PowerGenerator ;
  rdfs:range seas:MonetaryProperty ;
  vs:term_status "testing" ;
  rdfs:isDefinedBy seas:PowerGeneratorVocabulary .

seas:geeeCofC a seas:PropertyKey, rdf:Property ;
  rdfs:label "GEEE Coefficient C" ;
  rdfs:comment """Quadratic coefficient of the greenhouse gas emissions cost."""@en ;
  rdfs:subPropertyOf seas:hasProperty ;
  rdfs:domain seas:PowerGenerator ;
  rdfs:range seas:MonetaryProperty ;
  vs:term_status "testing" ;
  rdfs:isDefinedBy seas:PowerGeneratorVocabulary .

seas:rdPower a seas:PropertyKey, rdf:Property ;
  rdfs:label "Regulated down power" ;
  rdfs:comment """Regulated down power."""@en ;
  rdfs:subPropertyOf seas:hasProperty ;
  rdfs:domain seas:PowerGenerator ;
  rdfs:range seas:PowerProperty ;
  vs:term_status "testing" ;
  rdfs:isDefinedBy seas:PowerGeneratorVocabulary .

seas:ruPower a seas:PropertyKey, rdf:Property ;
  rdfs:label "Regulated up power" ;
  rdfs:comment """Regulated up power."""@en ;
  rdfs:subPropertyOf seas:hasProperty ;
  rdfs:domain seas:PowerGenerator ;
  rdfs:range seas:PowerProperty ;
  vs:term_status "testing" ;
  rdfs:isDefinedBy seas:PowerGeneratorVocabulary .

seas:spPower a seas:PropertyKey, rdf:Property ;
  rdfs:label "Spinning reserve power" ;
  rdfs:comment """Spinning reserve power."""@en ;
  rdfs:subPropertyOf seas:hasProperty ;
  rdfs:domain seas:PowerGenerator ;
  rdfs:range seas:PowerProperty ;
  vs:term_status "testing" ;
  rdfs:isDefinedBy seas:PowerGeneratorVocabulary .

seas:nspPower a seas:PropertyKey, rdf:Property ;
  rdfs:label "Non spinning reserve power" ;
  rdfs:comment """Non-spinning reserve power."""@en ;
  rdfs:subPropertyOf seas:hasProperty ;
  rdfs:domain seas:PowerGenerator ;
  rdfs:range seas:PowerProperty ;
  vs:term_status "testing" ;
  rdfs:isDefinedBy seas:PowerGeneratorVocabulary .

seas:rdAvailableCost a seas:PropertyKey, rdf:Property ;
  rdfs:label "RD available cost" ;
  rdfs:comment """Available cost of regulation down."""@en ;
  rdfs:subPropertyOf seas:hasProperty ;
  rdfs:domain seas:PowerGenerator ;
  rdfs:range seas:MonetaryProperty ;
  vs:term_status "testing" ;
  rdfs:isDefinedBy seas:PowerGeneratorVocabulary .

seas:ruAvailableCost a seas:PropertyKey, rdf:Property ;
  rdfs:label "RU available cost" ;
  rdfs:comment """Available cost of regulation up."""@en ;
  rdfs:subPropertyOf seas:hasProperty ;
  rdfs:domain seas:PowerGenerator ;
  rdfs:range seas:MonetaryProperty ;
  vs:term_status "testing" ;
  rdfs:isDefinedBy seas:PowerGeneratorVocabulary .

seas:spAvailableCost a seas:PropertyKey, rdf:Property ;
  rdfs:label "Spinning available cost" ;
  rdfs:comment """Available cost of spinning reserve."""@en ;
  rdfs:subPropertyOf seas:hasProperty ;
  rdfs:domain seas:PowerGenerator ;
  rdfs:range seas:MonetaryProperty ;
  vs:term_status "testing" ;
  rdfs:isDefinedBy seas:PowerGeneratorVocabulary .

seas:nspAvailableCost a seas:PropertyKey, rdf:Property ;
  rdfs:label "Non-spinning available cost" ;
  rdfs:comment """Available cost of non-spinning reserve."""@en ;
  rdfs:subPropertyOf seas:hasProperty ;
  rdfs:domain seas:PowerGenerator ;
  rdfs:range seas:MonetaryProperty ;
  vs:term_status "testing" ;
  rdfs:isDefinedBy seas:PowerGeneratorVocabulary .

seas:rdEnergyCost a seas:PropertyKey, rdf:Property ;
  rdfs:label "RD energy cost" ;
  rdfs:comment """Energy cost of regulation down."""@en ;
  rdfs:subPropertyOf seas:hasProperty ;
  rdfs:domain seas:PowerGenerator ;
  rdfs:range seas:MonetaryProperty ;
  vs:term_status "testing" ;
  rdfs:isDefinedBy seas:PowerGeneratorVocabulary .

seas:ruEnergyCost a seas:PropertyKey, rdf:Property ;
  rdfs:label "RU energy cost" ;
  rdfs:comment """Energy cost of regulation up."""@en ;
  rdfs:subPropertyOf seas:hasProperty ;
  rdfs:domain seas:PowerGenerator ;
  rdfs:range seas:MonetaryProperty ;
  vs:term_status "testing" ;
  rdfs:isDefinedBy seas:PowerGeneratorVocabulary .

seas:spEnergyCost a seas:PropertyKey, rdf:Property ;
  rdfs:label "Spinning energy cof" ;
  rdfs:comment """Energy cost of spinning reserve."""@en ;
  rdfs:subPropertyOf seas:hasProperty ;
  rdfs:domain seas:PowerGenerator ;
  rdfs:range seas:MonetaryProperty ;
  vs:term_status "testing" ;
  rdfs:isDefinedBy seas:PowerGeneratorVocabulary .

seas:nspEnergyCost a seas:PropertyKey, rdf:Property ;
  rdfs:label "Non-spinning energy cost" ;
  rdfs:comment """Energy cost of non-spinning reserve."""@en ;
  rdfs:subPropertyOf seas:hasProperty ;
  rdfs:domain seas:PowerGenerator ;
  rdfs:range seas:MonetaryProperty ;
  vs:term_status "testing" ;
  rdfs:isDefinedBy seas:PowerGeneratorVocabulary .

# todo: replace all the different cost properties by just seas:cost, and add a list of interpretation concepts 
