# Copyright 2016 ITEA 12004 SEAS Project.
# 
# Licensed under the Apache License, Version 2.0 (the "License");
# you may not use this file except in compliance with the License.
# You may obtain a copy of the License at
# 
#      http://www.apache.org/licenses/LICENSE-2.0
# 
# Unless required by applicable law or agreed to in writing,
# distributed under the License is distributed on an "AS IS" BASIS,
# WITHOUT WARRANTIES OR CONDITIONS OF ANY KIND, either express or implied.
# See the License for the specific language governing permissions and
# limitations under the License.

@prefix rdf: <http://www.w3.org/1999/02/22-rdf-syntax-ns#> . #Resource data framework
@prefix owl: <http://www.w3.org/2002/07/owl#> .              #Owl ontology language
@prefix rdfs: <http://www.w3.org/2000/01/rdf-schema#> .      #RDF schema 
@prefix xsd: <http://www.w3.org/2001/XMLSchema#> .           #XML standard datatypes
@prefix dc: <http://purl.org/dc/terms/> .     #Dublin Core Metadata Initiative terms
@prefix vann: <http://purl.org/vocab/vann/> .  #A vocabulary for annotating vocabulary descriptions
@prefix voaf: <http://purl.org/vocommons/voaf#> . #A vocabulary of a friend, for describing relations between linked vocabularies
@prefix vs: <http://www.w3.org/2003/06/sw-vocab-status/ns#> . #Semantic web vocabulary status ontology
@prefix foaf: <http://xmlns.com/foaf/0.1/>.
@prefix saref: <http://ontology.tno.nl/saref#>. #SAREF smart building appliances ontology
@prefix qudt: <http://data.qudt.org/qudt/owl/1.0.0/qudt.owl#> . #QUDT quantities
@prefix qudt-unit: <http://data.qudt.org/qudt/owl/1.0.0/unit.owl#> . #QUDT units

@prefix seas: <https://w3id.org/seas/>.
@base <https://w3id.org/seas/>.

seas:ElectricityPlayerVocabulary rdf:type voaf:Vocabulary , owl:Ontology ;
  dc:title "seas vocabulary"@en ;
  dc:description """The Seas Electricity Player Vocabulary defined for the ITEA SEAS (Smart Energy Aware Systems)
   project."""@en ;
  dc:issued "2016-07-22"^^xsd:date ;
  dc:modified "2016-07-22"^^xsd:date ;
  dc:contributor <http://www.maxime-lefrancois.info/me#> ;
  dc:author <https://w3id.org/people/gabrieljlsantos#> ;
  dc:contributor <https://w3id.org/people/franciscosilva#> ;
  dc:contributor <https://w3id.org/people/brigidateixeira#> ;
  vann:preferredNamespacePrefix "seas" ;
  vann:preferredNamespaceUri <https://w3id.org/seas/> ;  
  owl:versionIRI <https://w3id.org/seas/ElectricityPlayerVocabulary/0.10> ;
  owl:versionInfo "v0.10" .

seas:powerExchange a seas:PropertyKey, rdf:Property ;
  rdfs:label "power Exchange" ;
  rdfs:comment """power Exchange is the power exchanged in a electricity market."""@en ;
  rdfs:subPropertyOf seas:hasProperty ;
  rdfs:domain seas:ElectricityExchangeConnection ;
  rdfs:range seas:Property ;
  vs:term_status "testing" ;
  rdfs:isDefinedBy seas:ElectricityPlayerVocabulary .

seas:powerPriceContext a owl:ObjectProperty ;
  rdfs:label "power Price context"@en ;
  rdfs:comment """Links an evaluation to the power price context on which it is defined.
  for instance: 

   [] a seas:Evaluation ;
	seas:interpretedAs seas:sell ;
	seas:temporalContext [ a owl:Interval ... ] ;
	seas:literalValue "200 MWh"^^xsd:ucum ;
	seas:powerPriceContext "12 â‚¬/MWh"^^xsd:ucum . """@en ;
  rdfs:subPropertyOf seas:context ;
  rdfs:domain seas:Evaluation ;
  rdfs:range seas:ElectricityPrice ;
  vs:term_status "testing" ;
  rdfs:isDefinedBy seas:ElectricityPlayerVocabulary .



# code lists

#Bid Code List
seas:bid a skos:ConceptScheme, sdmx:CodeList;
  rdfs:label "Bid - codelist scheme"@en;
  skos:prefLabel "Bid - codelist scheme"@en;
  skos:notation "CL_BID";
  rdfs:comment """This code list enables to interpret the given value with respect to the Electricity Markets Bids."""@en;
  skos:note """This code list enables to interpret the given value with respect to the Electricity Markets Bids."""@en;
  skos:definition seas:bid ;
  rdfs:seeAlso seas:Bid ;
  vs:term_status "testing" ;
  rdfs:isDefinedBy seas:ElectricityPlayerVocabulary .

seas:Bid a rdfs:Class, owl:Class;
  rdfs:subClassOf skos:Concept ;
  rdfs:label "Bid - codelist class"@en;
  rdfs:comment """This code list enables to interpret the given value with respect to the Electricity Markets Bids."""@en;
  rdfs:seeAlso seas:bid ;
  vs:term_status "testing" ;
  rdfs:isDefinedBy seas:ElectricityPlayerVocabulary . 

#seas:bid-Bid a skos:Concept, seas:EvaluationInterpretationConcept, seas:Bid;
#  rdfs:label "Bid"@en ;
#  skos:prefLabel "Bid"@en ;
#  skos:notation "Bid" ;
#  rdfs:comment """The Bid is a pair of amount of power with a given price per unit."""@en ;
#  skos:definition """The Bid is a pair of amount of power with a given price per unit."""@en ;
#  skos:topConceptOf seas:bid;
#  skos:inScheme   seas:bid;
#  vs:term_status "testing" ;
#  rdfs:isDefinedBy seas:ElectricityPlayerVocabulary . 
#
#seas:bid skos:hasTopConcept seas:bid-Bid .

seas:bid-SellBid a skos:Concept, seas:EvaluationInterpretationConcept, seas:Bid;
  rdfs:label "Sell Bid"@en ;
  skos:prefLabel "Sell Bid"@en ;
  skos:notation "Sell Bid" ;
  rdfs:comment """A Sell Bid is a bid to sell in the Electricity Market. A Bid is a pair of amount of power with a given price per unit."""@en ;
  skos:definition """A Sell Bid is a bid to sell in the Electricity Market. A Bid is a pair of amount of power with a given price per unit."""@en ;
  skos:topConceptOf seas:bid;
  skos:inScheme   seas:bid;
  vs:term_status "testing" ;
  rdfs:isDefinedBy seas:ElectricityPlayerVocabulary . 

seas:bid skos:hasTopConcept seas:bid-SellBid .

seas:bid-BuyBid a skos:Concept, seas:EvaluationInterpretationConcept, seas:Bid;
  rdfs:label "Buy Bid"@en ;
  skos:prefLabel "Buy Bid"@en ;
  skos:notation "Buy Bid" ;
  rdfs:comment """A Buy Bid is a bid to buy in the Electricity Market. A Bid is a pair of amount of power with a given price per unit."""@en ;
  skos:definition """A Buy Bid is a bid to buy in the Electricity Market. A Bid is a pair of amount of power with a given price per unit."""@en ;
  skos:topConceptOf seas:bid;
  skos:inScheme   seas:bid;
  vs:term_status "testing" ;
  rdfs:isDefinedBy seas:ElectricityPlayerVocabulary . 

seas:bid skos:hasTopConcept seas:bid-BuyBid .


#Flexibility Code List
seas:flexibility a skos:ConceptScheme, sdmx:CodeList;
  rdfs:label "Flexibility - codelist scheme"@en;
  skos:prefLabel "Flexibility - codelist scheme"@en;
  skos:notation "CL_FLEXIBILITY";
  rdfs:comment """This code list enables to interpret the given value with respect to the consumption, production and Demand Response Flexibility."""@en;
  skos:note """This code list enables to interpret the given value with respect to the consumption, production and Demand Response Flexibility."""@en;
  skos:definition seas:flexibility ;
  rdfs:seeAlso seas:Flexibility ;
  vs:term_status "testing" ;
  rdfs:isDefinedBy seas:ElectricityPlayerVocabulary .

seas:Flexibility a rdfs:Class, owl:Class;
  rdfs:subClassOf skos:Concept ;
  rdfs:label "Flexibility - codelist class"@en;
  rdfs:comment """This code list enables to interpret the given value with respect to the consumption, production and Demand Response Flexibility."""@en;
  rdfs:seeAlso seas:flexibility ;
  vs:term_status "testing" ;
  rdfs:isDefinedBy seas:ElectricityPlayerVocabulary . 

seas:flexibility-Up a skos:Concept, seas:EvaluationInterpretationConcept, seas:Flexibility;
  rdfs:label "Flexibility Up"@en ;
  skos:prefLabel "Flexibility Up"@en ;
  skos:notation "Flexibility Up" ;
  rdfs:comment """The "Flexibility Up" is the ability to increase the consumption / production of energy."""@en ;
  skos:definition """The "Flexibility Up" is the ability to increase the consumption / production of energy."""@en ;
  skos:topConceptOf seas:flexibility;
  skos:inScheme   seas:flexibility;
  vs:term_status "testing" ;
  rdfs:isDefinedBy seas:ElectricityPlayerVocabulary . 

seas:flexibility skos:hasTopConcept seas:flexibility-Up .

seas:flexibility-Down a skos:Concept, seas:EvaluationInterpretationConcept, seas:Flexibility;
  rdfs:label "Flexibility Down"@en ;
  skos:prefLabel "Flexibility Down"@en ;
  skos:notation "Flexibility Down" ;
  rdfs:comment """The "Flexibility Down" is the ability to decrease the consumption / production of energy."""@en ;
  skos:definition """The "Flexibility Down" is the ability to decrease the consumption / production of energy."""@en ;
  skos:topConceptOf seas:flexibility;
  skos:inScheme   seas:flexibility;
  vs:term_status "testing" ;
  rdfs:isDefinedBy seas:ElectricityPlayerVocabulary . 

seas:flexibility skos:hasTopConcept seas:flexibility-Down .


seas:flexibility-Increase a skos:Concept, seas:EvaluationInterpretationConcept, seas:Flexibility;
  rdfs:label "Increase"@en ;
  skos:prefLabel "Increase"@en ;
  skos:notation "Increase" ;
  rdfs:comment """The "Increase" is the ability to increase the consumption / production of energy."""@en ;
  skos:definition """The "Increase" is the ability to increase the consumption / production of energy."""@en ;
  skos:topConceptOf seas:flexibility;
  skos:inScheme   seas:flexibility;
  vs:term_status "testing" ;
  rdfs:isDefinedBy seas:ElectricityPlayerVocabulary . 

seas:flexibility skos:hasTopConcept seas:flexibility-Increase .

seas:flexibility-Cut a skos:Concept, seas:EvaluationInterpretationConcept, seas:Flexibility;
  rdfs:label "Curtailment"@en ;
  skos:prefLabel "Curtailment"@en ;
  skos:notation "Curtailment" ;
  rdfs:comment """The "Curtailment" is the ability to decrease the consumption / production of energy."""@en ;
  skos:definition """The "Curtailment" is the ability to decrease the consumption / production of energy."""@en ;
  skos:topConceptOf seas:flexibility;
  skos:inScheme   seas:flexibility;
  vs:term_status "testing" ;
  rdfs:isDefinedBy seas:ElectricityPlayerVocabulary . 

seas:flexibility skos:hasTopConcept seas:flexibility-Cut .

seas:flexibility-Shift a skos:Concept, seas:EvaluationInterpretationConcept, seas:Flexibility;
  rdfs:label "Shift"@en ;
  skos:prefLabel "Shift"@en ;
  skos:notation "Shift" ;
  rdfs:comment """The "Shift" is the ability to move the power from one place to another."""@en ;
  skos:definition """The "Shift" is the ability to move the power from one place to another."""@en ;
  skos:topConceptOf seas:flexibility;
  skos:inScheme   seas:flexibility;
  vs:term_status "testing" ;
  rdfs:isDefinedBy seas:ElectricityPlayerVocabulary . 

seas:flexibility skos:hasTopConcept seas:flexibility-Shift .
