# Copyright 2016 ITEA 12004 SEAS Project.
# 
# Licensed under the Apache License, Version 2.0 (the "License");
# you may not use this file except in compliance with the License.
# You may obtain a copy of the License at
# 
#      http://www.apache.org/licenses/LICENSE-2.0
# 
# Unless required by applicable law or agreed to in writing,
# distributed under the License is distributed on an "AS IS" BASIS,
# WITHOUT WARRANTIES OR CONDITIONS OF ANY KIND, either express or implied.
# See the License for the specific language governing permissions and
# limitations under the License.

@prefix rdf: <http://www.w3.org/1999/02/22-rdf-syntax-ns#> .
@prefix owl: <http://www.w3.org/2002/07/owl#> .
@prefix rdfs: <http://www.w3.org/2000/01/rdf-schema#> .
@prefix xsd: <http://www.w3.org/2001/XMLSchema#> .
@prefix dcterms: <http://purl.org/dc/terms/> .  
@prefix vann: <http://purl.org/vocab/vann/> .
@prefix voaf: <http://purl.org/vocommons/voaf#> .
@prefix vs: <http://www.w3.org/2003/06/sw-vocab-status/ns#> .
@prefix foaf: <http://xmlns.com/foaf/0.1/>.
@prefix ssn: <https://www.w3.org/ns/ssn/>.
@prefix dul: <http://www.ontologydesignpatterns.org/ont/dul/DUL.owl#>.
@prefix liner: <https://w3id.org/liner/>.
@prefix skos: <http://www.w3.org/2004/02/skos/core#>.
@prefix qb: <http://purl.org/linked-data/cube#>.
@prefix cdt: <http://w3id.org/lindt/custom_datatypes#>.
@prefix pep: <https://w3id.org/pep/> .
@prefix schema: <https://schema.org/>.
@prefix gr: <http://purl.org/goodrelations/v1#>.

@prefix seas: <https://w3id.org/seas/>.
@base <https://w3id.org/seas/>.

voaf:Vocabulary a owl:Class .
dcterms:title a owl:AnnotationProperty .
dcterms:description a owl:AnnotationProperty .
dcterms:issued a owl:AnnotationProperty .
dcterms:modified a owl:AnnotationProperty .
dcterms:creator a owl:AnnotationProperty .
dcterms:contributor a owl:AnnotationProperty .
dcterms:license a owl:AnnotationProperty .
vann:preferredNamespacePrefix a owl:AnnotationProperty .
vann:preferredNamespaceUri a owl:AnnotationProperty .
vs:term_status a owl:AnnotationProperty .
foaf:Person a owl:Class .
foaf:name a owl:DatatypeProperty .



seas:ElectricLightingSystemOntology a owl:Ontology , voaf:Vocabulary ;
  dcterms:title "The SEAS Electric Street Light System Ontology."@en ;
  dcterms:description """The SEAS Electric Street Light System ontology describes Electric Street Light System."""@en ;
  dcterms:issued "2017-05-30"^^xsd:date ;
  dcterms:modified "2017-05-30"^^xsd:date ;
  dcterms:creator [  a foaf:Person; foaf:name "Lynda TEMAL"] ;
  dcterms:contributor <http://www.maxime-lefrancois.info/me#> ;
  dcterms:license <https://www.apache.org/licenses/LICENSE-2.0> ;
  vann:preferredNamespacePrefix "seas" ;
  vann:preferredNamespaceUri <https://w3id.org/seas/> ;  
  owl:imports seas:ZoneLightingOntology , 
              seas:ElectricPowerSystemOntology, 
              seas:ElectricLightSourceOntology , 
              seas:GenericPropertyOntology, 
              seas:BuildingOntology,
              seas:BooleanPropertyOntology, 
              seas:BatteryOntology,
              seas:DeviceOntology,
              seas:PhotovoltaicOntology,
              seas:EvaluationOntology,
              seas:BooleanPropertyOntology;
  owl:versionIRI <https://w3id.org/seas/ElectricStreetLightingSystemOntology-1.0> ;
  owl:versionInfo "v1.0" .



## Lighting, ElectricLightFixtureSystem, LightingExecution

seas:Lighting a owl:Class;
  rdfs:label "Lighting"@en ;
  rdfs:comment """Lighting is the process that allows to illuminate some zone."""@en ;
  rdfs:subClassOf seas:Actuating ;
  vs:term_status "testing" ;
  rdfs:isDefinedBy seas:ElectricStreetLightingSystemOntology .

# les luminaire peuvent avoir plusieurs fonctions parmi elle : l'eclairage public, la mise en valeur, la gestion du trafic. 
# à moins de créer un concept Function et d'jouter les differentes functions ou de de distingué  des sous classes de LightActuating 
seas:PublicLighting a owl:Class;
  rdfs:label "Public Lighting"@en ;
  rdfs:comment """Public Lighting is the process that allows to illuminate some public zone."""@en ;
  rdfs:subClassOf seas:Lighting ;
  vs:term_status "testing" ;
  rdfs:isDefinedBy seas:ElectricStreetLightingSystemOntology .

## mise en valeur 
seas:Highlighting a owl:Class;
  rdfs:label "Highlighting"@en ;
  rdfs:comment """the Highlighting is the process that allows to highlight some public zone."""@en ;
  rdfs:subClassOf seas:Lighting ;
  vs:term_status "testing" ;
  rdfs:isDefinedBy seas:ElectricStreetLightingSystemOntology .


seas:TrafficSignalsLighting a owl:Class;
  rdfs:label "Traffic Signals Lighting"@en ;
  rdfs:comment """the traffic signals Lighting is the process that give lighting signals to control  the traffic flow."""@en ;
  rdfs:subClassOf seas:Lighting ;
  vs:term_status "testing" ;
  rdfs:isDefinedBy seas:ElectricStreetLightingSystemOntology .


seas:LightActuation a owl:Class;
    rdfs:label "Light Actuation"@en;
    rdfs:comment """Light Actuation is the execution of the action of lighting or light Actuating."""@en ;
    rdfs:subClassOf seas:Actuation ;
    rdfs:subClassOf [ owl:onProperty pep:executedBy ; owl:someValuesFrom seas:LightActuator ] ;
    rdfs:subClassOf [ owl:onProperty pep:methodUsed ; owl:someValuesFrom seas:Lighting ] ;
    rdfs:subClassOf [ owl:onProperty seas:illuminates ; owl:someValuesFrom seas:IlluminableZone ] ;
    owl:equivalentClass [ owl:onProperty pep:methodUsed ; owl:someValuesFrom seas:Lighting ] ;
    vs:term_status "testing" ;
    rdfs:isDefinedBy seas:ElectricStreetLightingSystemOntology .




# Sub class of LightActuator 

seas:ElectricLightFixtureSystem a owl:Class ;
  rdfs:label "Electric Light Fixture System"@en ;
  rdfs:comment """An Electric Light Fixture System, light fixture (US English), light fitting (UK English), or luminaire is an electrical device used to create 
                  artificial light by use of an electric lamp. All light fixtures have a fixture body and a light socket to hold the lamp and allow for its replacement. 
                  Fixtures may also have a switch to control the light, either attached to the lamp body or attached to the power cable. (source: Wikipedia)"""@en 
                ;
  skos:prefLabel "Luminaire"@en;               
  rdfs:subClassOf seas:LightActuator ;
  rdfs:subClassOf [ owl:onProperty pep:implements ; owl:someValuesFrom seas:Lighting ] ;
  owl:equivalentClass [ owl:onProperty pep:implements ; owl:someValuesFrom seas:Lighting ] ;
  vs:term_status "testing" ;
  rdfs:isDefinedBy seas:ElectricStreetLightingSystemOntology .



seas:ElectricOutdoorLightingSystem a owl:Class ;
  rdfs:label "Electric Outdoor Lighting System"@en ;
  rdfs:comment """An Electric Outdoor Lighting System, is an Electric Light Fixture System which is used to lighting exterior areas."""@en ;
  rdfs:subClassOf seas:ElectricLightFixtureSystem ;
  vs:term_status "testing" ;
  rdfs:isDefinedBy seas:ElectricStreetLightingSystemOntology .


seas:ElectricPublicLightingSystem a owl:Class ;
  rdfs:label " Electric Public Lighting System"@en ;
  rdfs:comment """A Public Electric Lighting System, is an Electric Outdoor Lighting System which is used to lighting a public area like a road, street, public place, garden etc."""@en ;
  rdfs:subClassOf seas:ElectricOutdoorLightingSystem ;
  rdfs:subClassOf [ owl:onProperty seas:connectedTo ; owl:someValuesFrom seas:StreetLightSupport];
  rdfs:subClassOf [ owl:onProperty seas:connectedTo ; 
                    owl:qualifiedCardinality "1"^^xsd:nonNegativeInteger ;
                    owl:onClass seas:PowerBox];
  rdfs:subClassOf [ rdf:type owl:Restriction ;
                                   owl:onProperty seas:hasSubSystem ;
                                   owl:someValuesFrom seas:ElectricLightSource
                                 ] ;
  rdfs:subClassOf [ owl:onProperty seas:wearState ; owl:someValuesFrom seas:WearStateProperty];  
  rdfs:subClassOf [ owl:onProperty seas:height ; owl:someValuesFrom seas:LengthProperty]; 
  rdfs:subClassOf [ owl:onProperty seas:onState ; owl:someValuesFrom seas:BooleanProperty];       
  rdfs:subClassOf [ owl:onProperty seas:location ; owl:someValuesFrom seas:ZoneLightingOntology];                              
  vs:term_status "testing" ;
  rdfs:isDefinedBy seas:ElectricStreetLightingSystemOntology .


seas:TrafficControlSignal a owl:Class;
  rdfs:label "Traffic Control Signal"@en;
   rdfs:comment """Traffic lights, also known as traffic signals, traffic lamps, traffic semaphore, signal lights, stop lights, robots (in South Africa), 
                    and traffic control signals (in technical parlance),[1] are signalling devices positioned at road intersections, pedestrian crossings, and other 
                    locations to control flows of traffic."""@fr ;
  rdfs:subClassOf seas:ElectricPublicLightingSystem ;
  vs:term_status "testing" ;
  rdfs:isDefinedBy seas:ElectricStreetLightingSystemOntology .


seas:StreetLight a owl:Class ;
  rdfs:label "Street light"@en ;
  rdfs:comment """A Steet light, light pole, lamppost, street lamp, light standard, or lamp standard is an Public Electric Lighting System which   
                  is a raised source of light on the edge of a road or path.(source: Wikipedia)"""@en,
               """A luminaire is a lighting fixture used to distribute, filter or transform light from lamps. Also called lanterns, their function is to emit, 
                   distribute and control light emitted by a light source. Usually used for track lighting, they consist of an optics, electrical devices that 
                   allow the connection of the lamp (s), a body on which these different elements are based, and Makes it possible to be fixed to a support. """@en,
               """Un luminaire est un appareil d'éclairage servant à répartir, filtrer ou transformer la lumière des lampes. Egalement appelés lanternes, 
                   leur fonction est d'émettre, de distribuer et de contrôler la lumière émise par une source lumineuse. Généralement utilisés pour l'éclairage des 
                   voies, ils se composent d'une optique, d'appareils électriques qui permettent le branchement de la (les) lampe(s), d'un corps sur lequel 
                   s'appuient ces différents éléments, et qui permet d'être fixé à un support."""@fr ;
  rdfs:subClassOf seas:ElectricPublicLightingSystem ;
  vs:term_status "testing" ;
  rdfs:isDefinedBy seas:ElectricStreetLightingSystemOntology .


seas:Spotlight a owl:Class ;
  rdfs:label "Spotlight"@en ;
  rdfs:comment """A spotlight  (or searchlight) is a Street light that combines an extremely luminous source (traditionally a carbon arc lamp) with a mirrored
                   parabolic reflector to project a powerful beam of light of approximately parallel rays in a particular direction, usually constructed so that 
                   it can be swiveled about. (source: Wikipedia)"""@fr ;
  rdfs:subClassOf seas:StreetLight ;
  vs:term_status "testing" ;
  rdfs:isDefinedBy seas:ElectricStreetLightingSystemOntology .

seas:SolarStreetlight a owl:Class ;
  rdfs:label "Solar Street light"@en ;
  rdfs:comment """Solar street lights are raised light sources which are powered by photovoltaic panels generally mounted on the lighting structure or integrated in the 
                pole itself. The photovoltaic panels charge a rechargeable battery, which powers a fluorescent or LED lamp during the night. (source: Wikipedia)"""@fr ;
  rdfs:subClassOf seas:StreetLight ;
  rdfs:subClassOf [ owl:onProperty seas:isPoweredBy ; owl:someValuesFrom seas:Battery ] ; 
  owl:equivalentClass [owl:intersectionOf (seas:StreetLight [owl:onProperty seas:isPoweredBy ;
                                        owl:someValuesFrom [ owl:intersectionOf ( seas:Battery [ owl:onProperty seas:isPoweredBy ; owl:someValuesFrom seas:SolarPanel
                                                                                  ]
                                                                                ) ;
                                                             rdf:type owl:Class
                                                           ]])] ;
  vs:term_status "testing" ;
  rdfs:isDefinedBy seas:ElectricStreetLightingSystemOntology .  

seas:EquipableStreetLight a owl:Class;
  rdfs:label "Equipable Street light"@en ;
  rdfs:comment """An Equipable Street light,  is a Street light which   
                  can be equipable"""@en ;
  rdfs:subClassOf seas:StreetLight ;
  rdfs:subClassOf   [ owl:intersectionOf ( [ owl:onProperty seas:isEquipable ;
                                                                   owl:qualifiedCardinality "1"^^xsd:nonNegativeInteger ;
                                                                   owl:onClass seas:BooleanProperty
                                                                 ]
                                                                 [ rdf:type owl:Restriction ;
                                                                   owl:onProperty seas:simpleValue ;
                                                                   owl:hasValue "true"^^xsd:boolean
                                                                 ]
                                                               ) ;
                                          ] ; 
  owl:equivalentClass [ owl:intersectionOf ( seas:StreetLight
                                                                     [ owl:intersectionOf ( [ owl:onProperty seas:isEquipable ;
                                                                                              owl:qualifiedCardinality "1"^^xsd:nonNegativeInteger ;
                                                                                              owl:onClass seas:BooleanProperty
                                                                                            ]
                                                                                            [ rdf:type owl:Restriction ;
                                                                                              owl:onProperty seas:simpleValue ;
                                                                                              owl:hasValue "true"^^xsd:boolean
                                                                                            ]
                                                                                          ) ;
                                                                     ]
                                                                   ) ;
                                                rdf:type owl:Class
                                              ] ;
                         
  vs:term_status "testing" ;
  rdfs:isDefinedBy seas:ElectricStreetLightingSystemOntology .


seas:NoEquipableStreetLight a owl:Class;
  rdfs:label "No Equipable Street light"@en ;
  rdfs:comment """An No Equipable Street light,  is a Street light which   
                  is not equipable"""@en ;
  rdfs:subClassOf seas:StreetLight ;
  rdfs:subClassOf   [ owl:intersectionOf ( [ owl:onProperty seas:isEquipable ;
                                                                   owl:qualifiedCardinality "1"^^xsd:nonNegativeInteger ;
                                                                   owl:onClass seas:BooleanProperty
                                                                 ]
                                                                 [ rdf:type owl:Restriction ;
                                                                   owl:onProperty seas:simpleValue ;
                                                                   owl:hasValue "false"^^xsd:boolean
                                                                 ]
                                                               ) ;
                                          ] ; 
  owl:equivalentClass [ owl:intersectionOf ( seas:StreetLight
                                                                     [ owl:intersectionOf ( [ owl:onProperty seas:isEquipable ;
                                                                                              owl:qualifiedCardinality "1"^^xsd:nonNegativeInteger ;
                                                                                              owl:onClass seas:BooleanProperty
                                                                                            ]
                                                                                            [ rdf:type owl:Restriction ;
                                                                                              owl:onProperty seas:simpleValue ;
                                                                                              owl:hasValue "false"^^xsd:boolean
                                                                                            ]
                                                                                          ) ;
                                                                     ]
                                                                   ) ;
                                                rdf:type owl:Class
                                              ] ;
  
  owl:disjointWith seas:EquipableStreetLight;
  vs:term_status "testing" ;
  rdfs:isDefinedBy seas:ElectricStreetLightingSystemOntology .

seas:TopFixationStreetLight a owl:Class;
  rdfs:label "Top Fixation Street light"@en ;
  rdfs:comment """A Top fixation Street light,  is a Street light which   
                  is fixed on the top of the support through Top fixation"""@en ;
  rdfs:subClassOf seas:StreetLight ;
  owl:equivalentClass [ owl:intersectionOf (seas:StreetLight[ owl:onProperty seas:fixedInTopTo ; owl:someValuesFrom seas:StreetLightSupport ] )];
  owl:equivalentClass [ owl:intersectionOf (seas:StreetLight[ owl:onProperty seas:connectsSystem ; owl:someValuesFrom seas:TopFixation ])] ;
  vs:term_status "testing" ;
  rdfs:isDefinedBy seas:ElectricStreetLightingSystemOntology .

seas:FacadeFixationStreetLight a owl:Class;
  rdfs:label "Facade Fixation Street light"@en ;
  rdfs:comment """A Facade fixation Street light,  is a Street light which   
                  is fixed on the facade support through Facade fixation"""@en ;
  rdfs:subClassOf seas:StreetLight ;
  owl:equivalentClass [ owl:intersectionOf (seas:StreetLight[ owl:onProperty seas:fixedInFacadeTo ; owl:someValuesFrom seas:StreetLightSupport ] )];
  owl:equivalentClass [ owl:intersectionOf (seas:StreetLight[ owl:onProperty seas:connectsSystem ; owl:someValuesFrom seas:FacadeFixation ] )];
  vs:term_status "testing" ;
  rdfs:isDefinedBy seas:ElectricStreetLightingSystemOntology .

seas:ArmFixationStreetLight a owl:Class;
  rdfs:label "Arm Fixation Street light"@en ;
  rdfs:comment """An Arm fixation Street light, is a Street light which   
                  is fixed via an arm of the support through Arm fixation"""@en ;
  rdfs:subClassOf seas:StreetLight ;
  owl:equivalentClass [ owl:intersectionOf (seas:StreetLight[ owl:onProperty seas:fixedViaAnArmTo ; owl:someValuesFrom seas:StreetLightSupport ])] ;
  owl:equivalentClass [ owl:intersectionOf (seas:StreetLight[ owl:onProperty seas:connectsSystem ; owl:someValuesFrom seas:ArmFixation ] )];
  vs:term_status "testing" ;
  rdfs:isDefinedBy seas:ElectricStreetLightingSystemOntology .

seas:RecessedFloorStreetLight a owl:Class;
  rdfs:label "Recessed Floor Street Light"@en ;
  rdfs:comment """Recessed Floor Street Light is a StreetLight which is recessed in the floor."""@en ;
  rdfs:subClassOf seas:StreetLight ;
  rdfs:subClassOf [ owl:onProperty seas:connectedTo ; owl:someValuesFrom seas:RecessedFloorLightSupport];
  owl:equivalentClass [ owl:intersectionOf (seas:StreetLight [owl:onProperty seas:connectedTo ; owl:someValuesFrom seas:RecessedFloorLightSupport])];
  vs:term_status "testing" ;
  rdfs:isDefinedBy seas:ElectricStreetLightingSystemOntology .



seas:ElectricPublicLightingSystemGroup   a owl:Class;
  rdfs:label "Electric Public Lighting System Group"@en ;
  rdfs:comment """Electric Public Lighting System Group is a group system which has member only Electric Public Lighting System and minimum two of them."""@en ;
  rdfs:subClassOf seas:ElectricPowerSystem ;
  rdfs:subClassOf [ owl:onProperty seas:member ; owl:allValuesFrom seas:ElectricPublicLightingSystem];
  rdfs:subClassOf [ owl:onProperty seas:member ; owl:minQualifiedCardinality  "2"^^xsd:nonNegativeInteger ; owl:onClass seas:ElectricPublicLightingSystem];
  vs:term_status "testing" ;
  rdfs:isDefinedBy seas:ElectricStreetLightingSystemOntology .

[] a owl:AllDisjointClasses ; 
  owl:members ( 
    seas:ArmFixationStreetLight 
    seas:FacadeFixationStreetLight  
    seas:TopFixationStreetLight ) .

[] a owl:AllDisjointClasses ; 
  owl:members ( 
    seas:StreetLight 
    seas:StreetLightSupport  
    seas:StreetLightFixation
    seas:StreetLightFixationPoint
    seas:PowerBox
    seas:ElectricLightSource ) .

seas:StreetLightSupport a owl:Class ;
  rdfs:label "Lighting Support"@en ;
  rdfs:comment """Lighting Support is a support on which one or more streetLight are fixed on it"""@en ;
  rdfs:subClassOf seas:System ;
  rdfs:subClassOf [ owl:onProperty seas:wearState ; owl:someValuesFrom seas:WearStateProperty];
  rdfs:subClassOf [ owl:onProperty seas:height ; owl:someValuesFrom seas:LengthProperty];
  rdfs:subClassOf [ owl:onProperty seas:location ; owl:someValuesFrom seas:Property];
  vs:term_status "testing" ;
  rdfs:isDefinedBy seas:ElectricStreetLightingSystemOntology .


seas:StreetLightPole a owl:Class ;
  rdfs:label "Street Light Pole"@en ;
  rdfs:comment """Street Light Pole is a Lighting Support which is used to fixe  one or more streetlight on it."""@en ;
  rdfs:subClassOf seas:StreetLightSupport ;
  vs:term_status "testing" ;
  rdfs:isDefinedBy seas:ElectricStreetLightingSystemOntology .


seas:StreetLightCandelabra a owl:Class ;
  rdfs:label "Candelabra Street Light"@en ;
  rdfs:comment """Candelabra Street Light is a Lighting Support which is used to fixe one or more streetlight on it. It is generally designed like a Candelabra ."""@en ;
  rdfs:subClassOf seas:StreetLightSupport ;
  vs:term_status "testing" ;
  rdfs:isDefinedBy seas:ElectricStreetLightingSystemOntology .

seas:StreetLightFacadeSupport a owl:Class ;
  rdfs:label "Street Light Facade Support"@en ;
  rdfs:comment """Street Light Facade Support is a Lighting Support which is used to fixe the streetlight."""@en ;
  rdfs:subClassOf seas:StreetLightSupport ;
  vs:term_status "testing" ;
  rdfs:isDefinedBy seas:ElectricStreetLightingSystemOntology .

seas:RecessedFloorLightSupport a owl:Class ;
      rdfs:label "Recessed Floor Light Support"@en ;
      rdfs:comment """Recessed Floor Light Support is a Lighting Support which is used to fixe a Recessed Floor Light Support."""@en ;
      rdfs:subClassOf seas:StreetLightSupport ;
      vs:term_status "testing" ;
      rdfs:isDefinedBy seas:ElectricStreetLightingSystemOntology .


seas:StreetLightColumnSupport a owl:Class ;
  rdfs:label "Street Light Column Support"@en ;
  rdfs:comment """Street Light Column Support is a Lighting Support which is used to fixe the streetlight."""@en ;
  rdfs:subClassOf seas:StreetLightSupport ;
  vs:term_status "testing" ;
  rdfs:isDefinedBy seas:ElectricStreetLightingSystemOntology .


seas:StreetLightBornSupport a owl:Class ;
  rdfs:label "Street Light Born Support"@en ;
  rdfs:comment """Street Light Born Support is a Lighting Support which is used to fixe the streetlight."""@en ;
  rdfs:subClassOf seas:StreetLightSupport ;
  vs:term_status "testing" ;
  rdfs:isDefinedBy seas:ElectricStreetLightingSystemOntology .


seas:StreetLightFixation a owl:Class;
  rdfs:label "Street Light Fixation"@en ;
  rdfs:comment """Street Light Fixation is a connection which allowss to fixe a streetlight to the support."""@en ;
  rdfs:subClassOf seas:Connection ;
  vs:term_status "testing" ;
  rdfs:isDefinedBy seas:ElectricStreetLightingSystemOntology .

  
  seas:StreetLightFixationPoint a owl:Class;
      rdfs:label "Street Light Fixation Point"@en;
      rdfs:comment """Street Light Fixation Point is a connection Point which allowss to fixe a streetlight to the support."""@en ;
      rdfs:subClassOf seas:ConnectionPoint ;
      rdfs:subClassOf [ owl:onProperty seas:connectionPointOf ; owl:allValuesFrom   [owl:unionOf (seas:StreetLight seas:StreetLightSupport)]] ;
      rdfs:subClassOf [ owl:onProperty seas:connectsSystemThrough ; owl:allValuesFrom  seas:StreetLightFixation ] ;
      vs:term_status "testing" ;
      rdfs:isDefinedBy seas:ElectricStreetLightingSystemOntology .


  seas:ArmFixation a owl:Class;
  rdfs:label "Arm Fixation"@en ;
  rdfs:comment """Arm Fixation is a Street Light Fixation which allows to fixe a streetlight to the support via an Arm."""@en ;
  rdfs:subClassOf seas:StreetLightFixation ;
  vs:term_status "testing" ;
  rdfs:isDefinedBy seas:ElectricStreetLightingSystemOntology .


  seas:LuminaireArmFixationPoint a owl:Class;
  rdfs:label "Arm Fixation Point"@en ;
  rdfs:comment """A Luminaire Arm Fixation Point is a Street Light Fixation point which allows the point fixation between the luminaire and the ArmFixation."""@en ;
  rdfs:subClassOf seas:StreetLightFixationPoint ;
  rdfs:subClassOf [ owl:onProperty seas:connectionPointOf ; owl:allValuesFrom   seas:StreetLight ] ;
  rdfs:subClassOf [ owl:onProperty seas:connectsSystemThrough ; owl:allValuesFrom  seas:ArmFixation ] ;
  vs:term_status "testing" ;
  rdfs:isDefinedBy seas:ElectricStreetLightingSystemOntology .


 seas:SupportArmFixationPoint a owl:Class;
  rdfs:label "Arm Fixation Point"@en ;
  rdfs:comment """A Support Arm Fixation Point is a Street Light Fixation point which allows the point fixation between the support and the ArmFixation."""@en ;
  rdfs:subClassOf seas:StreetLightFixationPoint ;
  rdfs:subClassOf [ owl:onProperty seas:connectionPointOf ; owl:allValuesFrom   seas:StreetLightSupport ] ;
  rdfs:subClassOf [ owl:onProperty seas:connectsSystemThrough ; owl:allValuesFrom  seas:ArmFixation ] ;
  vs:term_status "testing" ;
  rdfs:isDefinedBy seas:ElectricStreetLightingSystemOntology .


  seas:TopFixation a owl:Class;
  rdfs:label "Top Fixation"@en ;
  rdfs:comment """Top fixation is a a Street Light Fixation which allows to fise a streetlight to the support on the top."""@en ;
  rdfs:subClassOf seas:StreetLightFixation ;
  vs:term_status "testing" ;
  rdfs:isDefinedBy seas:ElectricStreetLightingSystemOntology .

 
 seas:LuminaireTopFixationPoint a owl:Class;
  rdfs:label "Luminaire Top Fixation Point"@en ;
  rdfs:comment """A Luminaire Top Fixation Point is a Street Light Fixation point which allows the point fixation between the luminaire and the TopFixation."""@en ;
  rdfs:subClassOf seas:StreetLightFixationPoint ;
  rdfs:subClassOf [ owl:onProperty seas:connectionPointOf ; owl:allValuesFrom   seas:StreetLight ] ;
  rdfs:subClassOf [ owl:onProperty seas:connectsSystemThrough ; owl:allValuesFrom  seas:TopFixation ] ;
  vs:term_status "testing" ;
  rdfs:isDefinedBy seas:ElectricStreetLightingSystemOntology .


seas:SupportTopFixationPoint a owl:Class;
  rdfs:label "Support top Fixation Point"@en ;
  rdfs:comment """Support top Fixation Point is a Street Light Fixation point which allows the point fixation between the support and the TopFixation."""@en ;
  rdfs:subClassOf seas:StreetLightFixationPoint ;
  rdfs:subClassOf [ owl:onProperty seas:connectionPointOf ; owl:allValuesFrom   seas:StreetLightSupport] ;
  rdfs:subClassOf [ owl:onProperty seas:connectsSystemThrough ; owl:allValuesFrom  seas:TopFixation ] ;
  vs:term_status "testing" ;
  rdfs:isDefinedBy seas:ElectricStreetLightingSystemOntology .


  seas:FacadeFixation a owl:Class;
  rdfs:label "Facade Fixation"@en ;
  rdfs:comment """Facade fixation a a Street Light Fixation which allows a streetlight to the  facade support."""@en ;
  rdfs:subClassOf seas:StreetLightFixation ;
  vs:term_status "testing" ;
  rdfs:isDefinedBy seas:ElectricStreetLightingSystemOntology .

seas:LuminaireFacadeFixationPoint a owl:Class;
  rdfs:label "Luminaire Facade Fixation Point"@en ;
  rdfs:comment """A Luminaire Facade Fixation Point is a Street Light Fixation point which allows the point fixation between the luminaire and the FacadeFixation."""@en ;
  rdfs:subClassOf seas:StreetLightFixationPoint ;
  rdfs:subClassOf [ owl:onProperty seas:connectionPointOf ; owl:allValuesFrom   seas:StreetLight ] ;
  rdfs:subClassOf [ owl:onProperty seas:connectsSystemThrough ; owl:allValuesFrom  seas:FacadeFixation ] ;
  vs:term_status "testing" ;
  rdfs:isDefinedBy seas:ElectricStreetLightingSystemOntology .


seas:SupportFacadeFixationPoint a owl:Class;
  rdfs:label "Support Facade Fixation Point"@en ;
  rdfs:comment """Support Facade Fixation Point is a Street Light Fixation point which allows the point fixation between the support and the FacadeFixation."""@en ;
  rdfs:subClassOf seas:StreetLightFixationPoint ;
  rdfs:subClassOf [ owl:onProperty seas:connectionPointOf ; owl:allValuesFrom   seas:StreetLightSupport] ;
  rdfs:subClassOf [ owl:onProperty seas:connectsSystemThrough ; owl:allValuesFrom  seas:TopFixation ] ;
  vs:term_status "testing" ;
  rdfs:isDefinedBy seas:ElectricStreetLightingSystemOntology .


seas:RecessedFloorFixation a owl:Class;
  rdfs:label "Recessed Floor Fixation"@en ;
  rdfs:comment """A Recessed Floor Fixation is a Street Light Fixation which allows a streetlight to be recessed in the floor."""@en ;
  rdfs:subClassOf seas:StreetLightFixation ;
  vs:term_status "testing" ;
  rdfs:isDefinedBy seas:ElectricStreetLightingSystemOntology .

seas:RecessedFloorFixationPoint a owl:Class;
  rdfs:label "Recessed Floor Fixation Point"@en ;
  rdfs:comment """A Recessed Floor Fixation Point is a Street Light Fixation point which allows the point fixation between the support and the Recessed Floor Fixation."""@en ;
  rdfs:subClassOf seas:StreetLightFixationPoint ;
  rdfs:subClassOf [ owl:onProperty seas:connectionPointOf ; owl:allValuesFrom   seas:RecessedFloorLightSupport] ;
  rdfs:subClassOf [ owl:onProperty seas:connectsSystemThrough ; owl:allValuesFrom  seas:RecessedFloorFixation ] ;
  vs:term_status "testing" ;
  rdfs:isDefinedBy seas:ElectricStreetLightingSystemOntology .

  seas:PowerBox a owl:Class;
      rdfs:label "Power box"@en ;
      rdfs:comment """A power box (USA) or feeder pillar (UK) is a cabinet for electrical equipment, 
                      mounted in the street and controlling the electrical supply to a number of houses in a neighborhood. (source:wikipedia)"""@en ;
      rdfs:subClassOf seas:ElectricPowerSystem ;
      rdfs:subClassOf [ owl:onProperty seas:connectedTo ; owl:someValuesFrom seas:ElectricPublicLightingSystem];
      vs:term_status "testing" ;
      rdfs:isDefinedBy seas:ElectricStreetLightingSystemOntology .


seas:ElectricalBallast a owl:Class;
      rdfs:label "Electrical Ballast"@en ;
      rdfs:comment """An electrical ballast is a device placed in line with the load to limit the amount of current in an electrical circuit. 
                      It may be a fixed or variable resistor.
                      A familiar and widely used example is the inductive ballast used in fluorescent lamps to limit the current through the tube, 
                      which would otherwise rise to a destructive level due to the negative differential resistance artifact in the tube's voltage-current 
                      characteristic. Ballasts vary greatly in complexity. They may be as simple as a resistor, inductor or capacitor (or a combination of these) 
                      wired in series with the lamp; or as complex as the electronic ballasts used in compact fluorescent lamps and high-intensity discharge lamps. 
                      (source:wikipedia)"""@en ;
      rdfs:subClassOf seas:ElectricPowerSystem ;
      vs:term_status "testing" ;
      rdfs:isDefinedBy seas:ElectricStreetLightingSystemOntology .      

seas:ElectronicBallast a owl:Class;
      rdfs:label "Electronic ballast"@en ;
      rdfs:comment """An electronic ballast uses solid state electronic circuitry to provide the proper starting and operating electrical conditions to power discharge lamps.
                      An electronic ballast can be smaller and lighter than a comparably-rated magnetic one. An electronic ballast is usually quieter than a magnetic one,
                      which produces a line-frequency hum by vibration of the transformer laminations. 
                      (source:wikipedia)"""@en ;
      rdfs:subClassOf seas:ElectricalBallast ;
      vs:term_status "testing" ;
      rdfs:isDefinedBy seas:ElectricStreetLightingSystemOntology . 

seas:MagneticBallast   a owl:Class;
      rdfs:label "Magnetic ballast"@en ;
      rdfs:comment """Magnetic ballast is a Ballast which is Magnetic"""@en ;
      rdfs:subClassOf seas:ElectricalBallast ;
      vs:term_status "testing" ;
      rdfs:isDefinedBy seas:ElectricStreetLightingSystemOntology .

seas:DigitalBallast   a owl:Class;
      rdfs:label "Digital ballast "@en ;
      rdfs:comment """Digital ballast is a Ballast which is Digital"""@en ;
      rdfs:subClassOf seas:ElectricalBallast ;
      vs:term_status "testing" ;
      rdfs:isDefinedBy seas:ElectricStreetLightingSystemOntology .


seas:ElectricPowerDistributionNetwork   a owl:Class;
      rdfs:label "Electric Power Distribution Network"@en ;
      rdfs:comment """"""@en ;
      rdfs:subClassOf seas:ElectricPowerSystem ;
      vs:term_status "testing" ;
      rdfs:isDefinedBy seas:ElectricStreetLightingSystemOntology .


seas:UndergroundElectricPowerDistributionNetwork   a owl:Class;
      rdfs:label "Underground Electric Power Distribution Network"@en ;
      rdfs:comment """UndergroundElectricPowerDistributionNetwork is an ElectricPowerDistributionNetwork which is buried underground."""@en ;
      rdfs:subClassOf seas:ElectricPowerDistributionNetwork ;
      vs:term_status "testing" ;
      rdfs:isDefinedBy seas:ElectricStreetLightingSystemOntology .

seas:OverheadElectricPowerDistributionNetwork   a owl:Class;
      rdfs:label "Overhead Electric Power Distribution Network"@en ;
      rdfs:comment """OverheadElectricPowerDistributionNetwork is an ElectricPowerDistributionNetwork which is suspended in the air. """@en ;
      rdfs:subClassOf seas:ElectricPowerDistributionNetwork ;
      vs:term_status "testing" ;
      rdfs:isDefinedBy seas:ElectricStreetLightingSystemOntology .

seas:FacadeElectricPowerDistributionNetwork   a owl:Class;
      rdfs:label "Facade Electric Power Distribution Network"@en ;
      rdfs:comment """FacadeElectricPowerDistributionNetwork is an ElectricPowerDistributionNetwork which is hanging  along a facade."""@en ;
      rdfs:subClassOf seas:ElectricPowerDistributionNetwork;
      vs:term_status "testing" ;
      rdfs:isDefinedBy seas:ElectricStreetLightingSystemOntology .


## Model
 seas:ElectricLightFixtureSystemModel a owl:Class;
      rdfs:label "Electric Light Fixture System model"@en;
      rdfs:comment """Street light model."""@en ;
      rdfs:subClassOf gr:ProductOrServiceModel;
      vs:term_status "testing" ;
      rdfs:isDefinedBy seas:ElectricStreetLightingSystemOntology .

seas:LightingSupportModel       a owl:Class;
      rdfs:label "Electric Light Fixture System model"@en;
      rdfs:comment """Street light model."""@en ;
      rdfs:subClassOf gr:ProductOrServiceModel;
      vs:term_status "testing" ;
      rdfs:isDefinedBy seas:ElectricStreetLightingSystemOntology .




## concepts to add knowledge about the kind of location the streetilght is.

seas:City a owl:Class;
      rdfs:label "City"@en ;
      rdfs:comment """City is a Zone which is a relatively large and permanent human settlement ."""@en ;
      rdfs:subClassOf seas:Zone;
      vs:term_status "testing" ;
      rdfs:isDefinedBy seas:ElectricStreetLightingSystemOntology .

seas:CityCenter a owl:Class;
      rdfs:label "City Center"@en ;
      rdfs:comment """City center is a city which is A city centre (or city center) is the commercial, cultural and often the historical, 
                      political and geographic heart of a city. The term "city centre" is not usually used in American English;
                       rather, in North America, the term Downtown is used.."""@en ;
      rdfs:subClassOf seas:City;
      vs:term_status "testing" ;
      rdfs:isDefinedBy seas:ElectricStreetLightingSystemOntology .

seas:OldCityCenter a owl:Class;
      rdfs:label "Old City Center"@en ;
      rdfs:comment """Old City center is a city center which is which was constructed a long time ago."""@en ;
      rdfs:subClassOf seas:City;
      vs:term_status "testing" ;
      rdfs:isDefinedBy seas:ElectricStreetLightingSystemOntology .

seas:ShoppingCityCenter a owl:Class;
      rdfs:label "Shopping City Center"@en ;
      rdfs:comment """A Shopping City center is a city center which where there are a lot of shops."""@en ;
      rdfs:subClassOf seas:City;
      vs:term_status "testing" ;
      rdfs:isDefinedBy seas:ElectricStreetLightingSystemOntology .      

seas:Stadium a owl:Class;
      rdfs:label "Stadium"@en ;
      rdfs:comment """A stadium is a place or venue for (mostly) outdoor sports, concerts, or other events and consists of a field or stage either partly or completely 
                      surrounded by a tiered structure designed to allow spectators to stand or sit and view the event.(source:wikipedia)"""@en ;
      rdfs:subClassOf seas:CivilEngineeringWork;
      vs:term_status "testing" ;
      rdfs:isDefinedBy seas:ElectricStreetLightingSystemOntology .  

seas:CarPark a owl:Class;
      rdfs:label "CarPark"@en ;
      rdfs:comment """A parking lot (American English) or car park (British English), also known as a car lot, is a cleared area that is intended for parking vehicles.(source:wikipedia)"""@en ;
      rdfs:subClassOf seas:CivilEngineeringWork;
      vs:term_status "testing" ;
      rdfs:isDefinedBy seas:ElectricStreetLightingSystemOntology .  
    
seas:Bridge a owl:Class;
      rdfs:label "Bridge"@en ;
      rdfs:comment """A bridge is a structure built to span physical obstacles without closing the way underneath such as a body of water, valley, or road, 
                      for the purpose of providing passage over the obstacle.(source:wikipedia)"""@en ;
      rdfs:subClassOf seas:CivilEngineeringWork;
      vs:term_status "testing" ;
      rdfs:isDefinedBy seas:ElectricStreetLightingSystemOntology .

seas:Park a owl:Class;
      rdfs:label "Park"@en ;
      rdfs:comment """A park is an area of natural, semi-natural or planted space set aside for human enjoyment and recreation or for the protection of wildlife or natural habitats.(source:wikipedia)"""@en ;
      rdfs:subClassOf seas:Zone;
      vs:term_status "testing" ;
      rdfs:isDefinedBy seas:ElectricStreetLightingSystemOntology .  

seas:Garden a owl:Class;
      rdfs:label "Garden";
      rdfs:comment """A garden is a planned space, usually outdoors, set aside for the display, cultivation, and enjoyment of plants and other forms of nature. 
                      The garden can incorporate both natural and man-made materials. (source:wikipedia)"""@en ;
      rdfs:subClassOf seas:Zone;
      vs:term_status "testing" ;
      rdfs:isDefinedBy seas:ElectricStreetLightingSystemOntology .        

seas:Thoroughfare a owl:Class ;
  rdfs:label "Thoroughfare"@en ;     
  rdfs:comment """A thoroughfare is a transportation route connecting one location to another. On land a thoroughfare may refer to anything from a multi-lane 
                highway with grade separated junctions, to a rough trail.[citation needed] Thoroughfares used by a variety of traffic, such as cars on roads and 
                highways. On water a thoroughfare may refer to a strait, channel or waterway. The term may also refer to access to a route, distinct from the route 
                itself. In other words thoroughfare may refer to the legal right to use a particular way. (source:Wikipedia)"""@en ;
  rdfs:subClassOf seas:CivilEngineeringWork ;
  vs:term_status "testing" ;
  rdfs:isDefinedBy seas:ElectricStreetLightingSystemOntology . 

seas:Tunnel a owl:Class ;
  rdfs:label "Tunnel"@en ;
  rdfs:comment """A tunnel is an underground passageway, dug through the surrounding soil/earth/rock and enclosed except for entrance and exit, commonly at each end. 
                  A pipeline is not a tunnel, though some recent tunnels have used immersed tube construction techniques rather than traditional tunnel boring methods. (source: wikipedia)"""@en ;
  rdfs:subClassOf seas:Thoroughfare ;
  vs:term_status "testing" ;
  rdfs:isDefinedBy seas:ElectricStreetLightingSystemOntology . 

seas:Bickway a owl:Class ;
  rdfs:label "Bickway"@en ;
  rdfs:comment "A bikeway is a lane, route, way or path which in some manner is specifically designed and /or designated for bicycle travel"@en ;
  rdfs:subClassOf seas:Thoroughfare ;
  vs:term_status "testing" ;
  rdfs:isDefinedBy seas:ElectricStreetLightingSystemOntology . 

seas:Pedestrian_way a owl:Class ;
  rdfs:label "Pedestrian_way"@en ;
  rdfs:subClassOf seas:Thoroughfare ;
  vs:term_status "testing" ;
  rdfs:isDefinedBy seas:ElectricStreetLightingSystemOntology . 

seas:Road a owl:Class ;
  rdfs:label "Road"@en ;
  rdfs:comment """A road is a thoroughfare, route, or way on land between two places that has been paved or otherwise improved to allow travel by foot or some form of 
                  onveyance, including a motor vehicle, cart, bicycle, or horse."""@en ;
  rdfs:subClassOf seas:Thoroughfare ;
  vs:term_status "testing" ;
  rdfs:isDefinedBy seas:ElectricStreetLightingSystemOntology . 

seas:PrimaryPathway a owl:Class ;
  rdfs:label "Primary pathway"@en ;
  rdfs:comment """A Primary pathway is a thoroughfare, which is primary."""@en ;
  rdfs:subClassOf seas:Thoroughfare ;
  vs:term_status "testing" ;
  rdfs:isDefinedBy seas:ElectricStreetLightingSystemOntology .

seas:SecondaryPathway a owl:Class ;
  rdfs:label "Secondary pathway"@en ;
  rdfs:comment """A Secondary pathway is a thoroughfare, which is secondary."""@en ;
  rdfs:subClassOf seas:Thoroughfare ;
  vs:term_status "testing" ;
  rdfs:isDefinedBy seas:ElectricStreetLightingSystemOntology .

seas:TertiaryPathway a owl:Class ;
  rdfs:label "Tertiary pathway"@en ;
  rdfs:comment """A Tertiary pathway is a thoroughfare, which is tertiary."""@en ;
  rdfs:subClassOf seas:Thoroughfare ;
  vs:term_status "testing" ;
  rdfs:isDefinedBy seas:ElectricStreetLightingSystemOntology .


seas:Passageway a owl:Class ;
  rdfs:label "Passageway"@en ;
  rdfs:subClassOf seas:Thoroughfare ;
  vs:term_status "testing" ;
  rdfs:isDefinedBy seas:ElectricStreetLightingSystemOntology . 


seas:Avenue a owl:Class ;
  rdfs:label "Avenue"@en ;
  rdfs:comment """n landscaping, an avenue or allée is traditionally a straight path or road with a line of trees or large shrubs running along each side, 
                which is used, as its French source venir (\"to come\") indicates, to emphasize the \"coming to,\" or arrival at a landscape or architectural feature. 
                In most cases, the trees planted in an avenue will be all of the same species or cultivar, so as to give uniform appearance along the full length of the 
                avenue. (source : wikipedia)"""@en ;
  rdfs:subClassOf seas:Road ;
  vs:term_status "testing" ;
  rdfs:isDefinedBy seas:ElectricStreetLightingSystemOntology . 

seas:Backroad a owl:Class ;
  rdfs:label "Backroad"@en ;
  rdfs:comment "A backroad is a secondary type of road, usually found in rural areas. (source : wikipedia)"@en ;
  rdfs:subClassOf seas:Road ;
  vs:term_status "testing" ;
  rdfs:isDefinedBy seas:ElectricStreetLightingSystemOntology . 


seas:Boulevard a owl:Class ;
  rdfs:label "Boulevard"@en ;
  rdfs:comment """A boulevard (French, from Dutch: Bolwerk – bulwark, meaning bastion), often abbreviated Blvd, is a type of large road, usually running through a city.
In modern American usage it often means a wide, multi-lane arterial thoroughfare, divided with a median down the centre, and perhaps with roadways along each side designed as slow travel and parking lanes and for bicycle and pedestrian usage, often with an above-average quality of landscaping and scenery. (source:Wikipedia)"""@en ;
  rdfs:subClassOf seas:Road ;
  vs:term_status "testing" ;
  rdfs:isDefinedBy seas:ElectricStreetLightingSystemOntology . 

 seas:Dead_end a owl:Class ;
  rdfs:label "Dead end"@en ;
  rdfs:comment "A dead end, also known as a cul-de-sac, is a street with only one inlet/outlet.  (source: wikipedia)"@en ;
  rdfs:subClassOf seas:Road ;
  vs:term_status "testing" ;
  rdfs:isDefinedBy seas:ElectricStreetLightingSystemOntology . 
   
seas:Street a owl:Class ;
  rdfs:label "Street"@en ;
  rdfs:comment """A street is a public thoroughfare (usually paved) in a built environment. 
                  It is a public parcel of land adjoining buildings in an urban context, on which people may freely assemble, interact, and move about.(source: wikipedia) """@en;
  rdfs:subClassOf seas:Road ;
  vs:term_status "testing" ;
  rdfs:isDefinedBy seas:ElectricStreetLightingSystemOntology . 


seas:Highway a owl:Class;
  rdfs:label "Highway"@en ;
  rdfs:comment """A highway is any public road or other public way on land. It is used for major roads, but also includes other public roads and public tracks: 
                It is not an equivalent term to controlled-access highway, or a translation for autobahn, autoroute, etc. (source: wikipedia)"""@en ;
  rdfs:subClassOf seas:Road ;
  rdfs:isDefinedBy seas:ElectricStreetLightingSystemOntology . 

seas:Bypass a owl:Class;
  rdfs:label "Bypass"@en ;
  rdfs:comment """A bypass is a road  that avoids or "bypasses" a built-up area, town, or village, to let through traffic flow without interference from local traffic, 
                    to reduce congestion in the built-up area, and to improve road safety. A bypass specifically designated for trucks may be called a truck route. (source: wikipedia)"""@en ;
  rdfs:subClassOf seas:Road ;
  rdfs:isDefinedBy seas:ElectricStreetLightingSystemOntology .

seas:ThoroughfareSection  a owl:Class;
  rdfs:label "Thoroughfare Section"@en ;
  rdfs:comment """A Thoroughfare Section is a part of the throughfare. (source: wikipedia)"""@en ;
  rdfs:subClassOf seas:CivilEngineeringWork ;
  rdfs:subClassOf  [ owl:onProperty seas:subSystemOf; owl:qualifiedCardinality "1"^^xsd:nonNegativeInteger ; owl:onClass seas:Thoroughfare
                                         ] ;
  rdfs:isDefinedBy seas:ElectricStreetLightingSystemOntology .  


seas:IlluminanceProperty a owl:Class ; 
      rdfs:label "Illuminance Property"@en ;
      rdfs:comment """A Illuminance Property is a property which is inherent in a lightsource."""@en ;
      rdfs:subClassOf seas:Property;
      vs:term_status "testing" ;
      rdfs:isDefinedBy seas:ElectricStreetLightingSystemOntology .

seas:IlluminanceEvaluation  a owl:Class ; 
      rdfs:label "Illuminance Evaluation"@en ;
      rdfs:comment """A Illuminance Evaluation is an evaluation of Illuminance Propert."""@en ;
      rdfs:subClassOf seas:Evaluation;
      vs:term_status "testing" ;
      rdfs:isDefinedBy seas:ElectricStreetLightingSystemOntology .


seas:WearStateProperty  a owl:Class ; 
      rdfs:label "Wear State Property"@en ;
      rdfs:comment """A Wear State Property is a property which is inherent in a system."""@en ;
      rdfs:subClassOf seas:Property;
      vs:term_status "testing" ;
      rdfs:isDefinedBy seas:ElectricStreetLightingSystemOntology .

seas:WearStateEvaluation a owl:Class;
      rdfs:label "Wear State Evaluation"@en ;
      rdfs:comment """A Wear State evalaution is an evaluation which is an evaluation of the Property Wears State."""@en ;
      rdfs:subClassOf seas:Evaluation;
      rdfs:subClassOf [ owl:onProperty seas:evaluationOf ; owl:someValuesFrom seas:WearStateProperty ] ;
      owl:equivalentClass [ owl:onProperty seas:evaluationOf ; owl:someValuesFrom seas:WearStateProperty ] ;
      vs:term_status "testing" ;
      rdfs:isDefinedBy seas:ElectricStreetLightingSystemOntology .


seas:GoodStateEvaluation a owl:Class;
      rdfs:label "good State Evaluation"@en ;
      rdfs:comment """A good State evalaution is a WearStateEvaluation which is an evaluation of the Property Wears State."""@en ;
      rdfs:subClassOf seas:WearStateEvaluation;
      owl:equivalentClass [ owl:onProperty seas:evaluatedSimpleValue ; owl:hasValue "Bon"^^xsd:string ] ;
      vs:term_status "testing" ;
      rdfs:isDefinedBy seas:ElectricStreetLightingSystemOntology .

seas:VetusteStateEvaluation a owl:Class;
      rdfs:label "Vetuste State Evaluation"@en ;
      rdfs:comment """A Vetuste State evalaution is a WearStateEvaluation which is an evaluation of the Property Wears State."""@en ;
      rdfs:subClassOf seas:WearStateEvaluation;
      owl:equivalentClass [ owl:onProperty seas:evaluatedSimpleValue ; owl:hasValue "Vetuste"^^xsd:string ] ;
      vs:term_status "testing" ;
      rdfs:isDefinedBy seas:ElectricStreetLightingSystemOntology .  

seas:ObsoleteStateEvaluation a owl:Class;
      rdfs:label "Obsolete State Evaluation"@en ;
      rdfs:comment """A Obsolete State evalaution is a WearStateEvaluation which is an evaluation of the Property Wears State."""@en ;
      rdfs:subClassOf seas:WearStateEvaluation;
      owl:equivalentClass [ owl:onProperty seas:evaluatedSimpleValue ; owl:hasValue "Obsolete"^^xsd:string ] ;
      vs:term_status "testing" ;
      rdfs:isDefinedBy seas:ElectricStreetLightingSystemOntology . 

seas:AverageStateEvaluation a owl:Class;
      rdfs:label "Average State Evaluation"@en ;
      rdfs:comment """A Average State evalaution is a WearStateEvaluation which is an evaluation of the Property Wears State."""@en ;
      rdfs:subClassOf seas:WearStateEvaluation;
      owl:equivalentClass [ owl:onProperty seas:evaluatedSimpleValue ; owl:hasValue "Average"^^xsd:string ] ;
      vs:term_status "testing" ;
      rdfs:isDefinedBy seas:ElectricStreetLightingSystemOntology . 


seas:wearState a owl:ObjectProperty, owl:FunctionalProperty;
      rdfs:label "wearState"@en ;
      rdfs:comment """The wearState of some physical entity."""@en ;
      rdfs:subPropertyOf seas:hasProperty ;
      rdfs:domain seas:FeatureOfInterest ;
      rdfs:range seas:WearStateProperty ;
      vs:term_status "testing" ;
      rdfs:isDefinedBy seas:GenericPropertyOntology .

seas:fixedViaAnArmTo       a owl:ObjectProperty ;
      rdfs:label "fixed with arm to"@en ;
      rdfs:comment "means that the streetlight is fixed on the support via an ArmFixation."@en ;
      rdfs:subPropertyOf seas:connectedTo ;
      rdfs:domain seas:StreetLight ;
      rdfs:range seas:StreetLightSupport ;
      vs:term_status "testing" ;
      rdfs:isDefinedBy seas:ElectricStreetLightingSystemOntology .  

seas:fixedInTopTo       a owl:ObjectProperty ;
      rdfs:label "fixed in top to"@en ;
      rdfs:comment "means that the streetlight is fixed on the support via a top fixation."@en ;
      rdfs:subPropertyOf seas:connectedTo ;
      rdfs:domain seas:StreetLight ;
      rdfs:range seas:StreetLightSupport ;
      vs:term_status "testing" ;
      rdfs:isDefinedBy seas:ElectricStreetLightingSystemOntology .  

seas:fixedInFacadeTo       a owl:ObjectProperty ;
      rdfs:label "fixed in facade to"@en ;
      rdfs:comment "means that the streetlight is fixed on the facade support via a top fixation."@en ;
      rdfs:subPropertyOf seas:connectedTo ;
      rdfs:domain seas:StreetLight ;
      rdfs:range seas:StreetLightSupport ;
      vs:term_status "testing" ;
      rdfs:isDefinedBy seas:ElectricStreetLightingSystemOntology .          

seas:isFixingSupportViaAnArmOf   a owl:ObjectProperty ;
      rdfs:label "is Fixing Support Via An Arm Of"@en ;
      rdfs:comment "means that the streetlight is fixed on the support via an ArmFixation."@en ;
      rdfs:subPropertyOf seas:connectedTo ;
      rdfs:domain seas:StreetLightSupport ;
      rdfs:range seas:StreetLight ;
      owl:inverseOf seas:fixedViaAnArmTo;
      vs:term_status "testing" ;
      rdfs:isDefinedBy seas:ElectricStreetLightingSystemOntology .  

seas:isFixingSupportInTopOf   a owl:ObjectProperty ;
      rdfs:label "is Fixing Support Via An Arm Of"@en ;
      rdfs:comment "means that the streetlight is fixed on the support in the top."@en ;
      rdfs:subPropertyOf seas:connectedTo ;
      rdfs:domain seas:StreetLightSupport ;
      rdfs:range seas:StreetLight ;
      owl:inverseOf seas:fixedInTopTo;
      vs:term_status "testing" ;
      rdfs:isDefinedBy seas:ElectricStreetLightingSystemOntology .        

seas:isFixingSupportInFacadeOf   a owl:ObjectProperty ;
      rdfs:label "is Fixing Support In Facade Of"@en ;
      rdfs:comment "means that the streetlight is fixed on the support in a facade."@en ;
      rdfs:subPropertyOf seas:connectedTo ;
      rdfs:domain seas:StreetLightSupport ;
      rdfs:range seas:StreetLight ;
      owl:inverseOf seas:fixedInFacadeTo;
      vs:term_status "testing" ;
      rdfs:isDefinedBy seas:ElectricStreetLightingSystemOntology .       

seas:isEquipable a owl:DatatypeProperty;
        rdfs:comment "is equipable to check of the system is equipable or not."@en ;
      rdfs:domain seas:System ;
      rdfs:range seas:BooleanProperty ;
      vs:term_status "testing" ;
      rdfs:isDefinedBy seas:ElectricStreetLightingSystemOntology .  

seas:isPoweredBy  a owl:ObjectProperty ;
      rdfs:label "is powered by"@en ;
      rdfs:comment "links a System to its powered system."@en ;
      rdfs:subPropertyOf seas:exchangesElectricityWith ;
      rdfs:domain seas:System ;
      rdfs:range seas:System ;
      owl:inverseOf seas:powers;
      vs:term_status "testing" ;
      rdfs:isDefinedBy seas:ElectricStreetLightingSystemOntology .    

seas:powers  a owl:ObjectProperty ;
      rdfs:label "powers"@en ;
      rdfs:comment "links a system to the systms its powers."@en ;
      rdfs:subPropertyOf seas:exchangesElectricityWith ;
      rdfs:domain seas:System ;
      rdfs:range seas:System ;
      owl:inverseOf seas:isPoweredBy;
      vs:term_status "testing" ;
      rdfs:isDefinedBy seas:ElectricStreetLightingSystemOntology .    

seas:wasReplacedBy a owl:ObjectProperty ;
      rdfs:label "was replaced by"@en ;
      rdfs:comment "links a System to its replaced system."@en ;
      rdfs:domain seas:System ;
      rdfs:range seas:System ;
      owl:inverseOf seas:hasReplaced;
      vs:term_status "testing" ;
      rdfs:isDefinedBy seas:ElectricStreetLightingSystemOntology . 

seas:hasReplaced a owl:ObjectProperty ;
      rdfs:label "has Replaced"@en ;
      rdfs:comment "the System to its replaced system."@en ;
      rdfs:domain seas:System ;
      rdfs:range seas:System ;
      owl:inverseOf seas:isReplacedBy;
      vs:term_status "testing" ;
      rdfs:isDefinedBy seas:ElectricStreetLightingSystemOntology . 


seas:migrationCost a owl:ObjectProperty , owl:FunctionalProperty;
      rdfs:label "migration cost"@en ;
      rdfs:comment ""@en ;
      rdfs:range seas:PriceProperty ;
      vs:term_status "testing" ;
      rdfs:isDefinedBy seas:ElectricStreetLightingSystemOntology .       


seas:expectedConsumptionOfElectricEnergy  a owl:ObjectProperty , owl:FunctionalProperty;
      rdfs:label "expected consumption of electric energy"@en ;
      rdfs:comment ""@en ;
      rdfs:subPropertyOf seas:electricEnergy ;
      rdfs:range seas:ElectricEnergyProperty ;
      vs:term_status "testing" ;
      rdfs:isDefinedBy seas:ElectricStreetLightingSystemOntology .     

seas:member  a owl:ObjectProperty , owl:FunctionalProperty;
      rdfs:label "member"@en ;
      rdfs:comment "collection or group has memeber some FeatureOfInterest. "@en ;
      rdfs:range seas:FeatureOfInterest ;
      owl:inverseOf seas:isMemberOf;
      vs:term_status "testing" ;
      rdfs:isDefinedBy seas:ElectricStreetLightingSystemOntology .           

seas:isMemberOf  a owl:ObjectProperty , owl:FunctionalProperty;
      rdfs:label "isMemberOf"@en ;
      rdfs:comment "is member of some collection or group"@en ;
      rdfs:range seas:FeatureOfInterest ;
      owl:inverseOf seas:member;
      vs:term_status "testing" ;
      rdfs:isDefinedBy seas:ElectricStreetLightingSystemOntology .      