# Copyright 2016 ITEA 12004 SEAS Project.
# 
# Licensed under the Apache License, Version 2.0 (the "License");
# you may not use this file except in compliance with the License.
# You may obtain a copy of the License at
# 
#      http://www.apache.org/licenses/LICENSE-2.0
# 
# Unless required by applicable law or agreed to in writing,
# distributed under the License is distributed on an "AS IS" BASIS,
# WITHOUT WARRANTIES OR CONDITIONS OF ANY KIND, either express or implied.
# See the License for the specific language governing permissions and
# limitations under the License.

@prefix rdf: <http://www.w3.org/1999/02/22-rdf-syntax-ns#> .
@prefix owl: <http://www.w3.org/2002/07/owl#> .
@prefix rdfs: <http://www.w3.org/2000/01/rdf-schema#> .
@prefix xsd: <http://www.w3.org/2001/XMLSchema#> .
@prefix dcterms: <http://purl.org/dc/terms/> .  
@prefix vann: <http://purl.org/vocab/vann/> .
@prefix voaf: <http://purl.org/vocommons/voaf#> .
@prefix vs: <http://www.w3.org/2003/06/sw-vocab-status/ns#> .
@prefix foaf: <http://xmlns.com/foaf/0.1/>.
@prefix ssn: <https://www.w3.org/ns/ssn/>.
@prefix dul: <http://www.ontologydesignpatterns.org/ont/dul/DUL.owl#>.
@prefix liner: <https://w3id.org/liner/>.
@prefix skos: <http://www.w3.org/2004/02/skos/core#>.
@prefix qb: <http://purl.org/linked-data/cube#>.
@prefix cdt: <http://w3id.org/lindt/custom_datatypes#>.

@prefix seas: <https://w3id.org/seas/>.
@base <https://w3id.org/seas/>.

voaf:Vocabulary a owl:Class .
dcterms:title a owl:AnnotationProperty .
dcterms:description a owl:AnnotationProperty .
dcterms:issued a owl:AnnotationProperty .
dcterms:modified a owl:AnnotationProperty .
dcterms:creator a owl:AnnotationProperty .
dcterms:contributor a owl:AnnotationProperty .
dcterms:license a owl:AnnotationProperty .
vann:preferredNamespacePrefix a owl:AnnotationProperty .
vann:preferredNamespaceUri a owl:AnnotationProperty .
vs:term_status a owl:AnnotationProperty .
foaf:Person a owl:Class .
foaf:name a owl:DatatypeProperty .



seas:ElectricLightingSystemOntology a owl:Ontology , voaf:Vocabulary ;
  dcterms:title "The SEAS Electric Street Light System Ontology."@en ;
  dcterms:description """The SEAS Electric Street Light System ontology describes Electric Street Light System."""@en ;
  dcterms:issued "2017-05-30"^^xsd:date ;
  dcterms:modified "2017-05-30"^^xsd:date ;
  dcterms:creator [  a foaf:Person; foaf:name "Lynda TEMAL"] ;
  dcterms:contributor <http://www.maxime-lefrancois.info/me#> ;
  dcterms:license <https://www.apache.org/licenses/LICENSE-2.0> ;
  vann:preferredNamespacePrefix "seas" ;
  vann:preferredNamespaceUri <https://w3id.org/seas/> ;  
  owl:imports seas:ZoneLightingOntology , seas:ElectricPowerSystemOntology, seas:ElectricLightSourceOntology , seas:GenericPropertyOntology;
  owl:versionIRI <https://w3id.org/seas/ElectricStreetLightingSystemOntology-1.0> ;
  owl:versionInfo "v1.0" .






seas:ElectricLightFixtureSystem a owl:Class ;
  rdfs:label "Electric Light Fixture System"@en ;
  rdfs:comment """An Electric Light Fixture System, light fixture (US English), light fitting (UK English), or luminaire is an electrical device used to create 
                  artificial light by use of an electric lamp. All light fixtures have a fixture body and a light socket to hold the lamp and allow for its replacement. 
                  Fixtures may also have a switch to control the light, either attached to the lamp body or attached to the power cable. (source: Wikipedia)"""@en 
                ;
  skos:prefLabel "Luminaire"@en;               
  rdfs:subClassOf seas:ElectricPowerSystem ;
  vs:term_status "testing" ;
  rdfs:isDefinedBy seas:ElectricStreetLightingSystemOntology .


seas:ElectricOutdoorLightingSystem a owl:Class ;
  rdfs:label "Electric Outdoor Lighting System"@en ;
  rdfs:comment """An Electric Outdoor Lighting System, is an Electric Light Fixture System which is used to lighting exterior areas."""@en ;
  rdfs:subClassOf seas:ElectricLightFixtureSystem ;
  vs:term_status "testing" ;
  rdfs:isDefinedBy seas:ElectricStreetLightingSystemOntology .


seas:PublicElectricLightingSystem a owl:Class ;
  rdfs:label "Public Electric Lighting System"@en ;
  rdfs:comment """A Public Electric Lighting System, is an Electric Outdoor Lighting System which is used to lighting a public area like a road, street, public place, garden etc."""@en ;
  rdfs:subClassOf seas:ElectricOutdoorLightingSystem ;
  rdfs:subClassOf [ owl:onProperty seas:connectedTo ; owl:someValuesFrom seas:StreetLightSupport];
  rdfs:subClassOf [ owl:onProperty seas:connectedTo ; 
                    owl:qualifiedCardinality "1"^^xsd:nonNegativeInteger ;
                    owl:onClass seas:PowerBox];
  rdfs:subClassOf [ rdf:type owl:Restriction ;
                                   owl:onProperty seas:hasSubSystem ;
                                   owl:someValuesFrom seas:ElectricLightSource
                                 ] ;
  rdfs:subClassOf [ owl:onProperty seas:wearState ; owl:someValuesFrom seas:WearStateProperty];  
  rdfs:subClassOf [ owl:onProperty seas:height ; owl:someValuesFrom seas:LengthProperty];                               
  vs:term_status "testing" ;
  rdfs:isDefinedBy seas:ElectricStreetLightingSystemOntology .


seas:StreetLight a owl:Class ;
  rdfs:label "Street light"@en ;
  rdfs:comment """A Steet light, light pole, lamppost, street lamp, light standard, or lamp standard is an Public Electric Lighting System which   
                  is a raised source of light on the edge of a road or path.(source: Wikipedia)"""@en,
               """A luminaire is a lighting fixture used to distribute, filter or transform light from lamps. Also called lanterns, their function is to emit, 
                   distribute and control light emitted by a light source. Usually used for track lighting, they consist of an optics, electrical devices that 
                   allow the connection of the lamp (s), a body on which these different elements are based, and Makes it possible to be fixed to a support. """@en,
               """Un luminaire est un appareil d'éclairage servant à répartir, filtrer ou transformer la lumière des lampes. Egalement appelés lanternes, 
                   leur fonction est d'émettre, de distribuer et de contrôler la lumière émise par une source lumineuse. Généralement utilisés pour l'éclairage des 
                   voies, ils se composent d'une optique, d'appareils électriques qui permettent le branchement de la (les) lampe(s), d'un corps sur lequel 
                   s'appuient ces différents éléments, et qui permet d'être fixé à un support."""@fr ;
  rdfs:subClassOf seas:PublicElectricLightingSystem ;
  vs:term_status "testing" ;
  rdfs:isDefinedBy seas:ElectricStreetLightingSystemOntology .


seas:EquipableStreetLight a owl:Class;
  rdfs:label "Equipable Street light"@en ;
  rdfs:comment """An Equipable Street light,  is a Street light which   
                  can be equipable"""@en ;
  rdfs:subClassOf seas:StreetLight ;
  rdfs:subClassOf [ owl:onProperty seas:isEquipable ; owl:hasValue "true"^^xsd:boolean ] ; 
  owl:equivalentClass [ owl:intersectionOf (seas:StreetLight [owl:onProperty seas:isEquipable ; owl:hasValue "true"^^xsd:boolean])];
  vs:term_status "testing" ;
  rdfs:isDefinedBy seas:ElectricStreetLightingSystemOntology .


seas:NoEquipableStreetLight a owl:Class;
  rdfs:label "No Equipable Street light"@en ;
  rdfs:comment """An No Equipable Street light,  is a Street light which   
                  is not equipable"""@en ;
  rdfs:subClassOf seas:StreetLight ;
  rdfs:subClassOf [ owl:onProperty seas:isEquipable ; owl:hasValue "false"^^xsd:boolean ] ; 
  owl:equivalentClass [ owl:intersectionOf (seas:StreetLight [owl:onProperty seas:isEquipable ; owl:hasValue "false"^^xsd:boolean])];
  vs:term_status "testing" ;
  rdfs:isDefinedBy seas:ElectricStreetLightingSystemOntology .

seas:TopFixationStreetLight a owl:Class;
  rdfs:label "Top Fixation Street light"@en ;
  rdfs:comment """A Top fixation Street light,  is a Street light which   
                  is fixed on the top of the support through Top fixation"""@en ;
  rdfs:subClassOf seas:StreetLight ;
  owl:equivalentClass [ owl:intersectionOf (seas:StreetLight[ owl:onProperty seas:fixedInTopTo ; owl:someValuesFrom seas:StreetLightSupport ] )];
  owl:equivalentClass [ owl:intersectionOf (seas:StreetLight[ owl:onProperty seas:connectsSystem ; owl:someValuesFrom seas:TopFixation ])] ;
  vs:term_status "testing" ;
  rdfs:isDefinedBy seas:ElectricStreetLightingSystemOntology .

seas:FacadeFixationStreetLight a owl:Class;
  rdfs:label "Facade Fixation Street light"@en ;
  rdfs:comment """A Facade fixation Street light,  is a Street light which   
                  is fixed on the facade support through Facade fixation"""@en ;
  rdfs:subClassOf seas:StreetLight ;
  owl:equivalentClass [ owl:intersectionOf (seas:StreetLight[ owl:onProperty seas:fixedInFacadeTo ; owl:someValuesFrom seas:StreetLightSupport ] )];
  owl:equivalentClass [ owl:intersectionOf (seas:StreetLight[ owl:onProperty seas:connectsSystem ; owl:someValuesFrom seas:FacadeFixation ] )];
  vs:term_status "testing" ;
  rdfs:isDefinedBy seas:ElectricStreetLightingSystemOntology .

seas:ArmFixationStreetLight a owl:Class;
  rdfs:label "Arm Fixation Street light"@en ;
  rdfs:comment """An Arm fixation Street light, is a Street light which   
                  is fixed via an arm of the support through Arm fixation"""@en ;
  rdfs:subClassOf seas:StreetLight ;
  owl:equivalentClass [ owl:intersectionOf (seas:StreetLight[ owl:onProperty seas:fixedViaAnArmTo ; owl:someValuesFrom seas:StreetLightSupport ])] ;
  owl:equivalentClass [ owl:intersectionOf (seas:StreetLight[ owl:onProperty seas:connectsSystem ; owl:someValuesFrom seas:ArmFixation ] )];
  vs:term_status "testing" ;
  rdfs:isDefinedBy seas:ElectricStreetLightingSystemOntology .

seas:LightingSupport a owl:Class ;
  rdfs:label "Lighting Support"@en ;
  rdfs:comment """Lighting Support is a support on which one or more streetLight are fixed on it"""@en ;
  rdfs:subClassOf seas:System ;
  rdfs:subClassOf [ owl:onProperty seas:wearState ; owl:someValuesFrom seas:WearStateProperty];
  rdfs:subClassOf [ owl:onProperty seas:height ; owl:someValuesFrom seas:LengthProperty];
  rdfs:subClassOf [ owl:onProperty seas:location ; owl:someValuesFrom seas:Property];
  vs:term_status "testing" ;
  rdfs:isDefinedBy seas:ElectricStreetLightingSystemOntology .


  seas:StreetLightPole a owl:Class ;
  rdfs:label "Street Light Pole"@en ;
  rdfs:comment """Street Light Pole is a Lighting Support which is used to fixe  one or more streetlight on it."""@en ;
  rdfs:subClassOf seas:LightingSupport ;
  vs:term_status "testing" ;
  rdfs:isDefinedBy seas:ElectricStreetLightingSystemOntology .


  seas:StreetLightCandelabra a owl:Class ;
  rdfs:label "Candelabra Street Light"@en ;
  rdfs:comment """Candelabra Street Light is a Lighting Support which is used to fixe one or more streetlight on it. It is generally designed like a Candelabra ."""@en ;
  rdfs:subClassOf seas:LightingSupport ;
  vs:term_status "testing" ;
  rdfs:isDefinedBy seas:ElectricStreetLightingSystemOntology .

  seas:StreetLightFacadeSupport a owl:Class ;
  rdfs:label "Street Light Facade Support"@en ;
  rdfs:comment """Street Light Facade Support is a Lighting Support which is used to fixe the streetlight."""@en ;
  rdfs:subClassOf seas:LightingSupport ;
  vs:term_status "testing" ;
  rdfs:isDefinedBy seas:ElectricStreetLightingSystemOntology .


seas:StreetLightColumnSupport a owl:Class ;
  rdfs:label "Street Light Column Support"@en ;
  rdfs:comment """Street Light Column Support is a Lighting Support which is used to fixe the streetlight."""@en ;
  rdfs:subClassOf seas:LightingSupport ;
  vs:term_status "testing" ;
  rdfs:isDefinedBy seas:ElectricStreetLightingSystemOntology .


seas:StreetLightBornSupport a owl:Class ;
  rdfs:label "Street Light Born Support"@en ;
  rdfs:comment """Street Light Born Support is a Lighting Support which is used to fixe the streetlight."""@en ;
  rdfs:subClassOf seas:LightingSupport ;
  vs:term_status "testing" ;
  rdfs:isDefinedBy seas:ElectricStreetLightingSystemOntology .


  seas:StreetLightFixation a owl:Class;
  rdfs:label "Street Light Fixation"@en ;
  rdfs:comment """Street Light Fixation is a connection which allows to fixe a streetlight to the support."""@en ;
  rdfs:subClassOf seas:Connection ;
  vs:term_status "testing" ;
  rdfs:isDefinedBy seas:ElectricStreetLightingSystemOntology .

  
  seas:StreetLightFixationPoint a owl:Class;
      rdfs:label "Street Light Fixation Point"@en;
      rdfs:comment """Street Light Fixation Point is a connection Point which allows to fixe a streetlight to the support."""@en ;
      rdfs:subClassOf seas:ConnectionPoint ;
      rdfs:subClassOf [ owl:onProperty seas:connectionPointOf ; owl:allValuesFrom   [owl:unionOf (seas:StreetLight seas:StreetLightSupport)]] ;
      rdfs:subClassOf [ owl:onProperty seas:connectsSystemThrough ; owl:allValuesFrom  seas:StreetLightFixation ] ;
      vs:term_status "testing" ;
      rdfs:isDefinedBy seas:ElectricStreetLightingSystemOntology .


  seas:ArmFixation a owl:Class;
  rdfs:label "Arm Fixation"@en ;
  rdfs:comment """Arm Fixation is a Street Light Fixation which allow to fixe a streetlight to the support via an Arm."""@en ;
  rdfs:subClassOf seas:StreetLightFixation ;
  vs:term_status "testing" ;
  rdfs:isDefinedBy seas:ElectricStreetLightingSystemOntology .


  seas:LuminaireArmFixationPoint a owl:Class;
  rdfs:label "Arm Fixation Point"@en ;
  rdfs:comment """A Luminaire Arm Fixation Point is a Street Light Fixation point which allow the point fixation between the luminaire and the ArmFixation."""@en ;
  rdfs:subClassOf seas:StreetLightFixationPoint ;
  rdfs:subClassOf [ owl:onProperty seas:connectionPointOf ; owl:allValuesFrom   seas:StreetLight ] ;
  rdfs:subClassOf [ owl:onProperty seas:connectsSystemThrough ; owl:allValuesFrom  seas:ArmFixation ] ;
  vs:term_status "testing" ;
  rdfs:isDefinedBy seas:ElectricStreetLightingSystemOntology .


 seas:SupportArmFixationPoint a owl:Class;
  rdfs:label "Arm Fixation Point"@en ;
  rdfs:comment """A Support Arm Fixation Point is a Street Light Fixation point which allow the point fixation between the support and the ArmFixation."""@en ;
  rdfs:subClassOf seas:StreetLightFixationPoint ;
  rdfs:subClassOf [ owl:onProperty seas:connectionPointOf ; owl:allValuesFrom   seas:StreetLightSupport ] ;
  rdfs:subClassOf [ owl:onProperty seas:connectsSystemThrough ; owl:allValuesFrom  seas:ArmFixation ] ;
  vs:term_status "testing" ;
  rdfs:isDefinedBy seas:ElectricStreetLightingSystemOntology .


  seas:TopFixation a owl:Class;
  rdfs:label "Top Fixation"@en ;
  rdfs:comment """Top fixation is a a Street Light Fixation which allow to fise a streetlight to the support on the top."""@en ;
  rdfs:subClassOf seas:StreetLightFixation ;
  vs:term_status "testing" ;
  rdfs:isDefinedBy seas:ElectricStreetLightingSystemOntology .

 
 seas:LuminaireTopFixationPoint a owl:Class;
  rdfs:label "Luminaire Top Fixation Point"@en ;
  rdfs:comment """A Luminaire Top Fixation Point is a Street Light Fixation point which allow the point fixation between the luminaire and the TopFixation."""@en ;
  rdfs:subClassOf seas:StreetLightFixationPoint ;
  rdfs:subClassOf [ owl:onProperty seas:connectionPointOf ; owl:allValuesFrom   seas:StreetLight ] ;
  rdfs:subClassOf [ owl:onProperty seas:connectsSystemThrough ; owl:allValuesFrom  seas:TopFixation ] ;
  vs:term_status "testing" ;
  rdfs:isDefinedBy seas:ElectricStreetLightingSystemOntology .


seas:SupportTopFixationPoint a owl:Class;
  rdfs:label "Support top Fixation Point"@en ;
  rdfs:comment """Support top Fixation Point is a Street Light Fixation point which allow the point fixation between the support and the TopFixation."""@en ;
  rdfs:subClassOf seas:StreetLightFixationPoint ;
  rdfs:subClassOf [ owl:onProperty seas:connectionPointOf ; owl:allValuesFrom   seas:StreetLightSupport] ;
  rdfs:subClassOf [ owl:onProperty seas:connectsSystemThrough ; owl:allValuesFrom  seas:TopFixation ] ;
  vs:term_status "testing" ;
  rdfs:isDefinedBy seas:ElectricStreetLightingSystemOntology .


  seas:FacadeFixation a owl:Class;
  rdfs:label "Facade Fixation"@en ;
  rdfs:comment """Facade fixation a a Street Light Fixation which allow a streetlight to the  facade support."""@en ;
  rdfs:subClassOf seas:StreetLightFixation ;
  vs:term_status "testing" ;
  rdfs:isDefinedBy seas:ElectricStreetLightingSystemOntology .

seas:LuminaireFacadeFixationPoint a owl:Class;
  rdfs:label "Luminaire Facade Fixation Point"@en ;
  rdfs:comment """A Luminaire Facade Fixation Point is a Street Light Fixation point which allow the point fixation between the luminaire and the FacadeFixation."""@en ;
  rdfs:subClassOf seas:StreetLightFixationPoint ;
  rdfs:subClassOf [ owl:onProperty seas:connectionPointOf ; owl:allValuesFrom   seas:StreetLight ] ;
  rdfs:subClassOf [ owl:onProperty seas:connectsSystemThrough ; owl:allValuesFrom  seas:FacadeFixation ] ;
  vs:term_status "testing" ;
  rdfs:isDefinedBy seas:ElectricStreetLightingSystemOntology .


seas:SupportFacadeFixationPoint a owl:Class;
  rdfs:label "Support Facade Fixation Point"@en ;
  rdfs:comment """Support Facade Fixation Point is a Street Light Fixation point which allow the point fixation between the support and the FacadeFixation."""@en ;
  rdfs:subClassOf seas:StreetLightFixationPoint ;
  rdfs:subClassOf [ owl:onProperty seas:connectionPointOf ; owl:allValuesFrom   seas:StreetLightSupport] ;
  rdfs:subClassOf [ owl:onProperty seas:connectsSystemThrough ; owl:allValuesFrom  seas:TopFixation ] ;
  vs:term_status "testing" ;
  rdfs:isDefinedBy seas:ElectricStreetLightingSystemOntology .


  seas:PowerBox a owl:Class;
      rdfs:label "Power box"@en ;
      rdfs:comment """A power box (USA) or feeder pillar (UK) is a cabinet for electrical equipment, 
                      mounted in the street and controlling the electrical supply to a number of houses in a neighborhood. (source:wikipedia)"""@en ;
      rdfs:subClassOf seas:ElectricPowerSystem ;
      rdfs:subClassOf [ owl:onProperty seas:connectedTo ; owl:someValuesFrom seas:PublicElectricLightingSystem];
      vs:term_status "testing" ;
      rdfs:isDefinedBy seas:ElectricStreetLightingSystemOntology .


seas:ElectricalBallast a owl:Class;
      rdfs:label "Electrical Ballast"@en ;
      rdfs:comment """An electrical ballast is a device placed in line with the load to limit the amount of current in an electrical circuit. 
                      It may be a fixed or variable resistor.
                      A familiar and widely used example is the inductive ballast used in fluorescent lamps to limit the current through the tube, 
                      which would otherwise rise to a destructive level due to the negative differential resistance artifact in the tube's voltage-current 
                      characteristic. Ballasts vary greatly in complexity. They may be as simple as a resistor, inductor or capacitor (or a combination of these) 
                      wired in series with the lamp; or as complex as the electronic ballasts used in compact fluorescent lamps and high-intensity discharge lamps. 
                      (source:wikipedia)"""@en ;
      rdfs:subClassOf seas:ElectricPowerSystem ;
      vs:term_status "testing" ;
      rdfs:isDefinedBy seas:ElectricStreetLightingSystemOntology .      

seas:ElectronicBallast a owl:Class;
      rdfs:label "Electronic ballast"@en ;
      rdfs:comment """An electronic ballast uses solid state electronic circuitry to provide the proper starting and operating electrical conditions to power discharge lamps.
                      An electronic ballast can be smaller and lighter than a comparably-rated magnetic one. An electronic ballast is usually quieter than a magnetic one,
                      which produces a line-frequency hum by vibration of the transformer laminations. 
                      (source:wikipedia)"""@en ;
      rdfs:subClassOf seas:ElectricalBallast ;
      vs:term_status "testing" ;
      rdfs:isDefinedBy seas:ElectricStreetLightingSystemOntology . 


seas:MagneticBallast   a owl:Class;
      rdfs:label "Magnetic ballast"@en ;
      rdfs:comment """"""@en ;
      rdfs:subClassOf seas:ElectricalBallast ;
      vs:term_status "testing" ;
      rdfs:isDefinedBy seas:ElectricStreetLightingSystemOntology .

seas:DigitalBallast   a owl:Class;
      rdfs:label "Digital ballast"@en ;
      rdfs:comment """"""@en ;
      rdfs:subClassOf seas:ElectricalBallast ;
      vs:term_status "testing" ;
      rdfs:isDefinedBy seas:ElectricStreetLightingSystemOntology .


seas:ElectricPowerDistributionNetwork   a owl:Class;
      rdfs:label "Electric Power Distribution Network"@en ;
      rdfs:comment """"""@en ;
      rdfs:subClassOf seas:ElectricPowerSystem ;
      vs:term_status "testing" ;
      rdfs:isDefinedBy seas:ElectricStreetLightingSystemOntology .


seas:UndergroundElectricPowerDistributionNetwork   a owl:Class;
      rdfs:label "Underground Electric Power Distribution Network"@en ;
      rdfs:comment """UndergroundElectricPowerDistributionNetwork is an ElectricPowerDistributionNetwork which is buried underground."""@en ;
      rdfs:subClassOf seas:ElectricPowerDistributionNetwork ;
      vs:term_status "testing" ;
      rdfs:isDefinedBy seas:ElectricStreetLightingSystemOntology .

seas:OverheadElectricPowerDistributionNetwork   a owl:Class;
      rdfs:label "Overhead Electric Power Distribution Network"@en ;
      rdfs:comment """OverheadElectricPowerDistributionNetwork is an ElectricPowerDistributionNetwork which is suspended in the air. """@en ;
      rdfs:subClassOf seas:ElectricPowerDistributionNetwork ;
      vs:term_status "testing" ;
      rdfs:isDefinedBy seas:ElectricStreetLightingSystemOntology .

seas:FacadeElectricPowerDistributionNetwork   a owl:Class;
      rdfs:label "Facade Electric Power Distribution Network"@en ;
      rdfs:comment """FacadeElectricPowerDistributionNetwork is an ElectricPowerDistributionNetwork which is hanging  along a facade."""@en ;
      rdfs:subClassOf seas:ElectricPowerDistributionNetwork;
      vs:term_status "testing" ;
      rdfs:isDefinedBy seas:ElectricStreetLightingSystemOntology .


seas:WearStateProperty a owl:Class;
      rdfs:label "Wear State Property"@en ;
      rdfs:comment """A Wear State Property is a property which is inherent in a system."""@en ;
      rdfs:subClassOf seas:Property;
      vs:term_status "testing" ;
      rdfs:isDefinedBy seas:ElectricStreetLightingSystemOntology .

seas:WearStateEvaluation a owl:Class;
      rdfs:label "Wear State Evaluation"@en ;
      rdfs:comment """A Wear State evalaution is an evaluation which is an evaluation of the Property Wears State."""@en ;
      rdfs:subClassOf seas:Evaluation;
      rdfs:subClassOf [ owl:onProperty seas:evaluationOf ; owl:someValuesFrom seas:WearStateProperty ] ;
      owl:equivalentClass [ owl:onProperty seas:evaluationOf ; owl:someValuesFrom seas:WearStateProperty ] ;
      vs:term_status "testing" ;
      rdfs:isDefinedBy seas:ElectricStreetLightingSystemOntology .


seas:GoodStateEvaluation a owl:Class;
      rdfs:label "good State Evaluation"@en ;
      rdfs:comment """A good State evalaution is a WearStateEvaluation which is an evaluation of the Property Wears State."""@en ;
      rdfs:subClassOf seas:WearStateEvaluation;
      owl:equivalentClass [ owl:onProperty seas:evaluatedSimpleValue ; owl:hasValue "Bon"^^xsd:string ] ;
      vs:term_status "testing" ;
      rdfs:isDefinedBy seas:ElectricStreetLightingSystemOntology .

seas:VetusteStateEvaluation a owl:Class;
      rdfs:label "Vetuste State Evaluation"@en ;
      rdfs:comment """A Vetuste State evalaution is a WearStateEvaluation which is an evaluation of the Property Wears State."""@en ;
      rdfs:subClassOf seas:WearStateEvaluation;
      owl:equivalentClass [ owl:onProperty seas:evaluatedSimpleValue ; owl:hasValue "Vetuste"^^xsd:string ] ;
      vs:term_status "testing" ;
      rdfs:isDefinedBy seas:ElectricStreetLightingSystemOntology .  

seas:ObsoleteStateEvaluation a owl:Class;
      rdfs:label "Obsolete State Evaluation"@en ;
      rdfs:comment """A Obsolete State evalaution is a WearStateEvaluation which is an evaluation of the Property Wears State."""@en ;
      rdfs:subClassOf seas:WearStateEvaluation;
      owl:equivalentClass [ owl:onProperty seas:evaluatedSimpleValue ; owl:hasValue "Obsolete"^^xsd:string ] ;
      vs:term_status "testing" ;
      rdfs:isDefinedBy seas:ElectricStreetLightingSystemOntology . 

seas:AverageStateEvaluation a owl:Class;
      rdfs:label "Average State Evaluation"@en ;
      rdfs:comment """A Average State evalaution is a WearStateEvaluation which is an evaluation of the Property Wears State."""@en ;
      rdfs:subClassOf seas:WearStateEvaluation;
      owl:equivalentClass [ owl:onProperty seas:evaluatedSimpleValue ; owl:hasValue "Average"^^xsd:string ] ;
      vs:term_status "testing" ;
      rdfs:isDefinedBy seas:ElectricStreetLightingSystemOntology . 


seas:wearState a owl:ObjectProperty, owl:FunctionalProperty;
      rdfs:label "wearState"@en ;
      rdfs:comment """The wearState of some physical entity."""@en ;
      rdfs:subPropertyOf seas:hasProperty ;
      rdfs:domain seas:FeatureOfInterest ;
      rdfs:range seas:WearStateProperty ;
      vs:term_status "testing" ;
      rdfs:isDefinedBy seas:GenericPropertyOntology .

seas:fixedViaAnArmTo       a owl:ObjectProperty ;
      rdfs:label "fixed with arm to"@en ;
      rdfs:comment "means that the streetlight is fixed on the support via an ArmFixation."@en ;
      rdfs:subPropertyOf seas:connectedTo ;
      rdfs:domain seas:StreetLight ;
      rdfs:range seas:StreetLightSupport ;
      vs:term_status "testing" ;
      rdfs:isDefinedBy seas:ElectricStreetLightingSystemOntology .  

seas:fixedInTopTo       a owl:ObjectProperty ;
      rdfs:label "fixed in top to"@en ;
      rdfs:comment "means that the streetlight is fixed on the support via a top fixation."@en ;
      rdfs:subPropertyOf seas:connectedTo ;
      rdfs:domain seas:StreetLight ;
      rdfs:range seas:StreetLightSupport ;
      vs:term_status "testing" ;
      rdfs:isDefinedBy seas:ElectricStreetLightingSystemOntology .  

seas:fixedInFacadeTo       a owl:ObjectProperty ;
      rdfs:label "fixed in facade to"@en ;
      rdfs:comment "means that the streetlight is fixed on the facade support via a top fixation."@en ;
      rdfs:subPropertyOf seas:connectedTo ;
      rdfs:domain seas:StreetLight ;
      rdfs:range seas:StreetLightSupport ;
      vs:term_status "testing" ;
      rdfs:isDefinedBy seas:ElectricStreetLightingSystemOntology .          

seas:isFixingSupportViaAnArmOf   a owl:ObjectProperty ;
      rdfs:label "is Fixing Support Via An Arm Of"@en ;
      rdfs:comment "means that the streetlight is fixed on the support via an ArmFixation."@en ;
      rdfs:subPropertyOf seas:connectedTo ;
      rdfs:domain seas:StreetLightSupport ;
      rdfs:range seas:StreetLight ;
      owl:inverseOf seas:fixedViaAnArmTo;
      vs:term_status "testing" ;
      rdfs:isDefinedBy seas:ElectricStreetLightingSystemOntology .  

seas:isFixingSupportInTopOf   a owl:ObjectProperty ;
      rdfs:label "is Fixing Support Via An Arm Of"@en ;
      rdfs:comment "means that the streetlight is fixed on the support via an ArmFixation."@en ;
      rdfs:subPropertyOf seas:connectedTo ;
      rdfs:domain seas:StreetLightSupport ;
      rdfs:range seas:StreetLight ;
      owl:inverseOf seas:fixedInTopTo;
      vs:term_status "testing" ;
      rdfs:isDefinedBy seas:ElectricStreetLightingSystemOntology .        

seas:isFixingSupportInFacadeOf   a owl:ObjectProperty ;
      rdfs:label "is Fixing Support Via An Arm Of"@en ;
      rdfs:comment "means that the streetlight is fixed on the support via an ArmFixation."@en ;
      rdfs:subPropertyOf seas:connectedTo ;
      rdfs:domain seas:StreetLightSupport ;
      rdfs:range seas:StreetLight ;
      owl:inverseOf seas:fixedInFacadeTo;
      vs:term_status "testing" ;
      rdfs:isDefinedBy seas:ElectricStreetLightingSystemOntology .       

seas:isEquipable a owl:DatatypeProperty;
        rdfs:comment "is equipable to check of the system is equipable or not."@en ;
      rdfs:domain seas:System ;
      rdfs:range xsd:boolean ;
      vs:term_status "testing" ;
      rdfs:isDefinedBy seas:ElectricStreetLightingSystemOntology .  

seas:isPoweredBy  a owl:ObjectProperty ;
      rdfs:label "is powered by"@en ;
      rdfs:comment "links a System to its powered system."@en ;
      rdfs:subPropertyOf seas:connectedTo ;
      rdfs:domain seas:System ;
      rdfs:range seas:System ;
      owl:inverseOf seas:powers;
      vs:term_status "testing" ;
      rdfs:isDefinedBy seas:ElectricStreetLightingSystemOntology .    

seas:powers  a owl:ObjectProperty ;
      rdfs:label "is powered by"@en ;
      rdfs:comment "links a system to the systms its powers."@en ;
      rdfs:subPropertyOf seas:connectedTo ;
      rdfs:domain seas:System ;
      rdfs:range seas:System ;
      owl:inverseOf seas:isPoweredBy;
      vs:term_status "testing" ;
      rdfs:isDefinedBy seas:ElectricStreetLightingSystemOntology .    