# Copyright 2016 ITEA 12004 SEAS Project.
# 
# Licensed under the Apache License, Version 2.0 (the "License");
# you may not use this file except in compliance with the License.
# You may obtain a copy of the License at
# 
#      http://www.apache.org/licenses/LICENSE-2.0
# 
# Unless required by applicable law or agreed to in writing,
# distributed under the License is distributed on an "AS IS" BASIS,
# WITHOUT WARRANTIES OR CONDITIONS OF ANY KIND, either express or implied.
# See the License for the specific language governing permissions and
# limitations under the License.

@prefix rdf: <http://www.w3.org/1999/02/22-rdf-syntax-ns#> .
@prefix owl: <http://www.w3.org/2002/07/owl#> .
@prefix rdfs: <http://www.w3.org/2000/01/rdf-schema#> .
@prefix xsd: <http://www.w3.org/2001/XMLSchema#> .
@prefix dcterms: <http://purl.org/dc/terms/> .  
@prefix vann: <http://purl.org/vocab/vann/> .
@prefix voaf: <http://purl.org/vocommons/voaf#> .
@prefix vs: <http://www.w3.org/2003/06/sw-vocab-status/ns#> .
@prefix foaf: <http://xmlns.com/foaf/0.1/>.
@prefix ssn: <https://www.w3.org/ns/ssn/>.
@prefix dul: <http://www.ontologydesignpatterns.org/ont/dul/DUL.owl#>.
@prefix liner: <https://w3id.org/liner/>.
@prefix skos: <http://www.w3.org/2004/02/skos/core#>.
@prefix qb: <http://purl.org/linked-data/cube#>.
@prefix cdt: <http://w3id.org/lindt/custom_datatypes#>.
@prefix pep: <https://w3id.org/pep/> .
@prefix schema: <https://schema.org/>.
@prefix gr: <http://purl.org/goodrelations/v1#>.

@prefix seas: <https://w3id.org/seas/>.
@base <https://w3id.org/seas/>.

voaf:Vocabulary a owl:Class .
dcterms:title a owl:AnnotationProperty .
dcterms:description a owl:AnnotationProperty .
dcterms:issued a owl:AnnotationProperty .
dcterms:modified a owl:AnnotationProperty .
dcterms:creator a owl:AnnotationProperty .
dcterms:contributor a owl:AnnotationProperty .
dcterms:license a owl:AnnotationProperty .
vann:preferredNamespacePrefix a owl:AnnotationProperty .
vann:preferredNamespaceUri a owl:AnnotationProperty .
vs:term_status a owl:AnnotationProperty .
foaf:Person a owl:Class .
foaf:name a owl:DatatypeProperty .



seas:StreetLightSystemOntology a owl:Ontology , voaf:Vocabulary ;
  dcterms:title "The SEAS Electric Street Light System Ontology."@en ;
  dcterms:description """The SEAS Electric Street Light System ontology describes Electric Street Light Systems.
                        Figure below shows an overview on the street light taxonomy. 
                        [![StreetlightTaxonomy](https://w3id.org/seas/lighting-taxonomy-1.png)](https://w3id.org/seas/lighting-taxonomy-1.png)
                        """@en ;
  dcterms:issued "2017-05-30"^^xsd:date ;
  dcterms:modified "2017-05-30"^^xsd:date ;
  dcterms:creator [  a foaf:Person; foaf:name "Lynda TEMAL"] ;
  dcterms:contributor <http://www.maxime-lefrancois.info/me#> ;
  dcterms:license <https://www.apache.org/licenses/LICENSE-2.0> ;
  vann:preferredNamespacePrefix "seas" ;
  vann:preferredNamespaceUri <https://w3id.org/seas/> ;  
  owl:imports seas:ZoneLightingOntology , 
              seas:CityOntology, 
              seas:ElectricPowerSystemOntology, 
              seas:ElectricLightSourceOntology , 
              seas:BuildingOntology,
              seas:BooleanPropertyOntology, 
              seas:BatteryOntology,
              seas:DeviceOntology,
              seas:PhotovoltaicOntology,
              seas:EvaluationOntology,
              seas:BooleanPropertyOntology;
  owl:versionIRI <https://w3id.org/seas/StreetLightSystemOntology-1.0> ;
  owl:versionInfo "v1.0" .



################################################################
#    Classes
#################################################################

## Lighting, LightingActuator, LightingExecution
## le but de cette modélisation est de pouvoir explicité  l'action d'eclairer pour pouvoir par la suite  les identifier dans le temps distinctement. 
## Au lieu de garder des informations sur la dernière manipumlation dateLastSwitchingOff et dateLastSwitchingOn dateLastChange

seas:Lighting a owl:Class;
  rdfs:label "Lighting"@en ;
  rdfs:comment """A lighting is the procedure that allows to illuminate some zone."""@en ;
  rdfs:subClassOf seas:Actuating ;
  vs:term_status "testing" ;
  rdfs:isDefinedBy seas:StreetLightSystemOntology .

# les luminaire peuvent avoir plusieurs fonctions parmi elle : l'eclairage public, la mise en valeur, la gestion du traffic. 
# une autre façon serait d'ajouter  un concept Function et d'jouter les differentes functions ou de de distingué  des sous classes de LightActuating 

seas:PublicLighting a owl:Class; # Eclairage public
  rdfs:label "Public Lighting"@en ;
  rdfs:comment """A public lighting is the procedure that allows to illuminate some public zone."""@en ;
  rdfs:subClassOf seas:Lighting ;
  vs:term_status "testing" ;
  rdfs:isDefinedBy seas:StreetLightSystemOntology .

## mise en valeur 
seas:Highlighting a owl:Class;
  rdfs:label "Highlighting"@en ;
  rdfs:comment """The Highlighting is the procedure that allows to highlight some public zone (places, buildings,...)."""@en ;
  rdfs:subClassOf seas:Lighting ;
  vs:term_status "testing" ;
  rdfs:isDefinedBy seas:StreetLightSystemOntology .

## Feux de circulation
seas:TrafficSignalsLighting a owl:Class;
  rdfs:label "Traffic Signals Lighting"@en ;
  rdfs:comment """The traffic signals Lighting is the procedure that give lighting signals to control the traffic flow."""@en ;
  rdfs:subClassOf seas:Lighting ;
  vs:term_status "testing" ;
  rdfs:isDefinedBy seas:StreetLightSystemOntology .


## LightActuation est une action qui se déroule dans le temps. Elle s'étend du moment ou le luminaire est mise en marche (On Commande),
## Jusqu'au moment ou il est éteind (off commande). 
seas:LightActuation a owl:Class;
    rdfs:label "Light Actuation"@en;
    rdfs:comment """A Light Actuation is the execution of the action of lighting or light Actuating.
    The figure below shows how the Streetlight are modeled like the Procedure executor execution Pattern.
    [![lightgActuator](https://w3id.org/seas/lighting-0.1-1.png)](https://w3id.org/seas/lighting-0.1-1.png)
                     """@en ;
    rdfs:subClassOf seas:Actuation ;
    rdfs:subClassOf [ owl:onProperty pep:madeBy ; owl:someValuesFrom seas:LightActuator ] ;
    rdfs:subClassOf [ owl:onProperty pep:usedProcedure ; owl:someValuesFrom seas:Lighting ] ;
    rdfs:subClassOf [ owl:onProperty seas:illuminates ; owl:someValuesFrom seas:IlluminableZone ] ;
    owl:equivalentClass [ owl:onProperty pep:usedProcedure ; owl:someValuesFrom seas:Lighting ] ;
    vs:term_status "testing" ;
    rdfs:isDefinedBy seas:StreetLightSystemOntology .




# Sub class of LightActuator 

seas:ElectricLightFixtureSystem a owl:Class ;
  rdfs:label "Electric Light Fixture System"@en ;
  rdfs:comment """An Electric Light Fixture System, light fixture (US English), light fitting (UK English), or luminaire is an electrical device used to create 
  artificial light by use of an electric lamp. All light fixtures have a fixture body and a light socket to hold the lamp and allow for its replacement.
  Fixtures may also have a switch to control the light, either attached to the lamp body or attached to the power cable. (source: Wikipedia)"""@en;
  skos:prefLabel "Luminaire"@en;               
  rdfs:subClassOf seas:LightActuator ;
  rdfs:subClassOf [ owl:onProperty pep:implements ; owl:someValuesFrom seas:Lighting ] ;
  rdfs:subClassOf [ owl:onProperty seas:illuminates ; owl:someValuesFrom seas:IlluminableZone ] ;
  owl:equivalentClass [ owl:onProperty pep:implements ; owl:someValuesFrom seas:Lighting ] ;
  vs:term_status "testing" ;
  rdfs:isDefinedBy seas:StreetLightSystemOntology .


## Luminaire extérieurs
seas:ElectricOutdoorLightingSystem a owl:Class ;
  rdfs:label "Electric Outdoor Lighting System"@en ;
  rdfs:comment """An Electric Outdoor Lighting System, is an Electric Light Fixture System which is used to light exterior areas."""@en ;
  rdfs:subClassOf seas:ElectricLightFixtureSystem ;
  vs:term_status "testing" ;
  rdfs:isDefinedBy seas:StreetLightSystemOntology .

## luminaire public extérieurs
seas:ElectricPublicLightingSystem a owl:Class ;
  rdfs:label " Electric Public Lighting System"@en ;
  rdfs:comment """A Public Electric Lighting System is an Electric Outdoor Lighting System that is used to light a public area like a road, street, public place, garden etc.
  The figure below shows some relevant connections for the Electric Public Lighting System: 
  [![lightgActuator](https://w3id.org/seas/StreetLightConnections-1.png)](https://w3id.org/seas/StreetLightConnections-1.png)"""@en ;
  rdfs:subClassOf seas:ElectricOutdoorLightingSystem ;
  rdfs:subClassOf [ owl:onProperty seas:connectedTo ; owl:someValuesFrom seas:StreetLightSupport];
  rdfs:subClassOf [ owl:onProperty seas:connectedTo ; owl:qualifiedCardinality "1"^^xsd:nonNegativeInteger ; owl:onClass seas:PowerBox];
  rdfs:subClassOf [ rdf:type owl:Restriction ; owl:onProperty seas:hasSubSystem ; owl:someValuesFrom seas:ElectricLightSource] ;
  rdfs:subClassOf [ owl:onProperty seas:condition ; owl:someValuesFrom seas:ConditionProperty];  
  rdfs:subClassOf [ owl:onProperty seas:height ; owl:someValuesFrom seas:LengthProperty]; 
  rdfs:subClassOf [ owl:onProperty seas:onState ; owl:someValuesFrom seas:BooleanProperty];       
  rdfs:subClassOf [ owl:onProperty seas:location ; owl:someValuesFrom seas:Zone];                              
  vs:term_status "testing" ;
  rdfs:isDefinedBy seas:StreetLightSystemOntology .

## les feux de signalisation (pourrait s'étendre par la suite.)
seas:TrafficControlSignal a owl:Class;
  rdfs:label "Traffic Control Signal"@en;
  rdfs:comment """Traffic lights, also known as traffic signals, traffic lamps, traffic semaphore, signal lights, stop lights, robots (in South Africa), 
  and traffic control signals (in technical parlance), are signaling devices positioned at road intersections, pedestrian crossings, and other 
  locations to control flows of traffic. (source: Wikipedia)"""@fr ;
  rdfs:subClassOf seas:ElectricPublicLightingSystem ;
  vs:term_status "testing" ;
  rdfs:isDefinedBy seas:StreetLightSystemOntology .


seas:StreetLight a owl:Class ;
  rdfs:label "Street Light"@en ;
  rdfs:comment """A Street light, light pole, lamppost, street lamp, light standard, or lamp standard is an Public Electric Lighting System which   
  is a raised source of light on the edge of a road or path.(source: Wikipedia)"""@en,
  """A Street Light is a lighting fixture used to distribute, filter or transform light from lamps. Also called lanterns, their function is to emit, 
  distribute and control light emitted by a light source. Usually used for light tracking, they consist of an optics, electrical devices that 
  allow the connection of the lamp (s), a body on which these different elements are based, and makes it possible to be fixed to a support. """@en,
  """Un luminaire est un appareil d'éclairage servant à répartir, filtrer ou transformer la lumière des lampes. Egalement appelés lanternes, 
  leur fonction est d'émettre, de distribuer et de contrôler la lumière émise par une source lumineuse. Généralement utilisés pour l'éclairage des 
  voies, ils se composent d'une optique, d'appareils électriques qui permettent le branchement de la (les) lampe(s), d'un corps sur lequel 
  s'appuient ces différents éléments, et qui permet d'être fixé à un support."""@fr ;
  rdfs:subClassOf seas:ElectricPublicLightingSystem ;
  vs:term_status "testing" ;
  rdfs:isDefinedBy seas:StreetLightSystemOntology .

## projecteurs
seas:Spotlight a owl:Class ;
  rdfs:label "Spotlight"@en ;
  rdfs:comment """A spotlight  (or searchlight) is a Street light that combines an extremely luminous source (traditionally a carbon arc lamp) with a mirrored
                   parabolic reflector to project a powerful beam of light of approximately parallel rays in a particular direction, usually constructed so that 
                   it can be swiveled about. (source: Wikipedia)"""@en ;
  rdfs:subClassOf seas:StreetLight ;
  vs:term_status "testing" ;
  rdfs:isDefinedBy seas:StreetLightSystemOntology .

seas:SolarStreetLight a owl:Class ;
  rdfs:label "Solar Street Light"@en ;
  rdfs:comment """Solar street lights are raised light sources which are powered by photovoltaic panels generally mounted on the lighting structure or integrated in the 
                pole itself. The photovoltaic panels charge a rechargeable battery, which powers a fluorescent or LED lamp during the night. (source: Wikipedia)"""@en ;
  rdfs:subClassOf seas:StreetLight ;
  rdfs:subClassOf [ owl:onProperty seas:isPoweredBy ; owl:someValuesFrom seas:Battery ] ; 
  owl:equivalentClass [owl:intersectionOf (
                            seas:StreetLight 
                            [ owl:onProperty seas:isPoweredBy ;
                              owl:someValuesFrom [ owl:intersectionOf ( 
                                seas:Battery
                                [ owl:onProperty seas:isPoweredBy ;
                                  owl:someValuesFrom seas:SolarPanel ] ) ] ] ) ] ;
  vs:term_status "testing" ;
  rdfs:isDefinedBy seas:StreetLightSystemOntology .  

seas:EquipableStreetLight a owl:Class;
  rdfs:label "Equipable Street Light"@en ;
  rdfs:comment """An Equipable Street light, is a Street light which can be equipable"""@en ;
  rdfs:subClassOf seas:StreetLight ;
  rdfs:subClassOf   [ rdf:type owl:Restriction ;
                      owl:onProperty seas:isEquipable ;
                      owl:allValuesFrom [
                        rdf:type owl:Restriction ;
                        owl:onProperty seas:simpleValue ;
                        owl:hasValue "true"^^xsd:boolean ] ] ;
  vs:term_status "testing" ;
  rdfs:isDefinedBy seas:StreetLightSystemOntology .


seas:NotEquipableStreetLight a owl:Class;
  rdfs:label "Not Equipable Street Light"@en ;
  rdfs:comment """A Not Equipable Street light, is a Street light which is not equipable."""@en ;
  rdfs:subClassOf seas:StreetLight ;
  rdfs:subClassOf   [ rdf:type owl:Restriction ;
                      owl:onProperty seas:isEquipable ;
                      owl:allValuesFrom [
                        rdf:type owl:Restriction ;
                        owl:onProperty seas:simpleValue ;
                        owl:hasValue "false"^^xsd:boolean ] ] ;
  owl:disjointWith seas:EquipableStreetLight;
  vs:term_status "testing" ;
  rdfs:isDefinedBy seas:StreetLightSystemOntology .

##J'ai utilisé le modèle System, Connection et ConnectionPoint pour modéliser comment le luminaire est fixé sur son support de fixing.
## Il dans les données que j'ai eu. ils définissent trois façons de fixer le luminaire ==> top sur le support, via une cross et sur la façade ainsi que encastré

seas:TopFixingStreetLight a owl:Class;
  rdfs:label "Top Fixing Street Light"@en ;
  rdfs:comment """A Top fixing Street light,  is a Street light which is fixed to the top of the support through Top fixing.
  The figure below shows fixing modes of the Street light on the support. This figures is about the case where the Street light is in top of the support.
  [![topFixingStreetLight](https://w3id.org/seas/StreetLightAccordingToFixingType-1.png)](https://w3id.org/seas/StreetLightAccordingToFixingType-1.png)
                  """@en ;
  rdfs:subClassOf seas:StreetLight ;
  owl:equivalentClass [ owl:intersectionOf (seas:StreetLight[ owl:onProperty seas:topFixedTo ; owl:someValuesFrom seas:StreetLightSupport ] )];
  owl:equivalentClass [ owl:intersectionOf (seas:StreetLight[ owl:onProperty seas:connectedThrough ; owl:someValuesFrom seas:TopFixing ])] ;
  vs:term_status "testing" ;
  rdfs:isDefinedBy seas:StreetLightSystemOntology .

seas:FacadeFixingStreetLight a owl:Class;
  rdfs:label "Facade Fixing Street Light"@en ;
  rdfs:comment """A Facade fixing Street light is a Street light which is fixed to the facade support through facade fixing"""@en ;
  rdfs:subClassOf seas:StreetLight ;
  owl:equivalentClass [ owl:intersectionOf (seas:StreetLight[ owl:onProperty seas:facadeFixedTo ; owl:someValuesFrom seas:StreetLightSupport ] )];
  owl:equivalentClass [ owl:intersectionOf (seas:StreetLight[ owl:onProperty seas:connectedThrough ; owl:someValuesFrom seas:FacadeFixing ] )];
  vs:term_status "testing" ;
  rdfs:isDefinedBy seas:StreetLightSystemOntology .

seas:ArmFixingStreetLight a owl:Class;
  rdfs:label "Arm Fixing Street Light"@en ;
  rdfs:comment """An Arm fixing Street light is a Street light which is fixed via an arm of the support through Arm fixing"""@en ;
  rdfs:subClassOf seas:StreetLight ;
  owl:equivalentClass [ owl:intersectionOf (seas:StreetLight[ owl:onProperty seas:armFixedTo ; owl:someValuesFrom seas:StreetLightSupport ])] ;
  owl:equivalentClass [ owl:intersectionOf (seas:StreetLight[ owl:onProperty seas:connectedThrough ; owl:someValuesFrom seas:ArmFixing ] )];
  vs:term_status "testing" ;
  rdfs:isDefinedBy seas:StreetLightSystemOntology .

seas:RecessedFloorStreetLight a owl:Class;
  rdfs:label "Recessed Floor Street Light"@en ;
  rdfs:comment """A Recessed Floor Street Light is a StreetLight which is recessed in the floor."""@en ;
  rdfs:subClassOf seas:StreetLight ;
  rdfs:subClassOf [ owl:onProperty seas:connectedTo ; owl:someValuesFrom seas:RecessedFloorLightSupport];
  owl:equivalentClass [ owl:intersectionOf (seas:StreetLight [owl:onProperty seas:connectedTo ; owl:someValuesFrom seas:RecessedFloorLightSupport])];
  vs:term_status "testing" ;
  rdfs:isDefinedBy seas:StreetLightSystemOntology .


## permet de regrouper des luminaire selon certains critères
seas:ElectricPublicLightingSystemGroup   a owl:Class;
  rdfs:label "Electric Public Lighting System Group"@en ;
  rdfs:comment """Electric Public Lighting System Group is a group system which has member only Electric Public Lighting Systems."""@en ;
  rdfs:subClassOf seas:ElectricPowerSystem ;
  rdfs:subClassOf [ owl:onProperty seas:member ; owl:allValuesFrom seas:ElectricPublicLightingSystem];
  vs:term_status "testing" ;
  rdfs:isDefinedBy seas:StreetLightSystemOntology .


seas:StreetLightSupport a owl:Class ;
  rdfs:label "Street Light Support"@en ;
  rdfs:comment """A Street Light Support is a support on which one or more street light is fixed.
                  Figure below shows the taxonomy of the street light support.
                   [![StreetlightSupportTaxonomy](https://w3id.org/seas/LightSupportTaxonomy-1.png)](https://w3id.org/seas/LightSupportTaxonomy-1.png)
              """@en ;
  rdfs:subClassOf seas:System ;
  rdfs:subClassOf [ owl:onProperty seas:condition ; owl:someValuesFrom seas:ConditionProperty];
  rdfs:subClassOf [ owl:onProperty seas:height ; owl:someValuesFrom seas:LengthProperty];
  rdfs:subClassOf [ owl:onProperty seas:location ; owl:someValuesFrom seas:Property];
  vs:term_status "testing" ;
  rdfs:isDefinedBy seas:StreetLightSystemOntology .


seas:StreetLightPole a owl:Class ;
  rdfs:label "Street Light Pole"@en ;
  rdfs:comment """A Street Light Pole is a Lighting Support which is used to fix one or more street light to it."""@en ;
  rdfs:subClassOf seas:StreetLightSupport ;
  vs:term_status "testing" ;
  rdfs:isDefinedBy seas:StreetLightSystemOntology .


seas:StreetLightCandelabra a owl:Class ;
  rdfs:label "Street Light Candelabra"@en ;
  rdfs:comment """A Candelabra Street Light is a Lighting Support which is used to fix one or more street light to it. It is generally designed like a Candelabra ."""@en ;
  rdfs:subClassOf seas:StreetLightSupport ;
  vs:term_status "testing" ;
  rdfs:isDefinedBy seas:StreetLightSystemOntology .

seas:StreetLightFacadeSupport a owl:Class ;
  rdfs:label "Street Light Facade Support"@en ;
  rdfs:comment """A Street Light Facade Support is a Lighting Support which is used to fix a facade fixing street light."""@en ;
  rdfs:subClassOf seas:StreetLightSupport ;
  vs:term_status "testing" ;
  rdfs:isDefinedBy seas:StreetLightSystemOntology .

seas:RecessedFloorLightSupport a owl:Class ;
      rdfs:label "Recessed Floor Light Support"@en ;
      rdfs:comment """A Recessed Floor Light Support is a Lighting Support which is used to fix a recessed floor light."""@en ;
      rdfs:subClassOf seas:StreetLightSupport ;
      vs:term_status "testing" ;
      rdfs:isDefinedBy seas:StreetLightSystemOntology .


seas:StreetLightColumnSupport a owl:Class ;
  rdfs:label "Street Light Column Support"@en ;
  rdfs:comment """A Street Light Column Support is a column shaped Lighting Support which is used to fix the street light."""@en ;
  rdfs:subClassOf seas:StreetLightSupport ;
  vs:term_status "testing" ;
  rdfs:isDefinedBy seas:StreetLightSystemOntology .


seas:StreetLightBollardSupport a owl:Class ;
  rdfs:label "Street Light Bollard Support"@en ;
  rdfs:comment """A Street Light Bollard Support is a Lighting Support which is used to fix the street light."""@en ;
  rdfs:subClassOf seas:StreetLightSupport ;
  vs:term_status "testing" ;
  rdfs:isDefinedBy seas:StreetLightSystemOntology .


seas:StreetLightFixing a owl:Class;
  rdfs:label "Street Light Fixing"@en ;
  rdfs:comment """A Street Light Fixing is a connection which allows to fix a street light to the support."""@en ;
  rdfs:subClassOf seas:Connection ;
  vs:term_status "testing" ;
  rdfs:isDefinedBy seas:StreetLightSystemOntology .

seas:ArmFixing a owl:Class;
  rdfs:label "Arm Fixing"@en ;
  rdfs:comment """An Arm Fixing is a Street Light Fixing which allows to arm-fix a street light to the support."""@en ;
  rdfs:subClassOf seas:StreetLightFixing ;
  vs:term_status "testing" ;
  rdfs:isDefinedBy seas:StreetLightSystemOntology .

seas:TopFixing a owl:Class;
  rdfs:label "Top Fixing"@en ;
  rdfs:comment """A Top fixing is a Streetlight Fixing which allows to fix a street light to the support on the top."""@en ;
  rdfs:subClassOf seas:StreetLightFixing ;
  vs:term_status "testing" ;
  rdfs:isDefinedBy seas:StreetLightSystemOntology .

seas:FacadeFixing a owl:Class;
  rdfs:label "Facade Fixing"@en ;
  rdfs:comment """A Facade fixing is a Street Light Fixing which allows a street light to be fixed to a facade support."""@en ;
  rdfs:subClassOf seas:StreetLightFixing ;
  vs:term_status "testing" ;
  rdfs:isDefinedBy seas:StreetLightSystemOntology .

seas:RecessedFloorFixing a owl:Class;
  rdfs:label "Recessed Floor Fixing"@en ;
  rdfs:comment """A Recessed Floor Fixing is a Street Light Fixing which allows a street light to be recessed in the floor."""@en ;
  rdfs:subClassOf seas:StreetLightFixing ;
  vs:term_status "testing" ;
  rdfs:isDefinedBy seas:StreetLightSystemOntology .




#################################################################
#    Object Properties
#################################################################


seas:armFixedTo       a owl:ObjectProperty ;
      rdfs:label "arm fixed to"@en ;
      rdfs:comment "means that the street light is arm-fixed to the support."@en ;
      rdfs:subPropertyOf seas:connectedTo ;
      rdfs:domain seas:StreetLight ;
      rdfs:range seas:StreetLightSupport ;
      vs:term_status "testing" ;
      rdfs:isDefinedBy seas:StreetLightSystemOntology .  

seas:topFixedTo       a owl:ObjectProperty ;
      rdfs:label "top fixed to"@en ;
      rdfs:comment "means that the street light is top-fixed to the support."@en ;
      rdfs:subPropertyOf seas:connectedTo ;
      rdfs:domain seas:StreetLight ;
      rdfs:range seas:StreetLightSupport ;
      vs:term_status "testing" ;
      rdfs:isDefinedBy seas:StreetLightSystemOntology .  

seas:facadeFixedTo       a owl:ObjectProperty ;
      rdfs:label "facade fixed to"@en ;
      rdfs:comment "means that the street light is fixed to the facade support via a top fixing."@en ;
      rdfs:subPropertyOf seas:connectedTo ;
      rdfs:domain seas:StreetLight ;
      rdfs:range seas:StreetLightSupport ;
      vs:term_status "testing" ;
      rdfs:isDefinedBy seas:StreetLightSystemOntology .          

seas:isEquipable a owl:ObjectProperty;
        rdfs:comment "is equipable to check if the system is equipable or not."@en ;
      rdfs:domain seas:System ;
      rdfs:range seas:BooleanProperty ;
      vs:term_status "testing" ;
      rdfs:isDefinedBy seas:StreetLightSystemOntology .  

seas:member  a owl:ObjectProperty , owl:FunctionalProperty;
      rdfs:label "member"@en ;
      rdfs:comment "collection or group has member some FeatureOfInterest. "@en ;
      rdfs:range seas:FeatureOfInterest ;
      owl:inverseOf seas:isMemberOf;
      vs:term_status "testing" ;
      rdfs:isDefinedBy seas:StreetLightSystemOntology .           

seas:isMemberOf  a owl:ObjectProperty , owl:FunctionalProperty;
      rdfs:label "isMemberOf"@en ;
      rdfs:comment "is member of some collection or group"@en ;
      rdfs:range seas:FeatureOfInterest ;
      owl:inverseOf seas:member;
      vs:term_status "testing" ;
      rdfs:isDefinedBy seas:StreetLightSystemOntology .      


#################################################################
#    General axioms
#################################################################

[] a owl:AllDisjointClasses ; 
  owl:members ( 
    seas:ArmFixingStreetLight 
    seas:FacadeFixingStreetLight  
    seas:TopFixingStreetLight
    seas:RecessedFloorStreetLight ) .

[] a owl:AllDisjointClasses ; 
  owl:members ( 
    seas:StreetLight 
    seas:StreetLightSupport  
    seas:StreetLightFixing
    seas:PowerBox
    seas:ElectricPublicLightingSystemGroup
    seas:ElectricLightSource ) .

[] a owl:AllDisjointClasses ; 
  owl:members ( 
    seas:StreetLightSupport
    seas:StreetLightBollardSupport 
    seas:StreetLightColumnSupport  
    seas:StreetLightFacadeSupport
    seas:StreetLightCandelabra
    seas:RecessedFloorLightSupport ) .     