# Copyright 2016 ITEA 12004 SEAS Project.
# 
# Licensed under the Apache License, Version 2.0 (the "License");
# you may not use this file except in compliance with the License.
# You may obtain a copy of the License at
# 
#      http://www.apache.org/licenses/LICENSE-2.0
# 
# Unless required by applicable law or agreed to in writing,
# distributed under the License is distributed on an "AS IS" BASIS,
# WITHOUT WARRANTIES OR CONDITIONS OF ANY KIND, either express or implied.
# See the License for the specific language governing permissions and
# limitations under the License.

@prefix rdf: <http://www.w3.org/1999/02/22-rdf-syntax-ns#> . #Resource data framework
@prefix owl: <http://www.w3.org/2002/07/owl#> .              #Owl ontology language
@prefix rdfs: <http://www.w3.org/2000/01/rdf-schema#> .      #RDF schema 
@prefix xsd: <http://www.w3.org/2001/XMLSchema#> .           #XML standard datatypes
@prefix dc: <http://purl.org/dc/terms/> .     #Dublin Core Metadata Initiative terms
@prefix vann: <http://purl.org/vocab/vann/> .  #A vocabulary for annotating vocabulary descriptions
@prefix voaf: <http://purl.org/vocommons/voaf#> . #A vocabulary of a friend, for describing relations between linked vocabularies
@prefix vs: <http://www.w3.org/2003/06/sw-vocab-status/ns#> . #Semantic web vocabulary status ontology
@prefix foaf: <http://xmlns.com/foaf/0.1/>.
@prefix ifc: <http://www.buildingsmart-tech.org/ifcOWL/IFC2X3_TC1#>. #IFC owl ontology
@prefix fiemser:<http://sites.google.com/site/smartappliancesproject/ontologies/fiemser#>. #Fiemser building ontology
@prefix saref: <http://ontology.tno.nl/saref#>. #SAREF smart building appliances ontology
@prefix gbxml:<http://www.gbxml.org/schema#>.     #GBXML XML schema

@prefix seas: <https://w3id.org/seas/>.
@base <https://w3id.org/seas/>.

seas:AreaOntology rdf:type voaf:Vocabulary , owl:Ontology ;
  dc:title "seas-Area ontology"@en ;
  dc:description "The Seas Building BIM related vocabulary for the ITEA SEAS (Smart Energy Aware Systems) project. This ontology is targeted for defining structure of buildings (or more general facilities) and zones related to control and measurment with links to various BIM (Building Information Model) related standards."@en ;
  dc:issued "2016-07-21"^^xsd:date ;
  dc:modified "2016-07-21"^^xsd:date ;
  dc:author <http://www.maxime-lefrancois.info/me#> ;
  dc:contributor <https://w3id.org/people/gabrieljlsantos#> ;
  dc:contributor <https://w3id.org/people/franciscosilva#> ;
  dc:contributor <https://w3id.org/people/brigidateixeira#> ;
  vann:preferredNamespacePrefix "seas" ;
  vann:preferredNamespaceUri <https://w3id.org/seas/> ;  
  owl:versionIRI <https://w3id.org/seas/AreaOntology/0.10> ;
  owl:versionInfo "v0.10" .


seas:Area a owl:Class ;
  rdfs:label "Area" ;
  rdfs:comment """A part or a section of a building, campus, town, etc."""@en ;
  rdfs:subClassOf seas:System ;
  vs:term_status "testing" ;
  rdfs:isDefinedBy seas:AreaOntology .


seas:areaConnectedTo a owl:ObjectProperty , owl:SymmetricProperty ;
  rdfs:label "area connected to"@en ;
  rdfs:comment """Links an area to another area it is connected to. The two areas may be able to exchange people, heat, light radiation, sound."""@en ;
  rdfs:subPropertyOf seas:connectedTo ;
  vs:term_status "testing" ;
  rdfs:isDefinedBy seas:SystemOntology .

# door openings
# window opening
# window closing opening
# 


seas:crossableConnectionTo a owl:ObjectProperty , owl:SymmetricProperty ;
  rdfs:label "area connected to"@en ;
  rdfs:comment """Links an area to another area it is connected to. The two areas may be able to exchange people, heat, light radiation, sound."""@en ;
  rdfs:subPropertyOf seas:connectedTo ;
  vs:term_status "testing" ;
  rdfs:isDefinedBy seas:SystemOntology .


seas:soundConnectedTo a owl:ObjectProperty , owl:SymmetricProperty ;
  rdfs:label "area connected to"@en ;
  rdfs:comment """Links an area to another area it is connected to. The two areas may be able to exchange people, heat, light radiation, sound."""@en ;
  rdfs:subPropertyOf seas:connectedTo ;
  vs:term_status "testing" ;
  rdfs:isDefinedBy seas:SystemOntology .

seas:soundConnectedTo a owl:ObjectProperty , owl:SymmetricProperty ;
  rdfs:label "area connected to"@en ;
  rdfs:comment """Links an area to another area it is connected to. The two areas may be able to exchange people, heat, light radiation, sound."""@en ;
  rdfs:subPropertyOf seas:connectedTo ;
  vs:term_status "testing" ;
  rdfs:isDefinedBy seas:SystemOntology .





seas:subAreaOf a owl:ObjectProperty ;
  rdfs:label "sub area of"@en ;
  rdfs:comment "Links an area to another it is contained in."@en ;
  rdfs:subPropertyOf seas:subSystemOf ; 
  vs:term_status "testing" ;
  rdfs:isDefinedBy seas:SystemOntology .


