# Copyright 2016 ITEA 12004 SEAS Project.
# 
# Licensed under the Apache License, Version 2.0 (the "License");
# you may not use this file except in compliance with the License.
# You may obtain a copy of the License at
# 
#      http://www.apache.org/licenses/LICENSE-2.0
# 
# Unless required by applicable law or agreed to in writing,
# distributed under the License is distributed on an "AS IS" BASIS,
# WITHOUT WARRANTIES OR CONDITIONS OF ANY KIND, either express or implied.
# See the License for the specific language governing permissions and
# limitations under the License.

@prefix rdf: <http://www.w3.org/1999/02/22-rdf-syntax-ns#> . #Resource data framework
@prefix owl: <http://www.w3.org/2002/07/owl#> .              #Owl ontology language
@prefix rdfs: <http://www.w3.org/2000/01/rdf-schema#> .      #RDF schema 
@prefix xsd: <http://www.w3.org/2001/XMLSchema#> .           #XML standard datatypes
@prefix dc: <http://purl.org/dc/terms/> .     #Dublin Core Metadata Initiative terms
@prefix vann: <http://purl.org/vocab/vann/> .  #A vocabulary for annotating vocabulary descriptions
@prefix voaf: <http://purl.org/vocommons/voaf#> . #A vocabulary of a friend, for describing relations between linked vocabularies
@prefix vs: <http://www.w3.org/2003/06/sw-vocab-status/ns#> . #Semantic web vocabulary status ontology
@prefix foaf: <http://xmlns.com/foaf/0.1/>.
@prefix qudt: <http://data.qudt.org/qudt/owl/1.0.0/qudt.owl#> . #QUDT quantities
@prefix prov: <http://www.w3.org/ns/prov#>.
@prefix ssn: <http://www.w3.org/ns/ssn/>.

@prefix seas: <https://w3id.org/seas/>.
@base <https://w3id.org/seas/>.


#Core roles and activities (for devices and systems), this is related to actor module and could specialize it but now here defined as new vocabulary
seas:EvaluationOntology a owl:Ontology , voaf:Vocabulary ;
  dc:title "seas-Evaluation ontology"@en ;
  dc:description "The Seas Evaluation ontology generalizes QUDT and OM ontologies."@en ;
  dc:issued "2016-06-08"^^xsd:date ;
  dc:modified "2016-06-08"^^xsd:date ;
  dc:contributor <http://www.vtt.fi/JarmoKalaoja> ;
  dc:author <http://www.maxime-lefrancois.info/me#> ;
  dc:contributor <http://zimmer.aprilfoolsreview.com/antoine#me> ;
  dc:contributor [a foaf:Person ; foaf:name "Erkki Siira" ] ;
  dc:contributor [a foaf:Person ; foaf:name "Takoua Ghariani" ] ;
  dc:contributor [a foaf:Person ; foaf:name "Marc Girod-Genet" ] ;
  vann:preferredNamespacePrefix "seas" ;
  vann:preferredNamespaceUri <https://w3id.org/seas/> ;  
  owl:imports seas:FeatureOfInterestOntology ;
  owl:versionIRI <https://w3id.org/seas/EvaluationOntology/0.10> ;
  owl:versionInfo "v0.10" .

# generalizations of qudt:Quantity 


seas:QuantifiableProperty a owl:Class ;
  rdfs:label "Quantifiable Property"@en ;
  rdfs:comment """An observable or operable quantifiable property of an Event or Object."""@en ;
  rdfs:subClassOf seas:Property ;
  vs:term_status "testing" ;
  rdfs:isDefinedBy seas:FeatureOfInterestOntology .

qudt:Quantity rdfs:subClassOf seas:QuantifiableProperty ;

seas:evaluation a owl:DatatypeProperty ;
  rdfs:label "has value"@en ;
  rdfs:comment """Links a quantifiable property to one of its evaluations."""@en ;
  rdfs:domain seas:QuantifiableProperty ;
  rdfs:range rdfs:Literal ;
  vs:term_status "testing" ;
  rdfs:isDefinedBy seas:FeatureOfInterestOntology .

qudt:quantityValue rdfs:subPropertyOf seas:evaluation .

seas:Evaluation a owl:Class ;
  rdfs:label "Evaluation"@en ;
  rdfs:comment """The evaluation is an indirection between a quantifiable property a literal value that quantifies the property.
  seas:Evaluation extends qudt:QuantityValue as it holds metadata about:
  (a) the context of the evaluation, expressed using context properties. Prototypical context properties are seas:time, seas:lat, seas:long. They are defined in ontology seas:EvaluationContextOntology;
  (b) zero or more skos:Concepts that enable to interpret the evaluation. For instance seas:ag-Average, seas:op-Nominal. These concepts are defined in vocabulary seas:EvaluationInterpretationVocabulary."""@en ;
  vs:term_status "testing" ;
  rdfs:isDefinedBy seas:FeatureOfInterestOntology .

qudt:QuantityValue rdfs:subClassOf seas:Evaluation .

seas:literalValue a owl:DatatypeProperty ;
  rdfs:label "as literal"@en ;
  rdfs:comment """Links a quantity value to the literal that expresses the quantity."""@en ;
  rdfs:domain seas:Property ;
  rdfs:range rdfs:Literal ;
  vs:term_status "testing" ;
  rdfs:isDefinedBy seas:FeatureOfInterestOntology .

qudt:numericalValue rdfs:subPropertyOf seas:literalValue .


# evaluation context

seas:context a rdf:Property ;
  rdfs:label "context"@en ;
  rdfs:comment "super property of properties that link evaluations to their context of validity."@en ;
  rdfs:domain seas:Evaluation ;
  vs:term_status "testing" ;
  rdfs:isDefinedBy seas:FeatureOfInterestOntology .

# evaluation interpretation

seas:interpretedAs a rdf:Property ;
  rdfs:label "interpreted as"@en ;
  rdfs:comment "Links an evaluation to a skos:Concept that enables to interpret the evaluation of a quantifiable property."@en ;
  rdfs:domain seas:Evaluation ;
  rdfs:range seas:EvaluationInterpretationConcept ;
  vs:term_status "testing" ;
  rdfs:isDefinedBy seas:FeatureOfInterestOntology .

seas:EvaluationInterpretationConcept a owl:Class ;
  rdfs:label "Evaluation Interpretation Concept"@en ;
  rdfs:comment "The class of concepts that are used to interpret evaluations of quantifiable properties."@en ;
  rdfs:subClassOf skos:Concept ;
  vs:term_status "testing" ;
  rdfs:isDefinedBy seas:FeatureOfInterestOntology .
