# Copyright 2016 ITEA 12004 SEAS Project.
# 
# Licensed under the Apache License, Version 2.0 (the "License");
# you may not use this file except in compliance with the License.
# You may obtain a copy of the License at
# 
#      http://www.apache.org/licenses/LICENSE-2.0
# 
# Unless required by applicable law or agreed to in writing,
# distributed under the License is distributed on an "AS IS" BASIS,
# WITHOUT WARRANTIES OR CONDITIONS OF ANY KIND, either express or implied.
# See the License for the specific language governing permissions and
# limitations under the License.

@prefix rdf: <http://www.w3.org/1999/02/22-rdf-syntax-ns#> . #Resource data framework
@prefix owl: <http://www.w3.org/2002/07/owl#> .     #Owl ontology language
@prefix rdfs: <http://www.w3.org/2000/01/rdf-schema#> .   #RDF schema 
@prefix xsd: <http://www.w3.org/2001/XMLSchema#> .  #XML standard datatypes
@prefix dc: <http://purl.org/dc/terms/> .  #Dublin Core Metadata Initiative terms
@prefix vann: <http://purl.org/vocab/vann/> .  #A vocabulary for annotating vocabulary descriptions
@prefix voaf: <http://purl.org/vocommons/voaf#> . #A vocabulary of a friend, for describing relations between linked vocabularies
@prefix vs: <http://www.w3.org/2003/06/sw-vocab-status/ns#> . #Semantic web vocabulary status ontology
@prefix foaf: <http://xmlns.com/foaf/0.1/>.
@prefix ssn: <https://www.w3.org/ns/ssn/>.
@prefix cc: <http://creativecommons.org/ns#>.
@prefix dul: <http://www.ontologydesignpatterns.org/ont/dul/DUL.owl#>. # The DOLCE+DnS Ultralite ontology.
@prefix liner: <https://w3id.org/liner/>.
@prefix qb: <http://purl.org/linked-data/cube#>.

@prefix seas: <https://w3id.org/seas/>.
@base <https://w3id.org/seas/>.

seas:FeatureOfInterestOntology a owl:Ontology , voaf:Vocabulary ;
  dc:title "seas-FeatureOfInterest ontology."@en ;
  dc:description "This ontology extends the core of the SSN ontology at https://www.w3.org/ns/ssn/ with references to DUL, and enriches the expressivity of Feature of interest and their properties."@en ;
  dc:issued "2016-07-01"^^xsd:date ;
  dc:modified "2016-07-01"^^xsd:date ;
  dc:author <http://www.maxime-lefrancois.info/me#> ;
  cc:license <http://creativecommons.org/licenses/by/4.0/> ;
  vann:preferredNamespacePrefix "seas" ;
  vann:preferredNamespaceUri <https://w3id.org/seas/> ;  
  owl:versionIRI <https://w3id.org/seas/FeatureOfInterestOntology/0.10> ;
  owl:versionInfo "v0.10" ;
  owl:imports <http://www.w3.org/ns/ssn> ;
  liner:entailmentRegime seas:FeatureOfInterestOntologyEntailmentRegime . 

# - FeatureOfInterest, PropertyKey, and Property, grounded on SSN and Data-Cube.

seas:FeatureOfInterest a owl:Class ;
  rdfs:label "Feature of Interest"@en ;
  rdfs:comment """A feature of interest is an abstraction of a real world phenomena (thing, person, event, etc). 

  For instance the following RDF Graph describes a car, which is defined by <movingthings>, and <energy_consumer>:

  <car/1> a seas:FeatureOfInterest ;
    seas:definition <movingthings> , <energy_consumer> .

  One may also define the class of cars as the class of things that are defined by <movingthings>.

  <car/1> a owl:Class ;
    rdfs:subClassOf [ owl:onProperty seas:definition ; owl:hasValue <movingthings> ] .

  This concept is equivalent to ssn:FeatureOfInterest, which in the first version of the SSN ontology is defined as a subclass of the union of dul:Event and dul:Object. A dul:Event is any physical, social, or mental process, event, or state. A dul:Object is any physical, social, or mental object, or a substance."""@en ;
  owl:equivalentClass ssn:FeatureOfInterest ;
  vs:term_status "testing" ;
  rdfs:isDefinedBy seas:FeatureOfInterestOntology .

seas:Property a owl:Class ;
  rdfs:label "Property"@en ;
  rdfs:comment """An observable or operable Quality of an Event or Object. That is, not a quality of an abstract entity as is also allowed by DUL's Quality, but rather an aspect of an entity that is intrinsic to and cannot exist without the entity and is observable by a sensor, or operable by an actuator. This concept is equivalent to ssn:Property, which in the first version of the SSN ontology is a subclass of dul:Quality. dul:Quality is any aspect of an Entity (but not a part of it), which cannot exist without that Entity. The Semantic Actuator Network Ontology (SAN) proposes that ssn:Property be a subClass of qudt:QuantityKind. Yet a property may be not measureable and numerically quantifiable. Indeed, it may also be a boolean, or any other kind of quality value (e.g., "UNKNOWN")."""@en ;
  owl:equivalentClass ssn:Property ;
  rdfs:subClassOf [ owl:onProperty seas:propertyKey ; owl:cardinality 1 ] ;
  rdfs:subClassOf [ owl:onProperty seas:isPropertyOf ; owl:cardinality 1 ] ;
  vs:term_status "testing" ;
  rdfs:isDefinedBy seas:FeatureOfInterestOntology .

seas:FeatureOfInterestDefinition a rdfs:Class , owl:Class ;
  rdfs:label "Feature of interest structure definition"@en ;
  rdfs:comment """The class of definitions of features of interest in terms of properties.

  For instance the following RDF Graph describes the definition of features of interest that have a geolocation and a speed property:

  <movingthings> a seas:FeatureOfInterestDefinition ;
    seas:property <geolocation> ;
    seas:property <speed> .

  <geolocation> a seas:PropertyKey .
  <speed> a seas:PropertyKey ."""@en ;
  vs:term_status "testing" ;
  rdfs:isDefinedBy seas:FeatureOfInterestOntology .

seas:PropertyKey a rdfs:Class , owl:Class ;
  rdfs:label "Property property"@en ;
  rdfs:comment "The class of components which represent a Property of the feature of interest. That is, not a quality of an abstract entity as is also allowed by DUL's Quality, but rather an aspect of an entity that is intrinsic to and cannot exist without the entity and is observable by a sensor, or operable by an actuator."@en ;
  rdfs:isDefinedBy seas:FeatureOfInterestOntology .

seas:definition a rdf:Property, owl:ObjectProperty;
  rdfs:label "definition"@en ;
  rdfs:comment "indicates the definition to which this feature of interest conforms."@en ;
  rdfs:domain seas:FeatureOfInterest ;
  rdfs:range seas:FeatureOfInterestDefinition ;
  rdfs:isDefinedBy seas:FeatureOfInterestOntology .

seas:property a rdf:Property , owl:ObjectProperty ;
  rdfs:label "property"@en ;
  rdfs:comment """Links a seas:FeatureOfInterest to a seas:Property of that feature. In the first version of the SSN ontology, this concept was defined as a subproperty of dul:hasQuality. dul:hasQuality is a relation between entities and qualities, e.g. 'Dmitri's skin is yellowish'.

  For instance, the following RDF graph describes that feature of interest <car/1> has property <car/1/speed> .

  <car/1> seas:property <car/1/speed> ."""@en ;
  rdfs:domain seas:FeatureOfInterest ;
  rdfs:range seas:Property ;
  owl:inverseOf seas:isPropertyOf ;
  vs:term_status "testing" ;
  rdfs:isDefinedBy seas:FeatureOfInterestOntology .

ssn:hasProperty rdfs:subPropertyOf seas:property .

seas:isPropertyOf a owl:ObjectProperty ;
  rdfs:label "is property of"@en ;
  rdfs:comment """Links a seas:Property of its one and only seas:FeatureOfInterest. 
  For instance, <car/1/speed> seas:isPropertyOf <car/1> . """@en ;
  rdfs:domain seas:Property ;
  rdfs:range seas:FeatureOfInterest ;
  owl:inverseOf seas:property ;
  vs:term_status "testing" ;
  rdfs:isDefinedBy seas:FeatureOfInterestOntology .

seas:propertyKey a rdf:Property , owl:ObjectProperty ;
  rdfs:label "property"@en ;
  rdfs:comment """Links:

  (a) a seas:FeatureOfInterestDefinition to a seas:PropertyKey it defines.
  
  For instance, the following RDF graph describes that feature of interest definition <movingthings> has property key <speed> .

  <movingthings> seas:propertyKey <speed> .

  (b) a seas:Property to its one and only seas:PropertyKey with respect to which it is the property of a feature of interest.
  For instance, the following RDF graph describes that property <car/1/speed> is property <speed> of its feature of interest.

  <car/1/speed> seas:propertyKey <speed> ."""@en ;
  rdfs:range seas:PropertyKey ;
  vs:term_status "testing" ;
  rdfs:isDefinedBy seas:FeatureOfInterestOntology .

[] a owl:AllDisjointClasses ;
   owl:members ( seas:FeatureOfInterest seas:FeatureOfInterestDefinition seas:Property seas:PropertyKey ) .

seas:FeatureOfInterestOntologyEntailmentRegime a liner:EntailmentRegime ;
  liner:extends liner:OWL2RL ; ## this ontology profile extends the ontology profile liner:RDFS 
  liner:extends liner:DataCube ;
  liner:axiomaticTriples seas:ProcessOntology ;
  liner:inferenceRules [
    liner:asSPARQLRules (
      <https://w3id.org/seas/FeatureOfInterestOntologyRule-1> ) ] .

<https://w3id.org/seas/FeatureOfInterestOntologyRule-1> liner:rule """
PREFIX rdfs: <http://www.w3.org/2000/01/rdf-schema#>
PREFIX seas: <https://w3id.org/seas/>
INSERT { 
  ?p a rdf:Property , owl:ObjectProperty , owl:FunctionalProperty ;
    rdfs:subPropertyOf seas:property ;
    rdfs:domain seas:FeatureOfInterest ;
    rdfs:range seas:Property .
} WHERE { 
  ?p a seas:PropertyKey .
}"""^^<urn:iana:type:application/sparql-rule> . 
