# Copyright 2016 ITEA 12004 SEAS Project.
# 
# Licensed under the Apache License, Version 2.0 (the "License");
# you may not use this file except in compliance with the License.
# You may obtain a copy of the License at
# 
#      http://www.apache.org/licenses/LICENSE-2.0
# 
# Unless required by applicable law or agreed to in writing,
# distributed under the License is distributed on an "AS IS" BASIS,
# WITHOUT WARRANTIES OR CONDITIONS OF ANY KIND, either express or implied.
# See the License for the specific language governing permissions and
# limitations under the License.

@prefix rdf: <http://www.w3.org/1999/02/22-rdf-syntax-ns#> . #Resource data framework
@prefix owl: <http://www.w3.org/2002/07/owl#> .     #Owl ontology language
@prefix rdfs: <http://www.w3.org/2000/01/rdf-schema#> .   #RDF schema 
@prefix xsd: <http://www.w3.org/2001/XMLSchema#> .  #XML standard datatypes
@prefix dc: <http://purl.org/dc/terms/> .  #Dublin Core Metadata Initiative terms
@prefix vann: <http://purl.org/vocab/vann/> .  #A vocabulary for annotating vocabulary descriptions
@prefix voaf: <http://purl.org/vocommons/voaf#> . #A vocabulary of a friend, for describing relations between linked vocabularies
@prefix vs: <http://www.w3.org/2003/06/sw-vocab-status/ns#> . #Semantic web vocabulary status ontology
@prefix foaf: <http://xmlns.com/foaf/0.1/>.
@prefix ssn: <https://www.w3.org/ns/ssn/>.
@prefix cc: <http://creativecommons.org/ns#>.
@prefix dul: <http://www.ontologydesignpatterns.org/ont/dul/DUL.owl#>. # The DOLCE+DnS Ultralite ontology.
@prefix liner: <https://w3id.org/liner/>.
@prefix skos: <http://www.w3.org/2004/02/skos/core#>.
@prefix qb: <http://purl.org/linked-data/cube#>.
@prefix cdt: <http://w3id.org/lindt/custom_datatypes#>.

@prefix seas: <https://w3id.org/seas/>.
@base <https://w3id.org/seas/>.

seas:PowerConnectionPointVocabulary a owl:Ontology , voaf:Vocabulary ;
  dc:title "seas-PowerConnectionPoint vocabulary."@en ;
  dc:description """This vocabulary defines the power connection points, and their common properties."""@en ;
  dc:issued "2016-07-19"^^xsd:date ;
  dc:modified "2016-07-19"^^xsd:date ;
  dc:author <http://www.maxime-lefrancois.info/me#> ;
  dc:contributor <https://w3id.org/people/gabrieljlsantos#> ;
  dc:contributor <https://w3id.org/people/franciscosilva#> ;
  dc:contributor <https://w3id.org/people/brigidateixeira#> ;
  cc:license <http://creativecommons.org/licenses/by/4.0/> ;
  vann:preferredNamespacePrefix "seas" ;
  vann:preferredNamespaceUri <https://w3id.org/seas/> ;  
  owl:imports seas:ConnectionPointOntology ; 
  owl:imports seas:PowerConnectionVocabulary ;
  owl:versionIRI <https://w3id.org/seas/PowerConnectionPointVocabulary/0.10> ;
  owl:versionInfo "v0.10" .

seas:PowerConnectionPoint a owl:Class ;
  rdfs:subClassOf seas:ConnectionPoint ;
  rdfs:label "Power Connection Point" ;
  rdfs:comment """The class of connection points of power systems, where electricity flows in and out."""@en ;
  vs:term_status "testing" ;
  rdfs:subClassOf [ 
    owl:onProperty seas:connectedSystem ;
    owl:allValuesFrom seas:PowerSystem ] ;
  rdfs:isDefinedBy seas:PowerConnectionPointVocabulary .

seas:incomingPower a seas:PropertyKey, rdf:Property ;
  rdfs:label "incoming Power" ;
  rdfs:comment """incoming Power is the electric power that enters the system through this connection point. It must always be positive."""@en ;
  rdfs:subPropertyOf seas:hasProperty ;
  rdfs:domain seas:PowerConnectionPoint ;
  rdfs:range seas:PowerProperty ;
  vs:term_status "testing" ;
  rdfs:isDefinedBy seas:PowerAndEnergySystemsVocabulary .

seas:outgoingPower a seas:PropertyKey, rdf:Property ;
  rdfs:label "outgoing Power" ;
  rdfs:comment """outgoing Power is the electric power that leaves the system through this connection point. It must always be positive."""@en ;
  rdfs:subPropertyOf seas:hasProperty ;
  rdfs:domain seas:PowerConnectionPoint ;
  rdfs:range seas:PowerProperty ;
  vs:term_status "testing" ;
  rdfs:isDefinedBy seas:PowerAndEnergySystemsVocabulary .

seas:powerBalance a seas:PropertyKey, rdf:Property ;
  rdfs:label "power Balance" ;
  rdfs:comment """power Balance is the difference between the electric power that enters the system, and the electric power that leaves the system through this connection point. It is positive if and only if the electric power globally entered the system."""@en ;
  rdfs:subPropertyOf seas:hasProperty ;
  rdfs:domain seas:PowerConnectionPoint ;
  rdfs:range seas:PowerProperty ;
  vs:term_status "testing" ;
  rdfs:isDefinedBy seas:PowerAndEnergySystemsVocabulary .

# energy

seas:incomingEnergy a seas:PropertyKey, rdf:Property ;
  rdfs:label "incoming Energy" ;
  rdfs:comment """incoming Energy is the electric energy that entered the system through this connection point. It must always be positive."""@en ;
  rdfs:subPropertyOf seas:hasProperty ;
  rdfs:domain seas:PowerConnectionPoint ;
  rdfs:range seas:PowerProperty ;
  vs:term_status "testing" ;
  rdfs:isDefinedBy seas:PowerAndEnergySystemsVocabulary .

seas:outgoingEnergy a seas:PropertyKey, rdf:Property ;
  rdfs:label "outgoing Energy" ;
  rdfs:comment """outgoing Energy is the electric energy that left the system through this connection point. It must always be positive."""@en ;
  rdfs:subPropertyOf seas:hasProperty ;
  rdfs:domain seas:PowerConnectionPoint ;
  rdfs:range seas:PowerProperty ;
  vs:term_status "testing" ;
  rdfs:isDefinedBy seas:PowerAndEnergySystemsVocabulary .

seas:energyBalance a seas:PropertyKey, rdf:Property ;
  rdfs:label "energy Balance" ;
  rdfs:comment """energy Balance is the difference between the electric energy that enters the system, and the electric energy that leaves the system through this connection point. It is positive if and only if the electric energy globally entered the system."""@en ;
  rdfs:subPropertyOf seas:hasProperty ;
  rdfs:domain seas:PowerConnectionPoint ;
  rdfs:range seas:PowerProperty ;
  vs:term_status "testing" ;
  rdfs:isDefinedBy seas:PowerAndEnergySystemsVocabulary .



# single-phase connection points of power systems

seas:phase a rdf:Property, owl:InverseFunctionalProperty ;
  rdfs:label "connectionPoint"@en ;
  rdfs:comment "Links a system to one of its connection points."@en ;
  rdfs:domain seas:System ;
  rdfs:range seas:ConnectionPoint ;
  owl:inverseOf seas:connectionPointOf ;
#  owl:propertyChainAxiom ( seas:connectedSystem1Of seas:connectedPoint1Of ) ;
#  owl:propertyChainAxiom ( seas:connectedSystem2Of seas:connectedPoint2Of ) ;
  vs:term_status "testing" ;
  rdfs:isDefinedBy seas:ConnectionPointOntology .

seas:plus a owl:ObjectProperty ;
  rdfs:label "plus"@en ;
  rdfs:comment "Links an electrical system to its plus wire."@en ;
  rdfs:domain seas:DirectCurrentElectricalSystem ;
  rdfs:range seas:Wire ;
  vs:term_status "testing" ;
  rdfs:isDefinedBy <http://purl.org/NET/seas#> .

seas:minus a owl:ObjectProperty ;
  rdfs:label "phase1"@en ;
  rdfs:comment "Links an electrical system to its minus wire."@en ;
  rdfs:domain seas:DirectCurrentElectricalSystem ;
  rdfs:range seas:Wire ;
  vs:term_status "testing" ;
  rdfs:isDefinedBy <http://purl.org/NET/seas#> .

seas:ground a owl:ObjectProperty ;
  rdfs:label "ground"@en ;
  rdfs:comment "Links an electrical system to its ground wire."@en ;
  rdfs:domain seas:ElectricalSystem ;
  rdfs:range seas:Wire ;
  vs:term_status "testing" ;
  rdfs:isDefinedBy <http://purl.org/NET/seas#> .

seas:neutral a owl:ObjectProperty ;
  rdfs:label "phase1"@en ;
  rdfs:comment "Links an alternating electrical system to its neutral wire."@en ;
  rdfs:domain seas:AlternatingElectricalSystem ;
  rdfs:range seas:Wire ;
  vs:term_status "testing" ;
  rdfs:isDefinedBy <http://purl.org/NET/seas#> .

seas:phaseA a owl:ObjectProperty ;
  rdfs:label "phase1"@en ;
  rdfs:comment "Links the single-phase electrical system to its phase A wire."@en ;
  rdfs:domain seas:SinglePhaseElectricalSystem ;
  rdfs:range seas:Wire ;
  vs:term_status "testing" ;
  rdfs:isDefinedBy <http://purl.org/NET/seas#> .

seas:phase1 a owl:ObjectProperty ;
  rdfs:label "phase1"@en ;
  rdfs:comment "Links the three-phase electrical system to its phase 1 wire."@en ;
  rdfs:domain seas:ThreePhaseElectricalSystem ;
  rdfs:range seas:Wire ;
  vs:term_status "testing" ;
  rdfs:isDefinedBy <http://purl.org/NET/seas#> .

seas:phase2 a owl:ObjectProperty ;
  rdfs:label "phase2"@en ;
  rdfs:comment "Links the three-phase electrical system to its phase 2 wire."@en ;
  rdfs:domain seas:ThreePhaseElectricalSystem ;
  rdfs:range seas:Wire ;
  vs:term_status "testing" ;
  rdfs:isDefinedBy <http://purl.org/NET/seas#> .

seas:phase3 a owl:ObjectProperty ;
  rdfs:label "phase3"@en ;
  rdfs:comment "Links the three-phase electrical system to its phase 3 wire."@en ;
  rdfs:domain seas:ThreePhaseElectricalSystem ;
  rdfs:range seas:Wire ;
  vs:term_status "testing" ;
  rdfs:isDefinedBy <http://purl.org/NET/seas#> .
