# Copyright 2016 ITEA 12004 SEAS Project.
# 
# Licensed under the Apache License, Version 2.0 (the "License");
# you may not use this file except in compliance with the License.
# You may obtain a copy of the License at
# 
#      http://www.apache.org/licenses/LICENSE-2.0
# 
# Unless required by applicable law or agreed to in writing,
# distributed under the License is distributed on an "AS IS" BASIS,
# WITHOUT WARRANTIES OR CONDITIONS OF ANY KIND, either express or implied.
# See the License for the specific language governing permissions and
# limitations under the License.

@prefix rdf: <http://www.w3.org/1999/02/22-rdf-syntax-ns#> . #Resource data framework
@prefix owl: <http://www.w3.org/2002/07/owl#> .     #Owl ontology language
@prefix rdfs: <http://www.w3.org/2000/01/rdf-schema#> .   #RDF schema 
@prefix xsd: <http://www.w3.org/2001/XMLSchema#> .  #XML standard datatypes
@prefix dc: <http://purl.org/dc/terms/> .  #Dublin Core Metadata Initiative terms
@prefix vann: <http://purl.org/vocab/vann/> .  #A vocabulary for annotating vocabulary descriptions
@prefix voaf: <http://purl.org/vocommons/voaf#> . #A vocabulary of a friend, for describing relations between linked vocabularies
@prefix vs: <http://www.w3.org/2003/06/sw-vocab-status/ns#> . #Semantic web vocabulary status ontology
@prefix foaf: <http://xmlns.com/foaf/0.1/>.
@prefix ssn: <https://www.w3.org/ns/ssn/>.
@prefix cc: <http://creativecommons.org/ns#>.
@prefix dul: <http://www.ontologydesignpatterns.org/ont/dul/DUL.owl#>. # The DOLCE+DnS Ultralite ontology.
@prefix liner: <https://w3id.org/liner/>.
@prefix skos: <http://www.w3.org/2004/02/skos/core#>.
@prefix qb: <http://purl.org/linked-data/cube#>.
@prefix cdt: <http://w3id.org/lindt/custom_datatypes#>.

@prefix seas: <https://w3id.org/seas/>.
@base <https://w3id.org/seas/>.

seas:PowerConnectionVocabulary a owl:Ontology , voaf:Vocabulary ;
  dc:title "seas-PowerConnection vocabulary."@en ;
  dc:description """This vocabulary defines the lossless power connections, and their common properties."""@en ;
  dc:issued "2016-07-19"^^xsd:date ;
  dc:modified "2016-07-19"^^xsd:date ;
  dc:author <http://www.maxime-lefrancois.info/me#> ;
  dc:contributor <https://w3id.org/people/gabrieljlsantos#> ;
  dc:contributor <https://w3id.org/people/franciscosilva#> ;
  dc:contributor <https://w3id.org/people/brigidateixeira#> ;
  cc:license <http://creativecommons.org/licenses/by/4.0/> ;
  vann:preferredNamespacePrefix "seas" ;
  vann:preferredNamespaceUri <https://w3id.org/seas/> ; 
  owl:imports seas:ConnectionOntology ; 
  owl:imports seas:PowerSystemVocabulary ;
  owl:versionIRI <https://w3id.org/seas/PowerConnectionVocabulary/0.10> ;
  owl:versionInfo "v0.10" .

seas:PowerConnection a owl:Class ;
  rdfs:subClassOf seas:Connection ;
  rdfs:label "Power Connection" ;
  rdfs:comment """The class of lossless connections between power systems, where electricity flows."""@en ;
  vs:term_status "testing" ;
  rdfs:subClassOf [ 
    owl:onProperty seas:connectedSystem ;
    owl:allValuesFrom seas:PowerSystem ] ;
  rdfs:isDefinedBy seas:PowerConnectionVocabulary .

seas:transferredPower a seas:PropertyKey, rdf:Property ;
  rdfs:label "transferred Power" ;
  rdfs:comment """Transferred Power is the electric power that flows from the first power system to the second power system. It is positive if and only if the electric energy flobally flows from the first power system to the second."""@en ;
  rdfs:subPropertyOf seas:hasProperty ;
  rdfs:domain seas:PowerConnection ;
  rdfs:range seas:PowerProperty ;
  vs:term_status "testing" ;
  rdfs:isDefinedBy seas:PowerAndEnergySystemsVocabulary .

seas:transferredEnergy a seas:PropertyKey, rdf:Property ;
  rdfs:label "production Power" ;
  rdfs:comment """Transferred Energy is the electric energy that flows from the first power system to the second power system. It is positive if and only if the electric energy flobally flows from the first power system to the second."""@en ;
  rdfs:subPropertyOf seas:hasProperty ;
  rdfs:domain seas:PowerConnection ;
  rdfs:range seas:EnergyProperty ;
  vs:term_status "testing" ;
  rdfs:isDefinedBy seas:PowerAndEnergySystemsVocabulary .
