# Copyright 2016 ITEA 12004 SEAS Project.
# 
# Licensed under the Apache License, Version 2.0 (the "License");
# you may not use this file except in compliance with the License.
# You may obtain a copy of the License at
# 
#      http://www.apache.org/licenses/LICENSE-2.0
# 
# Unless required by applicable law or agreed to in writing,
# distributed under the License is distributed on an "AS IS" BASIS,
# WITHOUT WARRANTIES OR CONDITIONS OF ANY KIND, either express or implied.
# See the License for the specific language governing permissions and
# limitations under the License.

@prefix rdf: <http://www.w3.org/1999/02/22-rdf-syntax-ns#> .
@prefix owl: <http://www.w3.org/2002/07/owl#> .     #Owl ontology language
@prefix rdfs: <http://www.w3.org/2000/01/rdf-schema#> .   #RDF schema 
@prefix xsd: <http://www.w3.org/2001/XMLSchema#> .  #XML standard datatypes
@prefix dc: <http://purl.org/dc/terms/> .  #Dublin Core Metadata Initiative terms
@prefix vann: <http://purl.org/vocab/vann/> .
@prefix voaf: <http://purl.org/vocommons/voaf#> .
@prefix vs: <http://www.w3.org/2003/06/sw-vocab-status/ns#> .
@prefix cc: <http://creativecommons.org/ns#>.
@prefix foaf: <http://xmlns.com/foaf/0.1/>.
@prefix ssn: <https://www.w3.org/ns/ssn/>.
@prefix cc: <http://creativecommons.org/ns#>.
@prefix dul: <http://www.ontologydesignpatterns.org/ont/dul/DUL.owl#>. # The DOLCE+DnS Ultralite ontology.
@prefix liner: <https://w3id.org/liner/>.
@prefix skos: <http://www.w3.org/2004/02/skos/core#>.
@prefix sdmx: <http://purl.org/linked-data/sdmx#>.
@prefix time: <http://www.w3.org/2006/time#>.

@prefix seas: <https://w3id.org/seas/>.
@base <https://w3id.org/seas/>.

seas:TimeVocabulary a owl:Ontology , voaf:Vocabulary ;
  dc:title "SEAS-Time Vocabulary."@en ;
  dc:description "This ontology defines a set of SKOS Concepts and ConceptSchemes for code lists. These concepts are used as metadata on instances of seas:Evaluation and enable to interpret evaluations of quantifiable properties."@en ;
  dc:issued "2016-07-05"^^xsd:date ;
  dc:modified "2016-07-24"^^xsd:date ;
  dc:creator <http://www.maxime-lefrancois.info/me#> ;
  cc:license <http://creativecommons.org/licenses/by/4.0> ;
  vann:preferredNamespacePrefix "seas" ;
  vann:preferredNamespaceUri <https://w3id.org/seas/> ;  
  owl:imports seas:EvaluationOntology ;
  owl:imports time: ;
  owl:versionIRI <https://w3id.org/seas/TimeVocabulary-1.0> ;
  owl:versionInfo "v1.0" . 

seas:temporalContext a owl:ObjectProperty ;
  rdfs:label "temporal context"@en ;
  rdfs:comment """Links a property evaluation to the temporal context on which the property aspect is evaluated."""@en ;
  rdfs:domain seas:TimeContextualizedEvaluation ;
  rdfs:range time:TemporalEntity ;
  vs:term_status "stable" ;
  rdfs:isDefinedBy seas:TimeVocabulary .

seas:TimeDependentProperty a owl:ObjectProperty ;
  rdfs:label "Time Dependent Property"@en ;
  rdfs:comment "The class of properties that usually vary over time"@en ;
  rdfs:subClassOf seas:Property ;
  rdfs:subClassOf [ owl:onProperty seas:evaluation ; owl:allValuesFrom seas:TimeContextualizedEvaluation ] ;
  vs:term_status "stable" ;
  rdfs:isDefinedBy seas:TimeVocabulary .

seas:TimeContextualizedEvaluation a owl:ObjectProperty ;
  rdfs:label "Time Contextualized Evaluation"@en ;
  rdfs:comment "The class of evaluations that have a temporal context"@en ;
  rdfs:subClassOf seas:Evaluation ;
  rdfs:subClassOf [ owl:onProperty seas:temporalContext ; owl:someValuesFrom time:TemporalEntity ] ;
  vs:term_status "stable" ;
  rdfs:isDefinedBy seas:TimeVocabulary .

  seas:InstantaneousEvaluation a owl:ObjectProperty ;
    rdfs:label "Instantaneous Evaluation"@en ;
    rdfs:comment "The class of evaluations that are relative to an instant"@en ;
    rdfs:subClassOf seas:TimeContextualizedEvaluation ;
    rdfs:subClassOf [ owl:onProperty seas:temporalContext ; owl:someValuesFrom time:Instant ] ;
    vs:term_status "stable" ;
    rdfs:isDefinedBy seas:TimeVocabulary .

  seas:TimeIntervalEvaluation a owl:ObjectProperty ;
    rdfs:label "Time Interval Evaluation"@en ;
    rdfs:comment "The class of evaluations that are relative to a time interval"@en ;
    rdfs:subClassOf seas:TimeContextualizedEvaluation ;
    rdfs:subClassOf [ owl:onProperty seas:temporalContext ; owl:someValuesFrom time:ProperInterval ] ;
    vs:term_status "stable" ;
    rdfs:isDefinedBy seas:TimeVocabulary .


# CL_TS
seas:ts a skos:ConceptScheme, sdmx:CodeList;
  rdfs:label "Time Series - codelist scheme"@en;
  skos:prefLabel "Time Series - codelist scheme"@en;
  skos:notation "CL_TS";
  rdfs:comment """This code list enables to interpret the given value with respect to the actual time series of values."""@en;
  skos:note """This code list enables to interpret the given value with respect to the actual time series of values."""@en;
  skos:definition seas:time-series ;
  rdfs:seeAlso seas:Time-series ;
  vs:term_status "stable" ;
  rdfs:isDefinedBy seas:TimeVocabulary .

seas:Ts a rdfs:Class, owl:Class;
  rdfs:subClassOf skos:Concept ;
  rdfs:label "Time Series - codelist class"@en;
  rdfs:comment """This code list enables to interpret the given value with respect to the actual time series of values."""@en;
  rdfs:seeAlso seas:time-series ;
  vs:term_status "stable" ;
  rdfs:isDefinedBy seas:TimeVocabulary . 

seas:ts-Sum a skos:Concept, seas:EvaluationInterpretationConcept, seas:Ts;
  rdfs:label "Sum"@en ;
  skos:prefLabel "Sum"@en ;
  skos:notation "sum" ;
  rdfs:comment """Constant means that the given value is the sum of the quantity value over the temporal context."""@en ;
  skos:definition """Constant means that the given quantity value is the sum of the quantity value over the temporal context."""@en ;
  skos:topConceptOf seas:ts;
  skos:inScheme   seas:ts;
  vs:term_status "stable" ;
  rdfs:isDefinedBy seas:TimeVocabulary . 

seas:ts skos:hasTopConcept seas:ts-Sum .

seas:ts-Average a skos:Concept, seas:EvaluationInterpretationConcept, seas:Ts;
  rdfs:label "Average"@en ;
  skos:prefLabel "Average"@en ;
  skos:notation "avg" ;
  rdfs:comment """Constant means that the given value is the average of the quantity value over the temporal context."""@en ;
  skos:definition """Constant means that the given quantity value is the average of the quantity value over the temporal context."""@en ;
  skos:topConceptOf seas:ts;
  skos:inScheme   seas:ts;
  vs:term_status "stable" ;
  rdfs:isDefinedBy seas:TimeVocabulary . 

seas:ts skos:hasTopConcept seas:ts-Average .

seas:ts-Minimum a skos:Concept, seas:EvaluationInterpretationConcept, seas:Ts;
  rdfs:label "Minimum"@en ;
  skos:prefLabel "Minimum"@en ;
  skos:notation "min" ;
  rdfs:comment """Constant means that the given value is the minimum of the quantity value over the temporal context."""@en ;
  skos:definition """Constant means that the given quantity value is the minimum of the quantity value over the temporal context."""@en ;
  skos:topConceptOf seas:ts;
  skos:inScheme   seas:ts;
  vs:term_status "stable" ;
  rdfs:isDefinedBy seas:TimeVocabulary . 

seas:ts skos:hasTopConcept seas:ts-Minimum .

seas:ts-Maximum a skos:Concept, seas:EvaluationInterpretationConcept, seas:Ts;
  rdfs:label "Maximum"@en ;
  skos:prefLabel "Maximum"@en ;
  skos:notation "max" ;
  rdfs:comment """Constant means that the given value is the maximum of the quantity value over the temporal context."""@en ;
  skos:definition """Constant means that the given quantity value is the maximum of the quantity value over the temporal context."""@en ;
  skos:topConceptOf seas:ts;
  skos:inScheme   seas:ts;
  vs:term_status "stable" ;
  rdfs:isDefinedBy seas:TimeVocabulary . 

seas:ts skos:hasTopConcept seas:ts-Maximum .

seas:ts-Constant a skos:Concept, seas:EvaluationInterpretationConcept, seas:Ts;
  rdfs:label "Constant"@en ;
  skos:prefLabel "Constant"@en ;
  skos:notation "const" ;
  rdfs:comment """Constant means that the given quantity value is constant over the temporal context."""@en ;
  skos:definition """Constant means that the given quantity value is constant over the temporal context."""@en ;
  skos:topConceptOf seas:ts;
  skos:inScheme   seas:ts;
  vs:term_status "stable" ;
  rdfs:isDefinedBy seas:TimeVocabulary . 

seas:ts skos:hasTopConcept seas:ts-Maximum .

# CL_EVENT
seas:evt a skos:ConceptScheme, sdmx:CodeList;
  rdfs:label "Event - codelist scheme"@en;
  skos:prefLabel "Event - codelist scheme"@en;
  skos:notation "CL_EVENT";
  rdfs:comment """Interprets a given value as the number, sum, frequency, or duration of the event evaluation."""@en;
  skos:note """Interprets a given value as the number, sum, frequency, or duration of the event evaluation."""@en;
  skos:definition seas:evt ;
  rdfs:seeAlso seas:Evt ;
  vs:term_status "stable" ;
  rdfs:isDefinedBy seas:TimeVocabulary .

seas:Evt a rdfs:Class, owl:Class;
  rdfs:subClassOf skos:Concept ;
  rdfs:label "Event - codelist class"@en;
  rdfs:comment """Interprets a given value as the number, sum, 
  frequency, or duration of the event evaluation."""@en;
  rdfs:seeAlso seas:evt ;
  vs:term_status "stable" ;
  rdfs:isDefinedBy seas:TimeVocabulary . 

seas:evt-Number a skos:Concept, seas:EvaluationInterpretationConcept, seas:Event;
  rdfs:label "Number"@en ;
  skos:prefLabel "Number"@en ;
  skos:notation "#" ;
  rdfs:comment """Number of occurence of the event on the considered temporal context."""@en ;
  skos:definition """Number of occurence of the event on the considered temporal context."""@en ;
  skos:topConceptOf seas:evt;
  skos:inScheme   seas:evt;
  vs:term_status "stable" ;
  rdfs:isDefinedBy seas:TimeVocabulary . 

seas:evt skos:hasTopConcept seas:evt-Number .

seas:evt-Frequency a skos:Concept, seas:EvaluationInterpretationConcept, seas:Event;
  rdfs:label "Frequency"@en ;
  skos:prefLabel "Frequency"@en ;
  skos:notation "Freq" ;
  rdfs:comment """Frequency of occurence of the event on the considered temporal context."""@en ;
  skos:definition """Frequency of occurence of the event on the considered temporal context."""@en ;
  skos:topConceptOf seas:evt;
  skos:inScheme   seas:evt;
  vs:term_status "stable" ;
  rdfs:isDefinedBy seas:TimeVocabulary . 

seas:evt skos:hasTopConcept seas:evt-Frequency .

seas:evt-Duration a skos:Concept, seas:EvaluationInterpretationConcept, seas:Event;
  rdfs:label "Duration"@en ;
  skos:prefLabel "Duration"@en ;
  skos:notation "duration" ;
  rdfs:comment """Duration of occurence of the event on the considered temporal context."""@en ;
  skos:definition """Duration of occurence of the event on the considered temporal context."""@en ;
  skos:topConceptOf seas:evt;
  skos:inScheme   seas:evt;
  vs:term_status "stable" ;
  rdfs:isDefinedBy seas:TimeVocabulary . 

seas:evt skos:hasTopConcept seas:evt-Duration .

seas:evt-Sum a skos:Concept, seas:EvaluationInterpretationConcept, seas:Event;
  rdfs:label "Sum"@en ;
  skos:prefLabel "Sum"@en ;
  skos:notation "Sum" ;
  rdfs:comment """Sum of occurences of the event on the considered temporal context."""@en ;
  skos:definition """Sum of occurences of the event on the considered temporal context."""@en ;
  skos:topConceptOf seas:evt;
  skos:inScheme   seas:evt;
  vs:term_status "stable" ;
  rdfs:isDefinedBy seas:TimeVocabulary . 

seas:evt skos:hasTopConcept seas:evt-Sum .

# CL_DRV
seas:drv a skos:ConceptScheme, sdmx:CodeList;
  rdfs:label "Derivation - codelist scheme"@en;
  skos:prefLabel "Derivation - codelist scheme"@en;
  skos:notation "CL_DRV";
  rdfs:comment """Interprets the value as the delta or sum of the evaluated property aspect over the given temporal context."""@en;
  skos:note """Interprets the value as the delta or sum of the evaluated property aspect over the given temporal context."""@en;
  skos:definition seas:drv ;
  rdfs:seeAlso seas:Evt ;
  vs:term_status "testing" ;
  rdfs:isDefinedBy seas:TimeVocabulary .

seas:Drv a rdfs:Class, owl:Class;
  rdfs:subClassOf skos:Concept ;
  rdfs:label "Derivation - codelist class"@en;
  rdfs:comment """Interprets the value as the delta or sum of the evaluated property aspect over the given temporal context."""@en;
  rdfs:seeAlso seas:drv ;
  vs:term_status "testing" ;
  rdfs:isDefinedBy seas:TimeVocabulary . 

seas:drv-Variation a skos:Concept, seas:EvaluationInterpretationConcept, seas:Event;
  rdfs:label "Variation"@en ;
  skos:prefLabel "Variation"@en ;
  skos:notation "Delta" ;
  rdfs:comment """Variation of the value over the temporal context."""@en ;
  skos:definition """Variation of the value over the temporal context."""@en ;
  skos:topConceptOf seas:drv;
  skos:inScheme   seas:drv;
  vs:term_status "testing" ;
  rdfs:isDefinedBy seas:TimeVocabulary . 

seas:drv skos:hasTopConcept seas:drv-Variation .

seas:drv-Sum a skos:Concept, seas:EvaluationInterpretationConcept, seas:Event;
  rdfs:label "Sum"@en ;
  skos:prefLabel "Sum"@en ;
  skos:notation "Sum" ;
  rdfs:comment """Sum of the value over the temporal context."""@en ;
  skos:definition """Sum of the value over the temporal context."""@en ;
  skos:topConceptOf seas:drv;
  skos:inScheme   seas:drv;
  vs:term_status "testing" ;
  rdfs:isDefinedBy seas:TimeVocabulary . 

seas:drv skos:hasTopConcept seas:drv-Sum .
