# Copyright 2016 ITEA 12004 SEAS Project.
# 
# Licensed under the Apache License, Version 2.0 (the "License");
# you may not use this file except in compliance with the License.
# You may obtain a copy of the License at
# 
#      http://www.apache.org/licenses/LICENSE-2.0
# 
# Unless required by applicable law or agreed to in writing,
# distributed under the License is distributed on an "AS IS" BASIS,
# WITHOUT WARRANTIES OR CONDITIONS OF ANY KIND, either express or implied.
# See the License for the specific language governing permissions and
# limitations under the License.

@prefix rdf: <http://www.w3.org/1999/02/22-rdf-syntax-ns#> . #Resource data framework
@prefix owl: <http://www.w3.org/2002/07/owl#> .     #Owl ontology language
@prefix rdfs: <http://www.w3.org/2000/01/rdf-schema#> .   #RDF schema 
@prefix xsd: <http://www.w3.org/2001/XMLSchema#> .  #XML standard datatypes
@prefix dc: <http://purl.org/dc/terms/> .  #Dublin Core Metadata Initiative terms
@prefix vann: <http://purl.org/vocab/vann/> .  #A vocabulary for annotating vocabulary descriptions
@prefix voaf: <http://purl.org/vocommons/voaf#> . #A vocabulary of a friend, for describing relations between linked vocabularies
@prefix vs: <http://www.w3.org/2003/06/sw-vocab-status/ns#> . #Semantic web vocabulary status ontology
@prefix foaf: <http://xmlns.com/foaf/0.1/>.
@prefix ssn: <https://www.w3.org/ns/ssn/>.
@prefix cc: <http://creativecommons.org/ns#>.
@prefix dul: <http://www.ontologydesignpatterns.org/ont/dul/DUL.owl#>. # The DOLCE+DnS Ultralite ontology.
@prefix liner: <https://w3id.org/liner/>.
@prefix qb: <http://purl.org/linked-data/cube#>.
@prefix qudt: <http://qudt.org/1.1/schema/qudt#>.
@prefix sd: <http://www.w3.org/ns/sparql-service-description#>.
@prefix rdfg: <http://www.w3.org/2004/03/trix/rdfg-1/>.

@prefix seas: <https://w3id.org/seas/>.
@base <https://w3id.org/seas/>.

seas:GraphOntology a owl:Ontology , voaf:Vocabulary ;
  dc:title "SEAS-Graph ontology."@en ;
  dc:description """This ontology defines RDF Graph resources, and their representations. 
  In the SEAS project, inputs and outputs of process executions are named graphs.
  The URI of such graphs is the Identification in the sense of the W3C Architecture of the World Wide Web, Volume One. The graph is the content, whereas the actual exchanged documents are representations of such content.

  This ontology defines the description of such graphs and their representations."""@en ;
  dc:issued "2016-07-27"^^xsd:date ;
  dc:modified "2016-07-27"^^xsd:date ;
  dc:author <http://www.maxime-lefrancois.info/me#> ;
  cc:license <http://creativecommons.org/licenses/by/4.0/> ;
  vann:preferredNamespacePrefix "seas" ;
  vann:preferredNamespaceUri <https://w3id.org/seas/> ;  
  owl:versionIRI <https://w3id.org/seas/GraphOntology/1.0> ;
  owl:versionInfo "v1.0" ;
  # owl:imports <http://www.w3.org/ns/ssn> ;
  liner:entailmentRegime seas:GraphOntologyEntailmentRegime . 


seas:Graph a owl:Class ;
  rdfs:label "Graph"@en ;
  rdfs:comment """The class of RDF named graphs.
  This class is aligned with class sd:Graph from the SPARQL Service Description, and class rdfg:Graph from the W3C RDF Named Graphs vocabulary.
  Instance of seas:Graph are expected to be identified by URIs. Furthermore, in accordance to the Linked Data principles, such graphs are expected to be accessible by some mechanism at their URI.
  Graphs may be described using vocabularies such as the Dublin Core, FOAF, VoID, or RDFG. 
  
  They can also be linked to validation rules they must pass, or their representations means..

   For instance, 
   <http://example.org/graph/123> a seas:Graph ;
     seas:validationRule <some_sparql_ask_rule> ;
     seas:hasRepresentation <some_representation_description> ."""@en ;
  rdfs:subClassOf [ owl:onProperty seas:validationRule ; owl:allValuesFrom seas:GraphValidationRule ] ;
  rdfs:seeAlso sd:Graph , rdfg:Graph ;
  vs:term_status "testing" ;
  rdfs:isDefinedBy seas:GraphOntology .

seas:Representation a owl:Class ;
  rdfs:label "Representation"@en ;
  rdfs:comment """The class of representations. A representation may describe:
   - means to generate a RDF graph, using for instance a RML mapping, or a XSPARQL or SPARQL-Generate rule;
   - means to generate the representation from an RDF graph, using for instance a STTL rule (aka. SPARQL-Template).

   For example, 

	<g> a seas:Representation ; 
	  seas:mediaType "application/seas;p=8FI" ; 
	  seas:liftingRule <https://w3id.org/seas/representation/8FI/lifting> ;
	  seas:loweringRule <https://w3id.org/seas/representation/8FI/lowering> ;
	  seas:representationOf [ a seas:Graph ;
	    seas:validationRule <https://w3id.org/seas/representation/8FI/validation> ] ."""@en ;
  rdfs:subClassOf [ owl:onProperty seas:validationRule ; owl:allValuesFrom seas:RepresentationValidationRule ] ;
  vs:term_status "testing" ;
  rdfs:isDefinedBy seas:GraphOntology .

seas:hasRepresentation a owl:ObjectProperty ;
  rdfs:label "has representation"@en ;
  rdfs:comment """Links a RDF graph to one of its representations."""@en ;
  rdfs:domain seas:Graph ;
  rdfs:range seas:Representation ;
  owl:inverseOf seas:representationOf ;
  vs:term_status "testing" ;
  rdfs:isDefinedBy seas:GraphOntology .

seas:representationOf a owl:ObjectProperty ;
  rdfs:label "representation of"@en ;
  rdfs:comment """Links a representation to a RDF graph content it represents."""@en ;
  rdfs:domain seas:Representation ;
  rdfs:range seas:Graph ;
  owl:inverseOf seas:hasRepresentation ;
  vs:term_status "testing" ;
  rdfs:isDefinedBy seas:GraphOntology .

seas:mediaType a owl:DatatypeProperty ;
  rdfs:label "media type"@en ;
  rdfs:comment "Links a representation to its media type"@en ;
  rdfs:domain seas:GraphRepresentation ;
  vs:term_status "testing" ;
  rdfs:isDefinedBy seas:GraphOntology .

seas:validationRule a owl:ObjectProperty ;
  rdfs:label "validation rule"@en ;
  rdfs:comment """Links a resource to another resource it should validate against. Such resources may have various representations."""@en ;
  vs:term_status "testing" ;
  rdfs:isDefinedBy seas:GraphOntology .

seas:GraphValidationRule a owl:Class ;
  rdfs:label "Graph Validation Rule"@en ;
  rdfs:comment """The class of graph validation rules resources. 
  Such resources may have various representations:
  - a RDF Graph representation that contains SHACL instances;
  - a ShEx document;
  - a SPARQL ASK rule.

  For example, 

  <g> a seas:Graph ;
    seas:validationRule <v> .

  To validate conformance of graph <g>, an engine must first obtain the RDF Graph of name <g>, then operate a GET request URI <v>. Then if for example a representation of the resource at <v> with media type application/sparql-query can be obtained, then this query is run against G. If the result is true, then G validates against <v>. 

  In the version 1.0 of the SEAS framework, SEAS engines MUST be able to validate a graph against SPARQL ASK rules. Other validation formalisms are optional."""@en ;
  vs:term_status "testing" ;
  rdfs:isDefinedBy seas:GraphOntology .

seas:RepresentationValidationRule a owl:Class ;
  rdfs:label "Representation Validation Rule"@en ;
  rdfs:comment """The class of representation validation rules resources. 
  Such resources may have various representations:
  - a JSON Schema for JSON representations;
  - a XML Schema for XML representations;
  - a XPath query that must retrieve an element to validate."""@en ;
  vs:term_status "testing" ;
  rdfs:isDefinedBy seas:GraphOntology .


seas:liftingRule a owl:ObjectProperty ;
  rdfs:label "lifting rule"@en ;
  rdfs:comment """Links a graph representation to a resource that enables to lift it to a RDF Graph."""@en ;
  rdfs:domain seas:GraphRepresentation ;
  rdfs:range seas:LiftingRule ;
  vs:term_status "testing" ;
  rdfs:isDefinedBy seas:GraphOntology .

seas:LiftingRule a owl:Class ;
  rdfs:label "Lifting Rule"@en ;
  rdfs:comment """The class of rules that enable RDF lifting. Applied to a resource representation, a lifting rule enables to obtain a RDF graph resource.
  Such rules may have various representations, such as a RML mapping, a  SPARQL-Generate or a XSPARQL query."""@en ;
  vs:term_status "testing" ;
  rdfs:isDefinedBy seas:GraphOntology .


seas:loweringRule a owl:ObjectProperty ;
  rdfs:label "lowering rule"@en ;
  rdfs:comment """Links a graph representation to a resource that enables to lower a RDF Graph to this representation."""@en ;
  rdfs:domain seas:GraphRepresentation ;
  rdfs:range seas:LoweringRule ;
  vs:term_status "testing" ;
  rdfs:isDefinedBy seas:GraphOntology .

seas:LoweringRule a owl:Class ;
  rdfs:label "Lowering Rule"@en ;
  rdfs:comment """The class of rules that enable RDF lowering. Applied to a RDF graph, a lowering rule enables to obtain a representation of this resource. Such rules may have various representations, such as a STTL rule."""@en ;
  vs:term_status "testing" ;
  rdfs:isDefinedBy seas:GraphOntology .
  